PREFIX :            <http://www.w3.org/ns/prov#>
PREFIX dcterms:     <http://purl.org/dc/terms/>
PREFIX dqv:         <http://www.w3.org/ns/dqv#>
PREFIX foaf:        <http://xmlns.com/foaf/0.1/>
PREFIX owl:         <http://www.w3.org/2002/07/owl#>
PREFIX prov:        <http://www.w3.org/ns/prov#>
PREFIX rdf:         <http://www.w3.org/1999/02/22-rdf-syntax-ns#>
PREFIX rdfs:        <http://www.w3.org/2000/01/rdf-schema#>
PREFIX schema:      <http://schema.org/>
PREFIX skos:        <http://www.w3.org/2004/02/skos/core#>
PREFIX sosa:        <http://www.w3.org/ns/sosa/>
PREFIX sosa-act:    <http://www.w3.org/ns/sosa/act/>
PREFIX sosa-common: <http://www.w3.org/ns/sosa/common/>
PREFIX sosa-dep:    <http://www.w3.org/ns/sosa/dep/>
PREFIX sosa-obs:    <http://www.w3.org/ns/sosa/obs/>
PREFIX sosa-sam:    <http://www.w3.org/ns/sosa/sam/>
PREFIX sp:          <http://www.w3.org/ns/sosa/prov/>
PREFIX ssn:         <http://www.w3.org/ns/ssn/>
PREFIX ssn-act:     <http://www.w3.org/ns/ssn/act/>
PREFIX ssn-common:  <http://www.w3.org/ns/ssn/common/>
PREFIX ssn-dep:     <http://www.w3.org/ns/ssn/dep/>
PREFIX ssn-obs:     <http://www.w3.org/ns/ssn/obs/>
PREFIX ssn-sam:     <http://www.w3.org/ns/ssn/sam/>
PREFIX time:        <http://www.w3.org/2006/time#>
PREFIX xsd:         <http://www.w3.org/2001/XMLSchema#>

ssn:    rdf:type             owl:Ontology;
        rdfs:comment         "Please report any errors to the W3C Spatial Data on the Web Working Group via the SDW WG Public List public-sdw-wg@w3.org"@en;
        rdfs:seeAlso         <https://www.w3.org/2015/spatial/wiki/Semantic_Sensor_Network_Ontology>;
        dcterms:created      "2017-04-17"^^xsd:date;
        dcterms:creator      [ rdf:type   foaf:Agent;
                               foaf:name  "W3C/OGC Spatial Data on the Web Working Group"@en
                             ];
        dcterms:description  "This ontology describes sensors, actuators and observations, and related concepts. It does not describe domain concepts, time, locations, etc. these are intended to be included from other ontologies via OWL imports."@en , "\n  This module imports all the axiomatizations of the SOSA terms, and adds cross-module axioms. \n  "@en;
        dcterms:license      <http://www.w3.org/Consortium/Legal/2015/copyright-software-and-document> , <http://www.opengeospatial.org/ogc/Software>;
        dcterms:modified     "2024-02-03"^^xsd:date;
        dcterms:rights       "Copyright 2025 W3C/OGC.";
        dcterms:title        "Semantic Sensor Network Ontology"@en;
        owl:imports          sosa: , ssn-dep: , ssn-sam: , ssn-obs: , ssn-act:;
        owl:priorVersion     <http://www.w3.org/ns/ssn/2017/>;
        owl:versionIRI       <http://www.w3.org/ns/ssn/2023/>;
        owl:versionInfo      "New modular version of the SSN ontology. \n\nThis ontology was originally developed in 2009-2011 by the W3C Semantic Sensor Networks Incubator Group (SSN-XG). For more information on the group's activities see: http://www.w3.org/2005/Incubator/ssn/. The ontology was revised and modularized in 2015-2017 by the W3C/OGC Spatial Data on the Web Working Group, see: https://www.w3.org/2015/spatial/wiki/Semantic_Sensor_Network_Ontology. \n\nIn particular, (a) the scope is extended to include actuation and sampling; (b) the core concepts and properties are factored out into the SOSA ontology. The SSN ontology imports SOSA and adds formal axiomatization consistent with the text definitions in SOSA, and adds classes and properties to accommodate the scope of the original SSN ontology. "@en;
        skos:historyNote     "\n  Terms in the ssn: namespace have equivalence axioms to terms declared in the sosa: namespace, and are marked 'deprecated'. \n  The axiomatization from the 2017 version of the standard is preserved. \n\n  Terms in the sosa: namespace do not carry symmetric equivalent axioms. \n  Axiomatization only uses sosa: terms. \n  ";
        skos:scopeNote       "The SSN module contains an axiomatization of the core terms from the SOSA module (serialized in the sosa:ttl file) plus some deprecated terms in the ssn: namespace. " .

ssn-sam:  rdf:type           owl:Ontology;
        dcterms:created      "2024-02-02"^^xsd:date;
        dcterms:creator      [ rdf:type   foaf:Agent;
                               foaf:name  "W3C/OGC Spatial Data on the Web Working Group"@en
                             ];
        dcterms:description  "Sampling classes and properties for the SSN Ontology."@en;
        dcterms:license      <http://www.opengeospatial.org/ogc/Software> , <http://www.w3.org/Consortium/Legal/2015/copyright-software-and-document>;
        dcterms:rights       "Copyright 2025 W3C/OGC.";
        dcterms:title        "Sensor, Observation, Sample, and Actuator (SOSA) Ontology - actuation module"@en;
        owl:imports          ssn-common: , sosa-sam: .

ssn-obs:  rdf:type           owl:Ontology;
        dcterms:created      "2024-02-02"^^xsd:date;
        dcterms:creator      [ rdf:type   foaf:Agent;
                               foaf:name  "W3C/OGC Spatial Data on the Web Working Group"@en
                             ];
        dcterms:description  "Observation classes and properties for the SSN Ontology."@en;
        dcterms:license      <http://www.opengeospatial.org/ogc/Software> , <http://www.w3.org/Consortium/Legal/2015/copyright-software-and-document>;
        dcterms:rights       "Copyright 2025 W3C/OGC.";
        dcterms:title        "Sensor, Observation, Sample, and Actuator (SOSA) Ontology - actuation module"@en;
        owl:imports          ssn-common: , sosa-obs: .

ssn-common:  rdf:type        owl:Ontology;
        dcterms:created      "2024-02-03"^^xsd:date;
        dcterms:creator      [ rdf:type   foaf:Agent;
                               foaf:name  "W3C/OGC Spatial Data on the Web Working Group"@en
                             ];
        dcterms:description  "Core classes and properties for the SSN Ontology.\n  This module adds RDFS and OWL axioms to the terms defined in SOSA Core\n  "@en;
        dcterms:license      <http://www.opengeospatial.org/ogc/Software> , <http://www.w3.org/Consortium/Legal/2015/copyright-software-and-document>;
        dcterms:rights       "Copyright 2025 W3C/OGC.";
        dcterms:title        "SSN Ontology - core module"@en;
        owl:imports          sosa-common: .

ssn-act:  rdf:type           owl:Ontology;
        dcterms:created      "2024-02-02"^^xsd:date;
        dcterms:creator      [ rdf:type   foaf:Agent;
                               foaf:name  "W3C/OGC Spatial Data on the Web Working Group"@en
                             ];
        dcterms:description  "Actuation classes and properties for the SSN Ontology.\n  This module adds RDFS and OWL axioms to the terms defined in SOSA Actuation\n  "@en , "Actuation classes and properties for the SSN Ontology."@en;
        dcterms:license      <http://www.opengeospatial.org/ogc/Software> , <http://www.w3.org/Consortium/Legal/2015/copyright-software-and-document>;
        dcterms:rights       "Copyright 2025 W3C/OGC.";
        dcterms:title        "SSN Ontology - actuation module"@en , "Sensor, Observation, Sample, and Actuator (SOSA) Ontology - actuation module"@en;
        owl:imports          ssn-common: , sosa-act: .

sosa:   rdf:type             owl:Ontology;
        dcterms:created      "2017-04-17"^^xsd:date;
        dcterms:creator      [ rdf:type   foaf:Agent;
                               foaf:name  "W3C/OGC Spatial Data on the Web Working Group"@en
                             ];
        dcterms:description  "\n  This module imports all the terms in the SOSA module, and adds cross-module annotations (domain/rangeIncludes). \n  "@en;
        dcterms:license      <http://www.opengeospatial.org/ogc/Software> , <http://www.w3.org/Consortium/Legal/2015/copyright-software-and-document>;
        dcterms:modified     "2024-02-03"^^xsd:date;
        dcterms:rights       "Copyright 2025 W3C/OGC.";
        dcterms:title        "Sensor, Observation, Sample, and Actuator (SOSA) Ontology"@en;
        owl:imports          sosa-dep: , sosa-sam: , sosa-obs: , sosa-act:;
        owl:priorVersion     <http://www.w3.org/ns/sosa/2017/>;
        owl:versionIRI       <http://www.w3.org/ns/sosa/2023/> .

sosa:usedForExecutionHasResult
        rdf:type                owl:ObjectProperty;
        rdfs:isDefinedBy        sosa-sam:;
        rdfs:label              "used for execution has result"@en;
        schema:domainIncludes   sosa:SamplingProcedure;
        schema:rangeIncludes    sosa:SampleCollection , sosa:Sample;
        owl:inverseOf           sosa:isResultOfUsedProcedure;
        owl:propertyChainAxiom  ( sosa:usedForExecution sosa:hasResult );
        skos:definition         "\n  relation from a Procedure to a Sample or SampleCollection made by it\n  "@en .

sosa:madeSamplingHasResult
        rdf:type                owl:ObjectProperty;
        rdfs:isDefinedBy        sosa-sam:;
        rdfs:label              "made sampling has result"@en;
        schema:domainIncludes   sosa:Sampler;
        schema:rangeIncludes    sosa:SampleCollection , sosa:Sample;
        owl:inverseOf           sosa:isResultOfMadeBySampler;
        owl:propertyChainAxiom  ( sosa:madeSampling sosa:hasResult );
        skos:definition         "\n  relation from a Sampler to a Sample or SampleCollection made by it\n  "@en .

sosa:madeSampling  rdf:type    owl:ObjectProperty;
        rdfs:isDefinedBy       sosa-sam:;
        rdfs:label             "made sampling"@en;
        rdfs:subPropertyOf     sosa:madeExecution;
        schema:domainIncludes  sosa:Sampler;
        schema:rangeIncludes   sosa:SamplingCollection , sosa:Sampling;
        owl:inverseOf          sosa:madeBySampler;
        skos:definition        "\n  relation from a Sampler to the Sampling or SamplingCollection it has made\n  "@en .

sosa:madeBySampler  rdf:type   owl:ObjectProperty;
        rdfs:isDefinedBy       sosa-sam:;
        rdfs:label             "made by sampler"@en;
        rdfs:subPropertyOf     sosa:madeBySystem;
        schema:domainIncludes  sosa:SamplingCollection , sosa:Sampling;
        schema:rangeIncludes   sosa:Sampler;
        owl:inverseOf          sosa:madeSampling;
        skos:definition        "\n  relation from an act of Sampling to the Sampler that made it\n  "@en .

sosa:isSampleOfUltimateFOI
        rdf:type               owl:ObjectProperty;
        rdfs:isDefinedBy       sosa-sam:;
        rdfs:label             "has sampled feature"@en;
        schema:domainIncludes  sosa:SampleCollection , sosa:Sample;
        schema:rangeIncludes   sosa:FeatureOfInterest;
        owl:inverseOf          sosa:featureHasUltimateSample;
        skos:definition        "\n  relation from a Sample or SampleCollection to the ultimate FeatureOfInterest that it is intended to be representative of; i.e., the end of a chain of isSampleOf relations\n  "@en .

sosa:isResultOfUsedProcedure
        rdf:type                owl:ObjectProperty;
        rdfs:isDefinedBy        sosa-sam:;
        rdfs:label              "is a result of used procedure"@en;
        schema:domainIncludes   sosa:SampleCollection , sosa:Sample;
        schema:rangeIncludes    sosa:SamplingProcedure;
        owl:inverseOf           sosa:usedForExecutionHasResult;
        owl:propertyChainAxiom  ( sosa:isResultOf sosa:usedProcedure );
        skos:definition         "\n  relation from a Sample or SampleCollection to the Procedure (plan) used to make it\n  "@en .

sosa:isResultOfMadeBySampler
        rdf:type                owl:ObjectProperty;
        rdfs:isDefinedBy        sosa-sam:;
        rdfs:label              "is a result of made by sampler"@en;
        schema:domainIncludes   sosa:SampleCollection , sosa:Sample;
        schema:rangeIncludes    sosa:Sampler;
        owl:inverseOf           sosa:madeSamplingHasResult;
        owl:propertyChainAxiom  ( sosa:isResultOf sosa:madeBySampler );
        skos:definition         "\n  relation from a Sample or SampleCollection to the Sampler that made it\n  "@en .

sosa:isOriginalSampleOf
        rdf:type               owl:ObjectProperty;
        rdfs:isDefinedBy       sosa-sam:;
        rdfs:label             "is original sample  of"@en;
        schema:domainIncludes  sosa:Sample;
        schema:rangeIncludes   sosa:SampleCollection , sosa:Sample;
        owl:inverseOf          sosa:hasOriginalSample;
        skos:definition        "\n  relation from the initial Sample collected from the ultimate FeatureOfInterest to a downstream Sample or SampleCollection\n  "@en .

sosa:hasSample  rdf:type       owl:ObjectProperty;
        rdfs:isDefinedBy       sosa-sam:;
        rdfs:label             "has sample"@en;
        schema:domainIncludes  sosa:FeatureOfInterest;
        schema:rangeIncludes   sosa:Sample;
        owl:inverseOf          sosa:isSampleOf;
        skos:definition        "\n  relation from a FeatureOfInterest to the Sample or SampleCollection used to represent it\n  "@en .

sosa:hasOriginalSample
        rdf:type               owl:ObjectProperty;
        rdfs:isDefinedBy       sosa-sam:;
        rdfs:label             "has original sample"@en;
        schema:domainIncludes  sosa:SampleCollection , sosa:Sample;
        schema:rangeIncludes   sosa:Sample;
        owl:inverseOf          sosa:isOriginalSampleOf;
        skos:definition        "\n  relation from a Sample or SampleCollection to the initial Sample collected from the ultimate FeatureOfInterest\n  "@en .

sosa:featureHasUltimateSample
        rdf:type               owl:ObjectProperty;
        rdfs:isDefinedBy       sosa-sam:;
        rdfs:label             "feature has ultimate sample"@en;
        schema:domainIncludes  sosa:FeatureOfInterest;
        schema:rangeIncludes   sosa:SampleCollection , sosa:Sample;
        owl:inverseOf          sosa:isSampleOfUltimateFOI;
        skos:definition        "\n  relation from an ultimate FeatureOfInterest to a Sample or SampleCollection that is intended to be representative of it; i.e., the end of a chain of hasSample relations\n  "@en .

sosa:SamplingProcedure
        rdf:type          owl:Class;
        rdfs:isDefinedBy  sosa-sam:;
        rdfs:label        "Sampling Procedure"@en;
        rdfs:subClassOf   sosa:Procedure;
        rdfs:subClassOf   [ rdf:type           owl:Restriction;
                            owl:allValuesFrom  sosa:Sampler;
                            owl:onProperty     sosa:implementedBy
                          ];
        skos:definition   "\n  workflow, protocol, plan, algorithm, or computational method specifying how to make a Sampling\n\n  A Sampling Procedure is re-usable, and might be involved in many Samplings. \n  It explains the steps to be carried out to arrive at reproducible results.\n  "@en;
        skos:example      "\nspatial distribution of locations where to collect a sample (e.g., river segment)\ninstrument (or mode of use thereof) required to collect a sample (e.g., fish net, electric stunner)\nfield work instructions (e.g., dig four boreholes in each cardinal direction 2 metre way from the centre of the site; collect soil material from the 15-30 cm depth and mix it in a single bag)\n  "@en;
        skos:note         "\n[ISO 19156:2023] A SamplingProcedure shall be defined as the description of steps performed by a Sampler in order to extract a Sample from its sampledFeature in the frame of a Sampling.\n  "@en .

sosa:SamplingCollection
        rdf:type          owl:Class;
        rdfs:isDefinedBy  sosa-sam:;
        rdfs:label        "Sampling Collection"@en;
        rdfs:subClassOf   sosa:ExecutionCollection;
        rdfs:subClassOf   [ rdf:type           owl:Restriction;
                            owl:allValuesFrom  [ owl:unionOf  ( sosa:Sampling sosa:SamplingCollection )
                                               ];
                            owl:onProperty     sosa:hasMember
                          ];
        rdfs:subClassOf   [ rdf:type           owl:Restriction;
                            owl:allValuesFrom  [ owl:unionOf  ( sosa:Sampling sosa:SamplingCollection )
                                               ];
                            owl:onProperty     sosa:hasMember
                          ];
        rdfs:subClassOf   [ rdf:type           owl:Restriction;
                            owl:allValuesFrom  sosa:Sample;
                            owl:onProperty     sosa:hasResult
                          ];
        rdfs:subClassOf   [ rdf:type           owl:Restriction;
                            owl:allValuesFrom  sosa:FeatureOfInterest;
                            owl:onProperty     sosa:hasFeatureOfInterest
                          ];
        rdfs:subClassOf   [ rdf:type           owl:Restriction;
                            owl:allValuesFrom  sosa:SamplingProcedure;
                            owl:onProperty     sosa:usedProcedure
                          ];
        rdfs:subClassOf   [ rdf:type           owl:Restriction;
                            owl:allValuesFrom  sosa:Sampler;
                            owl:onProperty     sosa:madeBySampler
                          ];
        owl:disjointWith  sosa:SampleCollection , sosa:ObservationCollection , sosa:ActuationCollection;
        skos:definition   "\n  set of one or more Samplings or SamplingCollections; collections may be nested\n\n  All Sampling properties may appear in a Sampling Collection, including: \n  hasFeatureOfInterest , hasUltimateFeatureOfInterest , madeBySampler , usedProcedure , hasInputValue , startTime , phenomenonTime , resultTime , hasResult . \n  If they are present, the value of these properties summarize the values of the matching properties of the member samplings, where membership is either direct or transitive through one or more member sampling collections. \n  The following consistency rules apply with respect to the Sampling properties listed above: \n  \n  1. Where an individual Sampling Collection omits a property, a member Sampling (direct or transitive) MAY have any value for that property.\n\n  2. Where an individual Sampling Collection has a single value for a property, each member Sampling (direct or transitive) MUST have that same value for the property - i.e., the collection is homogeneous in that property.  That property MAY then be omitted in any member Sampling or Sampling Collection.\n\n  3. Where an individual Sampling Collection has more than one value for a property, each member Sampling (direct or transitive) MUST have a value for that property that matches one of the values for the property in the collection. \n  \n  4. Where an individual Sampling Collection has a value for a property that is a range or interval, each member Sampling (direct or transitive) MUST have a value for that property that matches or falls within that range or interval.\n\n  5. Where an individual Sampling Collection has more than one value for a property that is a range or interval, each member Sampling (direct or transitive) MUST have a value for that property that either matches or falls within one of those ranges or intervals.\n  "@en;
        skos:note         "The members of a collection do not necessarily share a common value for any property."@en .

sosa:Sampling  rdf:type   owl:Class;
        rdfs:isDefinedBy  sosa-sam:;
        rdfs:label        "Sampling"@en;
        rdfs:subClassOf   sosa:Execution;
        rdfs:subClassOf   [ rdf:type           owl:Restriction;
                            owl:allValuesFrom  sosa:Sample;
                            owl:onProperty     sosa:hasResult
                          ];
        rdfs:subClassOf   [ rdf:type           owl:Restriction;
                            owl:allValuesFrom  sosa:FeatureOfInterest;
                            owl:onProperty     sosa:hasFeatureOfInterest
                          ];
        rdfs:subClassOf   [ rdf:type           owl:Restriction;
                            owl:allValuesFrom  sosa:SamplingProcedure;
                            owl:onProperty     sosa:usedProcedure
                          ];
        rdfs:subClassOf   [ rdf:type           owl:Restriction;
                            owl:allValuesFrom  sosa:Sampler;
                            owl:onProperty     sosa:madeBySampler
                          ];
        skos:definition   "\n  act of carrying out a SamplingProcedure using a Sampler to create one or more Samples of a FeatureOfInterest\n  "@en;
        skos:example      "Crushing a rock sample in a ball mill."@en , "Digging a pit through a soil sequence."@en , "Dividing a field site into quadrants."@en , "Drawing blood from a patient."@en , "Drilling an observation well."@en , "Establishing a station for environmental monitoring."@en , "Registering an image of the landscape."@en , "Sieving a powder to separate the subset finer than 100-mesh."@en , "Selecting a subset of a population."@en , "Splitting a piece of drill-core to create two new samples."@en , "Taking a diamond-drill core from a rock outcrop."@en .

sosa:Sampler  rdf:type    owl:Class;
        rdfs:isDefinedBy  sosa-sam:;
        rdfs:label        "Sampler"@en;
        rdfs:subClassOf   sosa:System;
        rdfs:subClassOf   [ rdf:type           owl:Restriction;
                            owl:allValuesFrom  [ rdf:type     owl:Class;
                                                 owl:unionOf  ( sosa:Sampling sosa:SamplingCollection )
                                               ];
                            owl:onProperty     sosa:madeSampling
                          ];
        rdfs:subClassOf   [ rdf:type           owl:Restriction;
                            owl:allValuesFrom  sosa:SamplingProcedure;
                            owl:onProperty     sosa:implements
                          ];
        skos:definition   "\n  System that implements a SamplingProcedure to generate a Sample\n  "@en;
        skos:example      "A ball mill, diamond drill, hammer, hypodermic syringe and needle, image Sensor, or a soil auger can all act as Samplers. Sometimes, however, the distinction between the Sampler and the Sensor is not evident, if they are packaged as a unit."@en;
        skos:note         "A Sampler need not be a physical device."@en .

sosa:SampleCollection
        rdf:type          owl:Class;
        rdfs:isDefinedBy  sosa-sam:;
        rdfs:label        "Sample Collection"@en;
        rdfs:subClassOf   [ rdf:type           owl:Restriction;
                            owl:allValuesFrom  [ owl:unionOf  ( sosa:Sample sosa:SampleCollection )
                                               ];
                            owl:onProperty     sosa:hasMember
                          ];
        rdfs:subClassOf   [ rdf:type           owl:Restriction;
                            owl:allValuesFrom  [ rdf:type     owl:Class;
                                                 owl:unionOf  ( sosa:Sampling sosa:SamplingCollection )
                                               ];
                            owl:onProperty     sosa:isResultOf
                          ];
        rdfs:subClassOf   [ rdf:type           owl:Restriction;
                            owl:allValuesFrom  sosa:FeatureOfInterest;
                            owl:onProperty     sosa:isSampleOf
                          ];
        rdfs:subClassOf   [ rdf:type           owl:Restriction;
                            owl:allValuesFrom  sosa:Sample;
                            owl:onProperty     sosa:hasOriginalSample
                          ];
        rdfs:subClassOf   [ rdf:type           owl:Restriction;
                            owl:allValuesFrom  sosa:FeatureOfInterest;
                            owl:onProperty     sosa:isSampleOfUltimateFOI
                          ];
        rdfs:subClassOf   [ rdf:type           owl:Restriction;
                            owl:allValuesFrom  sosa:Sampler;
                            owl:onProperty     sosa:isResultOfMadeBySampler
                          ];
        rdfs:subClassOf   [ rdf:type           owl:Restriction;
                            owl:allValuesFrom  sosa:SamplingProcedure;
                            owl:onProperty     sosa:isResultOfUsedProcedure
                          ];
        rdfs:subClassOf   [ rdf:type           owl:Restriction;
                            owl:allValuesFrom  [ owl:unionOf  ( sosa:Sample sosa:SampleCollection )
                                               ];
                            owl:onProperty     sosa:hasMember
                          ];
        owl:disjointWith  sosa:ActuationCollection , sosa:ObservationCollection , sosa:SamplingCollection;
        skos:definition   "\n  set of one or more Samples or SampleCollections; collections may be nested.\n\n  All Sample properties may appear in a Sample Collection, including: \n  hasOriginalSample , isSampleOfUltimateFOI , isSampleOf , isResultOfUsedProcedure , isResultOfMadeBySampler . \n  If they are present, the value of these properties summarize the values of the matching properties of the member samples, where membership is either direct or transitive through one or more member sample collections. \n\n  The following consistency rules apply with respect to the Sample properties listed above: \n  \n  1. Where an individual Sample Collection omits a property, a member Sample (direct or transitive) MAY have any value for that property.\n\n  2. Where an individual Sample Collection has a single value for a property, each member Sample (direct or transitive) MUST have that same value for the property - i.e., the collection is homogeneous in that property.  That property MAY be omitted in any member Sample or Sample Collection.\n\n  3. Where an individual Sample Collection has more than one value for a property, each member Sample (direct or transitive) MUST have a value for that property that matches one of the values for the property in the collection. \n  \n  4. Where an individual Sample Collection has a value for a property that is a range or interval, each member Sample (direct or transitive) MUST have a value for that property that either matches or falls within that range or interval.\n\n  5. Where an individual Sample Collection has more than one value for a property that is a range or interval, each member Sample (direct or transitive) MUST have a value for that property that either matches or falls within one of those ranges or intervals.\n  "@en;
        skos:note         "\n  The members of a collection do not necessarily share a common value for any property. \n  " .

sosa:StatisticalSample
        rdf:type          owl:Class;
        rdfs:isDefinedBy  sosa-sam:;
        rdfs:label        "Statistical Sample"@en;
        rdfs:subClassOf   sosa:Sample;
        skos:definition   "\n  subset of a FeatureOfInterest defined by the statistical process used to create it\n  "@en;
        skos:example      "The male or female subset of a population."@en;
        skos:note         "StatisticalSamples usually apply to populations or other sets, of which a certain subset may be of specific interest."@en .

sosa:SpatialSample  rdf:type  owl:Class;
        rdfs:isDefinedBy  sosa-sam:;
        rdfs:label        "Spatial Sample"@en;
        rdfs:subClassOf   sosa:Sample;
        skos:definition   "\n  subset of a FeatureOfInterest defined by its location and shape in space\n  \n  When observations are made to estimate properties of a geospatial feature, particularly where the value of a property varies within the scope of the feature, a SpatialSample is used.\n  "@en;
        skos:example      "Some common names for spatial samples include: borehole, flightline, interval, lidar cloud, map horizon, microscope slide, mine level, mine, observation well, profile,  quadrat, scene, section, ship track, spot, station, swath, trajectory, traverse, etc..."@en;
        skos:note         "Depending on accessibility and on the nature of the expected property variation, a SpatialSample may extend in one, two or three spatial dimensions."@en .

sosa:MaterialSample  rdf:type  owl:Class;
        rdfs:isDefinedBy  sosa-sam:;
        rdfs:label        "Material Sample"@en;
        rdfs:subClassOf   sosa:Sample;
        skos:definition   "\n  subset of a FeatureOfInterest that is physical (i.e., tangible)\n  "@en;
        skos:example      "A piece of rock, a blood sample, a water sample, etc."@en;
        skos:note         "MaterialSamples may be destroyed in connexion with the observation act or a subsequent preparation step."@en , "MaterialSamples that are curated and preserved are sometimes known as 'specimens'."@en .

sosa-sam:  rdf:type          owl:Ontology;
        dcterms:created      "2024-02-02"^^xsd:date;
        dcterms:creator      [ rdf:type   foaf:Agent;
                               foaf:name  "W3C/OGC Spatial Data on the Web Working Group"@en
                             ];
        dcterms:description  "Sampling classes and properties for the SSN Ontology."@en;
        dcterms:license      <http://www.opengeospatial.org/ogc/Software> , <http://www.w3.org/Consortium/Legal/2015/copyright-software-and-document>;
        dcterms:rights       "Copyright 2025 W3C/OGC.";
        dcterms:title        "Sensor, Observation, Sample, and Actuator (SOSA) Ontology - actuation module"@en;
        owl:imports          sosa-common: .

sp:hadProcedure  rdf:type   owl:ObjectProperty;
        rdfs:range          sosa:Procedure;
        rdfs:subPropertyOf  prov:hadPlan .

sp:executionAssociation
        rdf:type            owl:ObjectProperty;
        rdfs:domain         sosa:Execution;
        rdfs:subPropertyOf  prov:qualifiedAssociation .

sosa:prov  rdf:type       owl:Ontology;
        rdfs:comment      "Alignment of the the W3C/OGC SOSA Ontology with the W3C PROV-O Ontology"@en;
        rdfs:label        "Alignment of SOSA with PROV-O"@en;
        dcterms:created   "2016-12-14"^^xsd:date;
        dcterms:creator   "Simon J D Cox";
        dcterms:creator   [ rdf:type   foaf:Agent;
                            foaf:name  "W3C/OGC Spatial Data on the Web Working Group"@en
                          ];
        dcterms:license   <http://www.w3.org/Consortium/Legal/2015/copyright-software-and-document> , <http://www.opengeospatial.org/ogc/Software>;
        dcterms:modified  "2025-10-23"^^xsd:date;
        dcterms:rights    "Copyright 2017, 2025 W3C/OGC.";
        owl:imports       sosa: , <http://www.w3.org/ns/prov-o#> .

sosa:isSampleOf  rdf:type      owl:ObjectProperty;
        rdfs:isDefinedBy       sosa-sam:;
        rdfs:label             "is sample of"@en;
        rdfs:subPropertyOf     prov:wasDerivedFrom;
        schema:domainIncludes  sosa:SampleCollection , sosa:Sample;
        schema:rangeIncludes   sosa:FeatureOfInterest;
        owl:inverseOf          sosa:hasSample;
        skos:definition        "\n  relation from a Sample or SampleCollection to the FeatureOfInterest that it is intended to represent\n  "@en .

sosa:Sample  rdf:type     owl:Class;
        rdfs:isDefinedBy  sosa-sam:;
        rdfs:label        "Sample"@en;
        rdfs:subClassOf   prov:Entity;
        rdfs:subClassOf   [ rdf:type           owl:Restriction;
                            owl:allValuesFrom  sosa:SamplingProcedure;
                            owl:onProperty     sosa:isResultOfUsedProcedure
                          ];
        rdfs:subClassOf   [ rdf:type           owl:Restriction;
                            owl:allValuesFrom  sosa:Sampler;
                            owl:onProperty     sosa:isResultOfMadeBySampler
                          ];
        rdfs:subClassOf   [ rdf:type           owl:Restriction;
                            owl:allValuesFrom  sosa:FeatureOfInterest;
                            owl:onProperty     sosa:isSampleOfUltimateFOI
                          ];
        rdfs:subClassOf   [ rdf:type           owl:Restriction;
                            owl:allValuesFrom  sosa:Sample;
                            owl:onProperty     sosa:hasOriginalSample
                          ];
        rdfs:subClassOf   [ rdf:type            owl:Restriction;
                            owl:minCardinality  "1"^^xsd:nonNegativeInteger;
                            owl:onProperty      sosa:isSampleOf
                          ];
        rdfs:subClassOf   [ rdf:type           owl:Restriction;
                            owl:allValuesFrom  sosa:FeatureOfInterest;
                            owl:onProperty     sosa:isSampleOf
                          ];
        rdfs:subClassOf   [ rdf:type           owl:Restriction;
                            owl:allValuesFrom  [ rdf:type     owl:Class;
                                                 owl:unionOf  ( sosa:Sampling sosa:SamplingCollection )
                                               ];
                            owl:onProperty     sosa:isResultOf
                          ];
        skos:definition   "\n  piece or subset that is intended to be representative of a FeatureOfInterest\n  "@en;
        skos:example      "A statistical sample is often designed to be characteristic of an entire population, so that observations can be made regarding the sample that provide a good estimate of the properties of the population."@en , "A 'station' is a spatial sample, in the form of an identifiable locality where a sensor system or Procedure may be deployed and an observation made. In the context of the observation model, it connotes the 'world in the vicinity of the station', so the observed properties relate to the physical medium at the station, and not to any physical artifact such as a mooring, buoy, benchmark, monument, well, etc."@en;
        skos:note         "\n  Samples are typically subsets or extracts from an entity or feature.\n  Every sample is expected to (eventually) be the feature of interest of an Observation. \n  \n  Samples are used in situations where observations cannot be made directly on the ultimate feature of interest, either because the entire feature cannot be observed, or because it is more convenient to use a proxy.\n  Samples are thus artifacts of an observational strategy, and have no significant function outside of their role in the observation process. \n  The characteristics of the samples themselves are of little interest, except perhaps to the manager of a sampling campaign.\n\n  A Sample is intended to sample some FatureOfInterest, so there is an expectation of at least one isSampleOf property. \n  However, in some cases the identity, and even the exact type, of the sampled feature may not be known when observations are made using the sample.\n\n  Physical samples are sometimes known as 'specimens'. A transient sample, such as a ships-track or flight-line, might be identified and described, but is unlikely to be revisited exactly.\n  "@en .

sosa:wasOriginatedBy  rdf:type  owl:ObjectProperty;
        rdfs:isDefinedBy       sosa-obs:;
        rdfs:label             "was originated by"@en;
        schema:domainIncludes  sosa:ObservationCollection , sosa:Observation;
        schema:rangeIncludes   sosa:Stimulus;
        owl:inverseOf          sosa:originated;
        skos:definition        "\n  relation from an Observation to the Stimulus that originated it\n  "@en .

sosa:wasObservedBy  rdf:type   owl:ObjectProperty;
        rdfs:isDefinedBy       sosa-obs:;
        rdfs:label             "was observed by"@en;
        schema:domainIncludes  sosa:Property;
        schema:rangeIncludes   sosa:ObservationCollection , sosa:Observation;
        owl:inverseOf          sosa:observedProperty;
        skos:definition        "\n  relation from a Property to an Observation that observed it\n  "@en .

sosa:resultQuality  rdf:type   owl:ObjectProperty;
        rdfs:isDefinedBy       sosa-obs:;
        rdfs:label             "observation result quality";
        schema:domainIncludes  sosa:ObservationCollection , sosa:Observation;
        owl:inverseOf          sosa:qualityOf;
        skos:definition        "\n  relation from an Observation or ObservationCollection to some information pertaining to the quality of the result\n  "@en;
        skos:note              "dqv:hasQualityMeasurement from the Data Quality Vocabulary is equivalent" , "\n  The quality of a result can be assessed following the procedures in the ISO 19157 series.\n  ";
        skos:scopeNote         "\n  This instance-specific description complements the description of the observation Procedure, which provides information concerning the quality of all observations using this procedure. Multiple measures can be provided.\n  "@en .

sosa:relatedObservation
        rdf:type               owl:ObjectProperty;
        rdfs:isDefinedBy       sosa-obs:;
        rdfs:label             "related observation"@en;
        schema:domainIncludes  sosa:SamplingCollection , sosa:Sampling , sosa:ActuationCollection , sosa:Actuation , sosa:ExecutionCollection , sosa:Execution;
        schema:rangeIncludes   sosa:ObservationCollection , sosa:Observation;
        owl:inverseOf          sosa:observationRelatedTo;
        skos:definition        "\n  relation from an Execution or ExecutionCollection to an Observation or ObservationCollection\n  "@en;
        skos:scopeNote         "This general relationship complements the specific predicates inbound to Observation. It is particularly useful to relate Observations (and collections) to other Executions (and collections)" .

sosa:qualityOf  rdf:type      owl:ObjectProperty;
        rdfs:isDefinedBy      sosa-obs:;
        rdfs:label            "quality of";
        schema:rangeIncludes  sosa:ObservationCollection , sosa:Observation;
        owl:inverseOf         sosa:resultQuality;
        skos:definition       "\n  link from a quality description to an Observation or ObservationCollection that it relates to\n  "@en .

sosa:originated  rdf:type      owl:ObjectProperty;
        rdfs:isDefinedBy       sosa-obs:;
        rdfs:label             "originated"@en;
        schema:domainIncludes  sosa:Stimulus;
        schema:rangeIncludes   sosa:Observation;
        owl:inverseOf          sosa:wasOriginatedBy;
        skos:definition        "\n  relation from a Stimulus to an Observation that was originated by it\n  "@en .

sosa:observes  rdf:type        owl:ObjectProperty;
        rdfs:isDefinedBy       sosa-obs:;
        rdfs:label             "observes"@en;
        rdfs:subPropertyOf     sosa:forProperty;
        schema:domainIncludes  sosa:Sensor;
        schema:rangeIncludes   sosa:Property;
        owl:inverseOf          sosa:isObservedBy;
        skos:definition        "\n  relation from a Sensor to a Property that it is capable of sensing\n  "@en .

sosa:observedProperty
        rdf:type               owl:ObjectProperty;
        rdfs:isDefinedBy       sosa-obs:;
        rdfs:label             "observed property"@en;
        schema:domainIncludes  sosa:ObservationCollection , sosa:Observation;
        schema:rangeIncludes   sosa:Property;
        owl:inverseOf          sosa:wasObservedBy;
        skos:definition        "\n  relation from an Observation or ObservationCollection to the property that was observed\n  "@en;
        skos:note              "\n  'observed property' covers the concepts referred to in [VIM] as 'measurand' (quantitative values) and 'examinand' (categorical and nominal values â€” [VIM4]), as well as complex and structured properties whose values may be represented as lists, vectors, arrays, rasters, geometries, etc. More specific terms are used in other contexts for related concepts, such as 'analyte' (chemistry) and 'determinand' (water quality).\n  "@en .

sosa:observationRelatedTo
        rdf:type               owl:ObjectProperty;
        rdfs:isDefinedBy       sosa-obs:;
        rdfs:label             "observation related to"@en;
        schema:domainIncludes  sosa:ObservationCollection , sosa:Observation;
        schema:rangeIncludes   sosa:SamplingCollection , sosa:Sampling , sosa:ActuationCollection , sosa:Actuation , sosa:ExecutionCollection , sosa:Execution;
        owl:inverseOf          sosa:relatedObservation;
        skos:definition        "\n  relation from an Observation or ObservationCollection to another Execution or ExecutionCollection\n  "@en;
        skos:scopeNote         "This general relationship complements the specific predicates outbound from Observation. It is particularly useful to relate Observations (and collections) to other Executions (and collections)" .

sosa:madeObservation  rdf:type  owl:ObjectProperty;
        rdfs:isDefinedBy       sosa-obs:;
        rdfs:label             "made observation"@en;
        rdfs:subPropertyOf     sosa:madeExecution;
        schema:domainIncludes  sosa:Sensor;
        schema:rangeIncludes   sosa:ObservationCollection , sosa:Observation;
        owl:inverseOf          sosa:madeBySensor;
        skos:definition        "\n  relation from a Sensor to an Observation or ObservationCollection it has made\n  "@en .

sosa:madeBySensor  rdf:type    owl:ObjectProperty;
        rdfs:isDefinedBy       sosa-obs:;
        rdfs:label             "made by sensor or observer"@en;
        rdfs:subPropertyOf     sosa:madeBySystem;
        schema:domainIncludes  sosa:ObservationCollection , sosa:Observation;
        schema:rangeIncludes   sosa:Sensor;
        owl:inverseOf          sosa:madeObservation;
        skos:definition        "\n  relation from an Observation or ObservationCollection to the Sensor that made it\n  "@en .

sosa:isProxyFor  rdf:type      owl:ObjectProperty;
        rdfs:isDefinedBy       sosa-obs:;
        rdfs:label             "is proxy for"@en;
        schema:domainIncludes  sosa:Stimulus;
        schema:rangeIncludes   sosa:Property;
        owl:inverseOf          sosa:hasProxy;
        skos:definition        "\n  relation from a Stimulus to the Property for which it is serving as a proxy\n  "@en;
        skos:example           "For example, the expansion of quicksilver is a stimulus that serves as a proxy for some temperature property. An increase or decrease in the velocity of spinning cups on a wind sensor is serving as a proxy for the wind speed."@en .

sosa:isObservedBy  rdf:type    owl:ObjectProperty;
        rdfs:isDefinedBy       sosa-obs:;
        rdfs:label             "is observed by"@en;
        schema:domainIncludes  sosa:Property;
        schema:rangeIncludes   sosa:Sensor;
        owl:inverseOf          sosa:observes;
        skos:definition        "\n  relation from a Property to a Sensor that is able to observe it\n  "@en .

sosa:isDetectedBy  rdf:type    owl:ObjectProperty;
        rdfs:isDefinedBy       sosa-obs:;
        rdfs:label             "is detected by"@en;
        schema:domainIncludes  sosa:Stimulus;
        schema:rangeIncludes   sosa:Sensor;
        owl:inverseOf          sosa:detects;
        skos:definition        "\n  relation from a Stimulus to a Sensor that may detect it\n\n  The Stimulus itself will be serving as a proxy for some Property.\n  "@en .

sosa:hasProxy  rdf:type        owl:ObjectProperty;
        rdfs:isDefinedBy       sosa-obs:;
        rdfs:label             "has proxy"@en;
        schema:domainIncludes  sosa:Property;
        schema:rangeIncludes   sosa:Stimulus;
        owl:inverseOf          sosa:isProxyFor;
        skos:definition        "\n  relation from an Property to a Stimulus that serves as its proxy\n  "@en;
        skos:example           "\nFor example, the expansion of mercury is a Stimulus that serves as a proxy for some temperature Property.\nAn increase or decrease in the velocity of spinning cups on a wind Sensor is serving as a proxy for the wind speed.\n  "@en .

sosa:detects  rdf:type         owl:ObjectProperty;
        rdfs:isDefinedBy       sosa-obs:;
        rdfs:label             "detects"@en;
        schema:domainIncludes  sosa:Sensor;
        schema:rangeIncludes   sosa:Stimulus;
        owl:inverseOf          sosa:isDetectedBy;
        skos:definition        "\n  relation from a Sensor to the Stimulus that it detects\n\n  The Stimulus itself will be serving as a proxy for some Property.\n  "@en .

sosa:Stimulus  rdf:type   owl:Class;
        rdfs:isDefinedBy  sosa-obs:;
        rdfs:label        "Stimulus"@en;
        rdfs:subClassOf   [ rdf:type           owl:Restriction;
                            owl:allValuesFrom  sosa:Property;
                            owl:onProperty     sosa:isProxyFor
                          ];
        rdfs:subClassOf   [ rdf:type           owl:Restriction;
                            owl:allValuesFrom  sosa:Sensor;
                            owl:onProperty     sosa:isDetectedBy
                          ];
        rdfs:subClassOf   [ rdf:type           owl:Restriction;
                            owl:allValuesFrom  [ rdf:type     owl:Class;
                                                 owl:unionOf  ( sosa:Observation sosa:ObservationCollection )
                                               ];
                            owl:onProperty     sosa:originated
                          ];
        skos:definition   "\n  event in the real world that triggers a Sensor\n  "@en;
        skos:note         "The properties associated to the Stimulus may be different to the eventual observed Property. It is the event, not the object, that triggers the Sensor."@en .

sosa:Sensor  rdf:type     owl:Class;
        rdfs:isDefinedBy  sosa-obs:;
        rdfs:label        "Sensor or Observer"@en;
        rdfs:subClassOf   sosa:System;
        rdfs:subClassOf   [ rdf:type           owl:Restriction;
                            owl:allValuesFrom  [ rdf:type     owl:Class;
                                                 owl:unionOf  ( sosa:Observation sosa:ObservationCollection )
                                               ];
                            owl:onProperty     sosa:madeObservation
                          ];
        rdfs:subClassOf   [ rdf:type           owl:Restriction;
                            owl:allValuesFrom  sosa:ObservingProcedure;
                            owl:onProperty     sosa:implements
                          ];
        rdfs:subClassOf   [ rdf:type           owl:Restriction;
                            owl:allValuesFrom  sosa:Property;
                            owl:onProperty     sosa:observes
                          ];
        rdfs:subClassOf   [ rdf:type           owl:Restriction;
                            owl:allValuesFrom  sosa:Stimulus;
                            owl:onProperty     sosa:detects
                          ];
        skos:altLabel     "Observer"@en;
        skos:definition   "\n  System that implements an ObservingProcedure to determine the value of an observable Property\n\n  This may be a device, a piece of infrastructure, an agent (including humans), or software (simulation).\n\n  A Sensor responds to a stimulus, e.g., a change in the environment, or input data composed from the results of prior Observations.\n  "@en;
        skos:example      "Accelerometers, gyroscopes, barometers, magnetometers, and so forth are Sensors that are typically mounted on a modern smartphone (which acts as Host or Platform). Other examples of Sensors include the human eyes."@en;
        skos:note         "The UML class 'Observer' from ISO 19156:2023 is implemented in SOSA by the OWL/RDFS class 'Sensor'. The class name 'Sensor' is preferred for backward compatibility with existing SOSA deployments. ";
        skos:prefLabel    "Sensor"@en .

sosa:ObservingProcedure
        rdf:type          owl:Class;
        rdfs:isDefinedBy  sosa-obs:;
        rdfs:label        "Observing Procedure"@en;
        rdfs:subClassOf   sosa:Procedure;
        rdfs:subClassOf   [ rdf:type           owl:Restriction;
                            owl:allValuesFrom  sosa:Sensor;
                            owl:onProperty     sosa:implementedBy
                          ];
        skos:definition   "\n  workflow, protocol, plan, algorithm, or computational method specifying how to make an Observation\n\n  An Observing Procedure is re-usable, and might be involved in many Observations. \n  It explains the steps to be carried out to arrive at reproducible results.\n  "@en;
        skos:example      "A workflow, protocol, plan, algorithm, or computational method specifying how to make an observation; the description of the process used by an observer. This could be a chemical analysis method, a protocol for measuring an object, or even a checklist used by a human observer during a biodiversity campaign. The Procedure could further describe the algorithms behind simulators or models used to generate a result from other inputs."@en;
        skos:note         "[ISO 19156:2023] An ObservingProcedure shall be defined as the description of steps performed in order to determine the value of an observableProperty by an Observer."@en .

sosa:ObservationCollection
        rdf:type          owl:Class;
        rdfs:isDefinedBy  sosa-obs:;
        rdfs:label        "Observation Collection"@en;
        rdfs:subClassOf   sosa:ExecutionCollection;
        rdfs:subClassOf   [ rdf:type           owl:Restriction;
                            owl:allValuesFrom  sosa:FeatureOfInterest;
                            owl:onProperty     sosa:hasUltimateFeatureOfInterest
                          ];
        rdfs:subClassOf   [ rdf:type           owl:Restriction;
                            owl:allValuesFrom  sosa:Sensor;
                            owl:onProperty     sosa:madeBySensor
                          ];
        rdfs:subClassOf   [ rdf:type           owl:Restriction;
                            owl:allValuesFrom  sosa:Property;
                            owl:onProperty     sosa:observedProperty
                          ];
        rdfs:subClassOf   [ rdf:type           owl:Restriction;
                            owl:allValuesFrom  sosa:ObservingProcedure;
                            owl:onProperty     sosa:usedProcedure
                          ];
        rdfs:subClassOf   [ rdf:type           owl:Restriction;
                            owl:allValuesFrom  [ owl:unionOf  ( sosa:Observation sosa:ObservationCollection )
                                               ];
                            owl:onProperty     sosa:hasMember
                          ];
        owl:disjointWith  sosa:ActuationCollection , sosa:SampleCollection , sosa:SamplingCollection;
        skos:definition   "\n  set of one or more Observations or ObservationCollections; collections may be nested\n\n  All Observation properties may appear in an Observation Collection, including: \n  hasFeatureOfInterest , hasUltimateFeatureOfInterest , usedProcedure , madeBySensor , observedProperty , phenomenonTime , startTime, resultTime , hasResult , hasSimpleResult : \n  If they are present, the value of these properties summarize the values of the matching properties of the member observations, where membership is either direct or transitive through one or more member observation collections. \n  The following consistency rules apply with respect to the Observation properties listed above: \n  \n  1. Where an individual Observation Collection omits a property, a member Observation (direct or transitive) MAY have any value for that property.\n\n  2. Where an individual Observation Collection has a single value for a property, each member Observation(direct or transitive) MUST have that same value for the property - i.e., the collection is homogeneous in that property.  That property MAY then be omitted in any member Observation or Observation Collection.\n\n  3. Where an individual Observation Collection has more than one value for a property, each member Observation (direct or transitive) MUST have a value for that property that matches one of the values for the property in the collection. \n  \n  4. Where an individual Observation Collection has a value for a property that is a range or interval, each member Observation (direct or transitive) MUST have a value for that property that matches or falls within that range or interval.\n\n  5. Where an individual Observation Collection has more than one value for a property that is a range or interval, each member Observation (direct or transitive) MUST have a value for that property that either matches or falls within one of those ranges or intervals.\n  "@en;
        skos:note         "The members of a collection do not necessarily share a common value for any property. "@en , "The results of collections of observations are often packaged in a 'data cube' whose axes define the\n      range of properties of the set of observations." , "An instance of ObservationCollection represents a container for a set of data derived from observations.\n  This broadly corresponds with the class Dataset from DCAT."@en .

sosa:Observation  rdf:type  owl:Class;
        rdfs:isDefinedBy  sosa-obs:;
        rdfs:label        "Observation"@en;
        rdfs:subClassOf   sosa:Execution;
        rdfs:subClassOf   [ rdf:type           owl:Restriction;
                            owl:allValuesFrom  sosa:Stimulus;
                            owl:onProperty     sosa:wasOriginatedBy
                          ];
        rdfs:subClassOf   [ rdf:type           owl:Restriction;
                            owl:allValuesFrom  sosa:Property;
                            owl:onProperty     sosa:observedProperty
                          ];
        rdfs:subClassOf   [ rdf:type           owl:Restriction;
                            owl:allValuesFrom  sosa:FeatureOfInterest;
                            owl:onProperty     sosa:hasUltimateFeatureOfInterest
                          ];
        rdfs:subClassOf   [ rdf:type           owl:Restriction;
                            owl:allValuesFrom  sosa:FeatureOfInterest;
                            owl:onProperty     sosa:hasFeatureOfInterest
                          ];
        rdfs:subClassOf   [ rdf:type           owl:Restriction;
                            owl:allValuesFrom  sosa:ObservingProcedure;
                            owl:onProperty     sosa:usedProcedure
                          ];
        rdfs:subClassOf   [ rdf:type           owl:Restriction;
                            owl:allValuesFrom  sosa:Sensor;
                            owl:onProperty     sosa:madeBySensor
                          ];
        skos:definition   "\n  act of carrying out an ObservingProcedure using a Sensor to estimate or calculate a value of an observable Property of a FeatureOfInterest\n  "@en;
        skos:example      "The activity of estimating the intensity of an Earthquake using the Mercalli intensity scale is an Observation as is measuring the moment magnitude, i.e., the energy released by said earthquake."@en;
        skos:note         "\n  When the feature of interest cannot be observed directly, a sample of it might be used in Observations as a proxy for it. In such case, the Sample is the proximate Feature of Interest of the Observation, while the (ultimate) Feature of Interest of the act of Sampling (i.e., the entity that the Sample is ultimately 'isSampleOf') is the ultimate Feature of Interest of the Observation.\n  ";
        skos:scopeNote    "\n  An Observation primarily concerns a single Property of a single FeatureOfInterest. \n  Observations of multiple properties, or other combinations of Observations, may be described in an ObservationCollection. \n  \n  Alternatively, applications may choose to encapsulate complexity by defining a complex property with multiple individual components, and a corresponding complex result (e.g., a vector). \n  This approach is not prohibited by the SSN Ontology, but the details are beyond the scope of SSN.\n  "@en .

sosa-obs:  rdf:type          owl:Ontology;
        dcterms:created      "2024-02-02"^^xsd:date;
        dcterms:creator      [ rdf:type   foaf:Agent;
                               foaf:name  "W3C/OGC Spatial Data on the Web Working Group"@en
                             ];
        dcterms:description  "Observation classes and properties for the SSN Ontology."@en;
        dcterms:license      <http://www.opengeospatial.org/ogc/Software> , <http://www.w3.org/Consortium/Legal/2015/copyright-software-and-document>;
        dcterms:rights       "Copyright 2025 W3C/OGC.";
        dcterms:title        "Sensor, Observation, Sample, and Actuator (SOSA) Ontology - actuation module"@en;
        owl:imports          sosa-common: .

sosa:systemDeployment
        rdf:type               owl:ObjectProperty;
        rdfs:isDefinedBy       sosa-common:;
        rdfs:label             "system deployment"@en;
        rdfs:subPropertyOf     sosa:hasDeployment;
        schema:domainIncludes  sosa:System;
        schema:rangeIncludes   sosa:Deployment;
        owl:inverseOf          sosa:deployedSystem;
        skos:definition        "\n  relation from a System to a Deployment\n  "@en .

sosa:madeExecution  rdf:type   owl:ObjectProperty;
        rdfs:isDefinedBy       sosa-common:;
        rdfs:label             "made execution"@en;
        schema:domainIncludes  sosa:System , sosa:Actuator , sosa:Sensor , sosa:Sampler;
        schema:rangeIncludes   sosa:SamplingCollection , sosa:Sampling , sosa:Execution , sosa:ExecutionCollection , sosa:Actuation , sosa:ActuationCollection , sosa:Observation , sosa:ObservationCollection;
        owl:inverseOf          sosa:madeBySystem;
        skos:definition        "\n  relation from a System to an Execution or ExecutionCollection that it has made\n  "@en;
        skos:scopeNote         "\n  madeExecution generalizes the madeActuation, madeObservation, and madeSampling properties. \n  It is included in the ontology to support the definition of a common pattern for executions and their properties. \n\n  madeExecution MUST be considered to be abstract, so SHOULD NOT appear in data instances. \n  Applications can use concrete sub-properties of madeExecution.\n  "@en .

sosa:madeBySystem  rdf:type    owl:ObjectProperty;
        rdfs:isDefinedBy       sosa-common:;
        rdfs:label             "made by system"@en;
        rdfs:subPropertyOf     prov:wasAssociatedWith;
        schema:domainIncludes  sosa:Execution , sosa:ExecutionCollection , sosa:Actuation , sosa:ActuationCollection , sosa:Observation , sosa:ObservationCollection , sosa:Sampling , sosa:SamplingCollection;
        schema:rangeIncludes   sosa:Sampler , sosa:Sensor , sosa:Actuator , sosa:System;
        owl:inverseOf          sosa:madeExecution;
        skos:definition        "\n  relation from an Execution to the System that made it\n  "@en;
        skos:scopeNote         "\n  madeBySystem generalizes the madeByActuator, madeBySensor, and madeBySampler properties. \n  It is included in the ontology to support the definition of a common pattern for executions and their properties. \n\n  madeBySystem MUST be considered to be abstract, so SHOULD NOT appear in data instances. \n  Applications can use concrete sub-properties of madeBySystem.\n  "@en .

sosa:Result  rdf:type     owl:Class;
        rdfs:isDefinedBy  sosa-common:;
        rdfs:label        "Result"@en;
        rdfs:subClassOf   [ rdf:type            owl:Restriction;
                            owl:onProperty      sosa:isResultOf;
                            owl:someValuesFrom  sosa:Execution
                          ];
        owl:deprecated    true;
        skos:definition   "\n  outcome of an Observation, Actuation, or act of Sampling. \n  \n  To store an observation's simple result value one can use the hasSimpleResult property.\n  "@en;
        skos:example      "The value 20 as the height of a certain tree together with the unit, e.g., Meter."@en .

sosa:ExecutionCollection
        rdf:type          owl:Class;
        rdfs:isDefinedBy  sosa-common:;
        rdfs:label        "Execution Collection"@en;
        rdfs:subClassOf   [ rdf:type           owl:Restriction;
                            owl:allValuesFrom  [ owl:unionOf  ( sosa:Execution sosa:ExecutionCollection )
                                               ];
                            owl:onProperty     sosa:hasMember
                          ];
        rdfs:subClassOf   [ rdf:type           owl:Restriction;
                            owl:allValuesFrom  sosa:FeatureOfInterest;
                            owl:onProperty     sosa:hasUltimateFeatureOfInterest
                          ];
        rdfs:subClassOf   [ rdf:type           owl:Restriction;
                            owl:allValuesFrom  sosa:FeatureOfInterest;
                            owl:onProperty     sosa:hasFeatureOfInterest
                          ];
        rdfs:subClassOf   [ rdf:type           owl:Restriction;
                            owl:allValuesFrom  sosa:Procedure;
                            owl:onProperty     sosa:usedProcedure
                          ];
        rdfs:subClassOf   [ rdf:type           owl:Restriction;
                            owl:allValuesFrom  sosa:System;
                            owl:onProperty     sosa:madeBySystem
                          ];
        skos:definition   "\n  set of one or more Executions or ExecutionCollections; collections may be nested\n\n  All Execution properties may appear in an Execution Collection, including: \n  hasFeatureOfInterest , usedProcedure , madeBySystem , endTime, resultTime , startTime . \n  If they are present, the value of these properties summarize the values of the matching properties of the member Executions, where membership is either direct or transitive through one or more member execution collections.\n\n  The following consistency rules apply with respect to the execution properties listed above: \n  \n  1. Where an individual Execution Collection omits a property, a member Execution (direct or transitive) MAY have any value for that property.\n\n  2. Where an individual Execution Collection has a single value for a property, each member Execution (direct or transitive) MUST have that same value for the property - i.e., the collection is homogeneous in that property.  That property MAY then be omitted in any member Execution or Execution Collection.\n\n  3. Where an individual Execution Collection has more than one value for a property, each member Execution (direct or transitive) MUST have a value for that property that matches one of the values for the property in the collection. \n  \n  4. Where an individual Execution Collection has a value for a property that is a range or interval, each member Execution (direct or transitive) MUST have a value for that property that matches or falls within that range or interval.\n\n  5. Where an individual Execution Collection has more than one value for a property that is a range or interval, each member Execution (direct or transitive) MUST have a value for that property that either matches or falls within one of those ranges or intervals.\n  "@en;
        skos:note         "The members of a collection do not necessarily share a common value for any property. "@en;
        skos:scopeNote    "\n  Execution Collection generalizes the Actuation Collection, Observation Collection, and Sampling Collection classes. \n  It is included in the ontology to support the definition of a common pattern for executions and their properties. \n\n  Execution Collection MUST be considered to be abstract, so any individual Execution Collection SHOULD be declared to be an instance of one of the concrete sub-classes, and not of the Execution Collection class.\n  "@en .

sosa:isProcedureFor  rdf:type  owl:ObjectProperty;
        rdfs:isDefinedBy       sosa-common:;
        rdfs:label             "is procedure for"@en;
        rdfs:subPropertyOf     sosa:forProperty;
        schema:domainIncludes  sosa:Procedure;
        schema:rangeIncludes   sosa:Property;
        owl:inverseOf          sosa:hasProcedure;
        skos:definition        "\n  relation from a Procedure to a Property that it can observe or act on\n  "@en .

sosa-common:  rdf:type       owl:Ontology;
        dcterms:created      "2024-02-02"^^xsd:date;
        dcterms:creator      [ rdf:type   foaf:Agent;
                               foaf:name  "W3C/OGC Spatial Data on the Web Working Group"@en
                             ];
        dcterms:description  "Core classes and properties for the SSN Ontology."@en;
        dcterms:license      <http://www.opengeospatial.org/ogc/Software> , <http://www.w3.org/Consortium/Legal/2015/copyright-software-and-document>;
        dcterms:rights       "Copyright 2025 W3C/OGC.";
        dcterms:title        "Sensor, Observation, Sample, and Actuator (SOSA) Ontology - core module"@en .

sosa:deployedOnPlatform
        rdf:type               owl:ObjectProperty;
        rdfs:isDefinedBy       sosa-common:;
        rdfs:label             "deployed on platform"@en;
        rdfs:subPropertyOf     sosa:deployedAsset;
        schema:domainIncludes  sosa:Deployment;
        schema:rangeIncludes   sosa:Platform;
        owl:inverseOf          sosa:inDeployment;
        skos:definition        "\n  relation from a Deployment to a Platform on which Systems are hosted\n  "@en .

sosa:deployedSystem  rdf:type  owl:ObjectProperty;
        rdfs:isDefinedBy       sosa-common:;
        rdfs:label             "deployed system"@en;
        rdfs:subPropertyOf     sosa:deployedAsset;
        schema:domainIncludes  sosa:Deployment;
        schema:rangeIncludes   sosa:Sampler , sosa:Sensor , sosa:System , sosa:Actuator;
        owl:inverseOf          sosa:systemDeployment;
        owl:inverseOf          [ rdfs:subPropertyOf
                          sosa:hasDeployment ];
        skos:definition        "\n  relation from a Deployment to a deployed System\n  "@en .

sosa:deployedAsset  rdf:type   owl:ObjectProperty;
        rdfs:isDefinedBy       sosa-common:;
        rdfs:label             "deployed asset"@en;
        schema:domainIncludes  sosa:Deployment;
        schema:rangeIncludes   sosa:Sampler , sosa:Sensor , sosa:System , sosa:Platform , sosa:Actuator;
        owl:inverseOf          sosa:hasDeployment;
        skos:definition        "\n  relation from a Deployment to an asset (System or Platform)\n  "@en .

sosa:Deployment  rdf:type  owl:Class;
        rdfs:isDefinedBy  sosa-common:;
        rdfs:label        "Deployment"@en;
        rdfs:subClassOf   [ rdf:type           owl:Restriction;
                            owl:allValuesFrom  sosa:FeatureOfInterest;
                            owl:onProperty     sosa:hasFeatureOfInterest
                          ];
        rdfs:subClassOf   [ rdf:type           owl:Restriction;
                            owl:allValuesFrom  sosa:System;
                            owl:onProperty     sosa:deployedSystem
                          ];
        rdfs:subClassOf   [ rdf:type           owl:Restriction;
                            owl:allValuesFrom  sosa:Platform;
                            owl:onProperty     sosa:deployedOnPlatform
                          ];
        rdfs:subClassOf   [ rdf:type           owl:Restriction;
                            owl:allValuesFrom  [ rdf:type     owl:Class;
                                                 owl:unionOf  ( sosa:Platform sosa:System )
                                               ];
                            owl:onProperty     sosa:deployedAsset
                          ];
        skos:definition   "\n  arrangement of one or more assets (Systems or Platforms) to execute Procedures with respect to designated features of interest.\n  "@en;
        skos:example      "A temperature Sensor deployed on a wall, a network of Sensors deployed for an Observation campaign."@en;
        skos:note         "\n  A Deployment will usually be for a specified time interval. \n  It MAY involve Platforms, or Systems, or both. \n  A Deployment can be used quite flexibly to describe the use of systems, and platforms that host systems, with respect to a feature of interest. \n  "@en .

sosa:inDeployment  rdf:type    owl:ObjectProperty;
        rdfs:isDefinedBy       sosa-common:;
        rdfs:label             "in deployment"@en;
        rdfs:subPropertyOf     sosa:hasDeployment;
        schema:domainIncludes  sosa:Platform;
        schema:rangeIncludes   sosa:Deployment;
        owl:inverseOf          sosa:deployedOnPlatform;
        skos:definition        "\n  relation from a Platform to a Deployment\n  "@en;
        skos:example           "For example, a relation between a buoy and a deployment of several Sensors."@en .

sosa:hosts  rdf:type            owl:ObjectProperty;
        rdfs:isDefinedBy        sosa-common:;
        rdfs:label              "hosts"@en;
        schema:domainIncludes   sosa:Platform;
        schema:rangeIncludes    sosa:Sampler , sosa:Sensor , sosa:System , sosa:Platform , sosa:Actuator;
        owl:inverseOf           sosa:isHostedBy;
        owl:propertyChainAxiom  ( sosa:inDeployment sosa:deployedSystem );
        skos:definition         "\n  relation from a Platform to an asset (System or Platform) hosted or mounted on it\n  "@en .

sosa:Platform  rdf:type   owl:Class;
        rdfs:isDefinedBy  sosa-common:;
        rdfs:label        "Platform or Host"@en;
        rdfs:subClassOf   prov:Entity;
        rdfs:subClassOf   [ rdf:type           owl:Restriction;
                            owl:allValuesFrom  sosa:Deployment;
                            owl:onProperty     sosa:inDeployment
                          ];
        rdfs:subClassOf   [ rdf:type           owl:Restriction;
                            owl:allValuesFrom  [ owl:unionOf  ( sosa:System sosa:Platform )
                                               ];
                            owl:onProperty     sosa:hosts
                          ];
        dcterms:source    <https://inspire.ec.europa.eu/id/document/tg/ef>;
        skos:altLabel     "Host";
        skos:definition   "\n  entity that hosts other entities, particularly Systems and other Platforms\n  "@en;
        skos:example      "A post, buoy, vehicle, ship, aircraft, satellite, cell-phone, human or animal may act as platforms for (technical or biological) sensors or actuators.\n  An environmental monitoring facility. \n  A platform that hosts a set of sensors. \n  A team performing a survey, where each team member would be modeled as an Observer."@en;
        skos:prefLabel    "Platform";
        skos:scopeNote    "The INSPIRE 'Environmental Monitoring Facility' may be implemented using SOSA by the OWL/RDFS class 'Platform'" .

sosa:hasDeployment  rdf:type   owl:ObjectProperty;
        rdfs:isDefinedBy       sosa-common:;
        rdfs:label             "has deployment"@en;
        schema:domainIncludes  sosa:Sampler , sosa:Sensor , sosa:Platform , sosa:System , sosa:Actuator;
        schema:rangeIncludes   sosa:Deployment;
        owl:inverseOf          sosa:deployedAsset;
        skos:definition        "\n  relation from an asset (System or Platform) to a Deployment\n  "@en .

sosa:isHostedBy  rdf:type      owl:ObjectProperty;
        rdfs:isDefinedBy       sosa-common:;
        rdfs:label             "is hosted by"@en;
        schema:domainIncludes  sosa:Sampler , sosa:Sensor , sosa:Platform , sosa:System , sosa:Actuator;
        schema:rangeIncludes   sosa:Platform;
        owl:inverseOf          sosa:hosts;
        skos:definition        "\n  relation from an asset (System or Platform), to a Platform that it is mounted on or hosted by\n  "@en .

sosa:isSubSystemOf  rdf:type   owl:ObjectProperty;
        rdfs:isDefinedBy       sosa-common:;
        rdfs:label             "is subsystem of"@en;
        schema:domainIncludes  sosa:Sampler , sosa:Sensor , sosa:System , sosa:Actuator;
        schema:rangeIncludes   sosa:Sampler , sosa:Sensor , sosa:System , sosa:Actuator;
        owl:inverseOf          sosa:hasSubSystem;
        skos:definition        "\n  relation from a component System to a System that it belongs to\n  "@en .

sosa:hasSubSystem  rdf:type    owl:ObjectProperty;
        rdfs:isDefinedBy       sosa-common:;
        rdfs:label             "has subsystem"@en;
        schema:domainIncludes  sosa:Sampler , sosa:Sensor , sosa:System , sosa:Actuator;
        schema:rangeIncludes   sosa:Sampler , sosa:Sensor , sosa:System , sosa:Actuator;
        owl:inverseOf          sosa:isSubSystemOf;
        skos:definition        "\n  relation from a System to its component parts\n  "@en .

sosa:implements  rdf:type      owl:ObjectProperty;
        rdfs:isDefinedBy       sosa-common:;
        rdfs:label             "implements"@en;
        schema:domainIncludes  sosa:Sampler , sosa:Sensor , sosa:System , sosa:Actuator;
        schema:rangeIncludes   sosa:SamplingProcedure , sosa:ObservingProcedure , sosa:Procedure , sosa:ActuatingProcedure;
        owl:inverseOf          sosa:implementedBy;
        skos:definition        "\n  relation from a System to the Procedure that it is capable of executing\n  "@en;
        skos:example           "For example, the relationship between a sensor and the scientific measuring Procedure via which it senses."@en .

sosa:System  rdf:type     owl:Class;
        rdfs:isDefinedBy  sosa-common:;
        rdfs:label        "System"@en;
        rdfs:subClassOf   prov:Agent , prov:Entity;
        rdfs:subClassOf   [ rdf:type           owl:Restriction;
                            owl:allValuesFrom  [ rdf:type     owl:Class;
                                                 owl:unionOf  ( sosa:Execution sosa:ExecutionCollection )
                                               ];
                            owl:onProperty     sosa:madeExecution
                          ];
        rdfs:subClassOf   [ rdf:type           owl:Restriction;
                            owl:allValuesFrom  sosa:Platform;
                            owl:onProperty     sosa:isHostedBy
                          ];
        rdfs:subClassOf   [ rdf:type           owl:Restriction;
                            owl:allValuesFrom  sosa:Procedure;
                            owl:onProperty     sosa:implements
                          ];
        rdfs:subClassOf   [ rdf:type           owl:Restriction;
                            owl:allValuesFrom  sosa:Property;
                            owl:onProperty     sosa:forProperty
                          ];
        rdfs:subClassOf   [ rdf:type           owl:Restriction;
                            owl:allValuesFrom  sosa:System;
                            owl:onProperty     sosa:hasSubSystem
                          ];
        rdfs:subClassOf   [ rdf:type           owl:Restriction;
                            owl:allValuesFrom  sosa:System;
                            owl:onProperty     sosa:isSubSystemOf
                          ];
        rdfs:subClassOf   [ rdf:type           owl:Restriction;
                            owl:allValuesFrom  sosa:Deployment;
                            owl:onProperty     sosa:hasDeployment
                          ];
        skos:definition   "\n  entity that implements a Procedure in the context of an Execution\n  "@en;
        skos:note         "\n  This may be a device, a piece of infrastructure, an agent (including humans), or software (simulation).\n\n  Different Systems can implement the same (reusable) Procedure for different Executions.\n\n  A System may have components, its sub-systems, which are other systems.\n  "@en;
        skos:scopeNote    "\n  System generalizes the Actuator, Sensor, and Sampler classes. \n  It is included in the ontology to support the definition of a common pattern for executions and their properties. \n\n  System MUST be considered to be abstract, so any individual System SHOULD be declared to be an instance of a concrete sub-class, and not of the System class.\n  "@en , "\n  Specific system types may be implemented as sub-classes of this class or its sub-classes.\n  Their descriptions may capture the properties and characteristics of a whole class of systems, corresponding with the information typically found in a data-sheet.\n\n  Individual system instances are members of this class or its sub-classes. \n  "@en , "\n  The association of a System (Actuator, Sensor, and Sampler) with a FeatureOfInterest is usually in the context of an Execution or a Deployment. \n\n  A System can be hosted by a Platform. \n\n  A System can be deployed for a specified time interval as part of a Deployment.\n  "@en .

sosa:hasSimpleResult  rdf:type  owl:FunctionalProperty , owl:DatatypeProperty;
        rdfs:isDefinedBy       sosa-common:;
        rdfs:label             "has simple result"@en;
        schema:domainIncludes  sosa:ObservationCollection , sosa:Observation , sosa:ExecutionCollection , sosa:Execution , sosa:ActuationCollection , sosa:Actuation;
        skos:definition        "\n  relation from an Execution to its value expressed as a literal\n\n  In the case of an Actuation, the result may be the value of the Property following the execution of the Procedure by the Actuator. \n\n  In the case of an Observation, the result is the value of the Property produced by the execution of the Procedure by the Sensor. \n  "@en;
        skos:example           "For instance, the values 23 or true."@en;
        skos:note              "This DatatypeProperty provides an alternative to hasResult, to be used only if the execution result can be expressed as a Literal"@en .

sosa:isResultOf  rdf:type      owl:ObjectProperty;
        rdfs:isDefinedBy       sosa-common:;
        rdfs:label             "is result of"@en;
        rdfs:subPropertyOf     prov:wasGeneratedBy;
        schema:domainIncludes  sosa:Sample;
        schema:rangeIncludes   sosa:Sampling , sosa:Observation , sosa:ExecutionCollection , sosa:Execution , sosa:Actuation;
        owl:inverseOf          sosa:hasResult;
        skos:definition        "\n  relation from a result to the Execution that created or caused it\n  "@en .

sosa:hasResult  rdf:type       owl:ObjectProperty , owl:FunctionalProperty;
        rdfs:isDefinedBy       sosa-common:;
        rdfs:label             "has result"@en;
        rdfs:subPropertyOf     prov:generated;
        schema:domainIncludes  sosa:Actuation , sosa:ActuationCollection , sosa:Execution , sosa:ExecutionCollection , sosa:Observation , sosa:ObservationCollection , sosa:Sampling , sosa:SamplingCollection;
        schema:rangeIncludes   sosa:Sample;
        owl:inverseOf          sosa:isResultOf;
        skos:definition        "\n  relation from an Execution to its result\n\n  In the case of an Actuation, the result may be the value of the Property following the execution of the Procedure by the Actuator. \n\n  In the case of an Observation, the result is the value of the Property produced by the execution of the Procedure by the Sensor. \n  \n  In the case of a Sampling, the result is the Sample produced by the execution of the Procedure by the Sampler. \n\n  An Execution has a single result, therefore sosa:hasResult is Functional.\n  "@en;
        skos:note              "The result value MUST be consistent with the hasOutput definition from the corresponding Procedure"@en .

sosa:inputValueForExecution
        rdf:type              owl:ObjectProperty;
        rdfs:isDefinedBy      sosa-common:;
        rdfs:label            "input value for execution"@en;
        schema:rangeIncludes  sosa:Sampling , sosa:Observation , sosa:ExecutionCollection , sosa:Execution , sosa:ActuationCollection , sosa:Actuation;
        owl:inverseOf         sosa:hasInputValue;
        skos:definition       "\n  relation from an input value to an Execution that used it\n  "@en .

sosa:hasInputValue  rdf:type   owl:ObjectProperty;
        rdfs:isDefinedBy       sosa-common:;
        rdfs:label             "has input value"@en;
        schema:domainIncludes  sosa:Sampling , sosa:Observation , sosa:ExecutionCollection , sosa:Execution , sosa:ActuationCollection , sosa:Actuation;
        skos:definition        "\n  assigns a value to an input defined by the Procedure that is used in an Execution\n  "@en;
        skos:note              "The input value MUST be consistent with a hasInput definition from the corresponding Procedure"@en;
        skos:scopeNote         "The input might be a calibration or conditioning parameter, or the output of a previous procedure within an extended processing chain."@en .

sosa:hasUltimateFeatureOfInterest
        rdf:type               owl:ObjectProperty;
        rdfs:isDefinedBy       sosa-common:;
        rdfs:label             "has ultimate feature of interest"@en;
        schema:domainIncludes  sosa:Actuation , sosa:ActuationCollection , sosa:Deployment , sosa:Execution , sosa:ExecutionCollection , sosa:Observation , sosa:ObservationCollection , sosa:Sampling , sosa:SamplingCollection;
        schema:rangeIncludes   sosa:FeatureOfInterest;
        skos:definition        "\n  relation from a Deployment or Execution to its ultimate subject entity\n\n  i.e., from an Actuation to the ultimate entity whose property was modified;\n  from an Observation to the ultimate entity whose property was observed;\n  from an act of Sampling to the ultimate entity that was sampled;\n  or from a Deployment to its ultimate target\n  "@en;
        skos:note              "should match a property chain something like this but with sosa:isSampleOf*\n      owl:propertyChainAxiom ( sosa:hasFeatureOfInterest sosa:isSampleOf )";
        skos:scopeNote         "This is useful when the proximate feature of interest is a sample of the ultimate feature of interest, directly or transitively." .

sosa:hasFeatureOfInterest
        rdf:type               owl:ObjectProperty;
        rdfs:isDefinedBy       sosa-common:;
        rdfs:label             "has feature of interest"@en;
        rdfs:subPropertyOf     prov:used;
        schema:domainIncludes  sosa:SamplingCollection , sosa:Sampling , sosa:Actuation , sosa:ActuationCollection , sosa:Deployment , sosa:Execution , sosa:ExecutionCollection , sosa:Observation , sosa:ObservationCollection;
        schema:rangeIncludes   sosa:FeatureOfInterest;
        owl:inverseOf          sosa:isFeatureOfInterestOf;
        skos:definition        "\n  relation from an Execution or Deployment to its subject entity\n\n  i.e., from an Actuation to the entity whose property was modified;\n  from an Observation to the entity whose quality was observed;\n  from an act of Sampling to the entity that was sampled;\n  or from a Deployment to its target\n  "@en;
        skos:example           "For example, in an Observation of the weight of a person, the FeatureOfInterest is the person and the property is its weight."@en;
        skos:scopeNote         "This is the _proximate_ feature of interest, which may be a proxy entity such as a sample of the _ultimate_ feature of interest. Use `hasUltimateFeatureOfInterest` if the intention is to link to the _ultimate_ feature of interest. " .

sosa:phenomenonOccurred
        rdf:type               owl:ObjectProperty;
        rdfs:isDefinedBy       sosa-common:;
        rdfs:label             "phenomenon occurred"@en;
        schema:domainIncludes  time:TemporalEntity;
        schema:rangeIncludes   sosa:Sampling , sosa:Observation , sosa:ExecutionCollection , sosa:Execution , sosa:ActuationCollection , sosa:Actuation;
        owl:inverseOf          sosa:phenomenonTime;
        skos:definition        "\n  result of an Execution that this time applies to\n  "@en .

sosa:phenomenonTime  rdf:type  owl:ObjectProperty;
        rdfs:isDefinedBy       sosa-common:;
        rdfs:label             "phenomenon time"@en;
        schema:domainIncludes  sosa:SamplingCollection , sosa:Sampling , sosa:ObservationCollection , sosa:Observation , sosa:ExecutionCollection , sosa:Execution , sosa:ActuationCollection , sosa:Actuation;
        schema:rangeIncludes   time:TemporalEntity;
        owl:inverseOf          sosa:phenomenonOccurred;
        skos:definition        "\n  time that the result of an Execution applies to the subject entity\n\n  It may be an interval or an instant, or some other compound temporal entity [[!owl-time]].\n  "@en;
        skos:scopeNote         "\n  The phenomenonTime is not necessarily the same as the resultTime. \n  \n  In the case of Actuation, phenomenonTime SHOULD indicate the time during which the actuator was active. \n\n  In the case of Observation, the phenomenonTime MAY be distant from the resultTime. \n  For example in the case of forecasts the phenomenonTime is after the resultTime. \n  In historical, geological and cosmological investigations the phenomenonTime can be far in the past, while the resultTime is contemporary. \n\n  In the case of Sampling the phenomenonTime SHOULD indicate the time during which the Sampling Procedure was active.\n  The resultTime can indicate when the sample comes into the posession of the operator. \n  "@en .

sosa:resultTime  rdf:type      owl:DatatypeProperty;
        rdfs:comment           "The value would usually be encoded using xsd:dateTime xsd:date xsd:gYearMonth xsd:gYear"@en;
        rdfs:isDefinedBy       sosa-common:;
        rdfs:label             "result time"@en;
        schema:domainIncludes  sosa:SamplingCollection , sosa:Sampling , sosa:ObservationCollection , sosa:Observation , sosa:ExecutionCollection , sosa:Execution;
        skos:definition        "\n  instant of time when the result of the Execution became available\n  "@en .

sosa:endTime  rdf:type         owl:DatatypeProperty;
        rdfs:comment           "The value would usually be encoded using xsd:dateTime xsd:date xsd:gYearMonth xsd:gYear"@en;
        rdfs:isDefinedBy       sosa-common:;
        rdfs:label             "end time"@en;
        rdfs:subPropertyOf     prov:endedAtTime;
        schema:domainIncludes  sosa:Deployment , sosa:ExecutionCollection , sosa:Execution , sosa:ActuationCollection , sosa:Actuation;
        skos:definition        "\n  instant of time when the Execution or Deployment was ended or completed\n  "@en .

sosa:startTime  rdf:type       owl:DatatypeProperty;
        rdfs:comment           "The value would usually be encoded using xsd:dateTime xsd:date xsd:gYearMonth xsd:gYear"@en;
        rdfs:isDefinedBy       sosa-common:;
        rdfs:label             "start time"@en;
        rdfs:subPropertyOf     prov:startedAtTime;
        schema:domainIncludes  sosa:SamplingCollection , sosa:Sampling , sosa:ObservationCollection , sosa:Observation , sosa:ExecutionCollection , sosa:Execution , sosa:Deployment , sosa:ActuationCollection , sosa:Actuation;
        skos:definition        "\n  instant of time when the Execution or Deployment was initiated or tasked\n  "@en .

sosa:usedProcedure  rdf:type    owl:ObjectProperty;
        rdfs:isDefinedBy        sosa-common:;
        rdfs:label              "used procedure"@en;
        schema:domainIncludes   sosa:SamplingCollection , sosa:Actuation , sosa:ActuationCollection , sosa:Execution , sosa:ExecutionCollection , sosa:Observation , sosa:ObservationCollection , sosa:Sampling;
        schema:rangeIncludes    sosa:SamplingProcedure , sosa:ActuatingProcedure , sosa:Procedure , sosa:ObservingProcedure;
        owl:inverseOf           sosa:usedForExecution;
        owl:propertyChainAxiom  ( sp:executionAssociation sp:hadProcedure );
        skos:definition         "\n  relation from an Execution or ExecutionCollection to a Procedure used to make it\n  "@en .

sosa:Execution  rdf:type  owl:Class;
        rdfs:isDefinedBy  sosa-common:;
        rdfs:label        "Execution of a Procedure"@en;
        rdfs:subClassOf   prov:Activity;
        rdfs:subClassOf   [ rdf:type           owl:Restriction;
                            owl:allValuesFrom  sosa:FeatureOfInterest;
                            owl:onProperty     sosa:hasUltimateFeatureOfInterest
                          ];
        rdfs:subClassOf   [ rdf:type           owl:Restriction;
                            owl:allValuesFrom  sosa:FeatureOfInterest;
                            owl:onProperty     sosa:hasFeatureOfInterest
                          ];
        rdfs:subClassOf   [ rdf:type            owl:Restriction;
                            owl:onProperty      sosa:hasFeatureOfInterest;
                            owl:someValuesFrom  sosa:FeatureOfInterest
                          ];
        rdfs:subClassOf   [ rdf:type           owl:Restriction;
                            owl:allValuesFrom  sosa:Procedure;
                            owl:onProperty     sosa:usedProcedure
                          ];
        rdfs:subClassOf   [ rdf:type           owl:Restriction;
                            owl:allValuesFrom  sosa:System;
                            owl:onProperty     sosa:madeBySystem
                          ];
        skos:definition   "\n  act of carrying out a Procedure using a System\n  "@en;
        skos:scopeNote    "\n  Execution generalizes the Actuation, Observation, and Sampling classes. \n  It is included in the ontology to support the definition of a common pattern for executions and their properties. \n\n  Execution MUST be considered to be abstract, so any individual Execution SHOULD be declared to be an instance of one of the concrete sub-classes, and not of the Execution class.\n  "@en .

sosa:outputFor  rdf:type      owl:ObjectProperty;
        rdfs:isDefinedBy      sosa-common:;
        rdfs:label            "output for"@en;
        schema:rangeIncludes  sosa:Procedure;
        owl:inverseOf         sosa:hasOutput;
        skos:definition       "\n  relation from an output to a Procedure that generates it in an Execution\n  "@en .

sosa:hasOutput  rdf:type       owl:ObjectProperty;
        rdfs:isDefinedBy       sosa-common:;
        rdfs:label             "has output"@en;
        schema:domainIncludes  sosa:Procedure;
        owl:inverseOf          sosa:outputFor;
        skos:definition        "\n  relation from a Procedure to an output of its execution\n  "@en;
        skos:note              "This property will typically describe the type of the result from executing the Procedure."@en .

sosa:inputFor  rdf:type       owl:ObjectProperty;
        rdfs:isDefinedBy      sosa-common:;
        rdfs:label            "input for"@en;
        schema:rangeIncludes  sosa:Procedure;
        owl:inverseOf         sosa:hasInput;
        skos:definition       "\n  relation from an input to a Procedure that uses it in an Execution\n  "@en .

sosa:hasInput  rdf:type        owl:ObjectProperty;
        rdfs:isDefinedBy       sosa-common:;
        rdfs:label             "has input"@en;
        schema:domainIncludes  sosa:Procedure;
        owl:inverseOf          sosa:inputFor;
        skos:definition        "\n  relation from a Procedure to an input required for its execution\n  "@en;
        skos:note              "This property will typically describe the type of the inputs required to execute the Procedure."@en;
        skos:scopeNote         "An input might be a calibration or conditioning parameter, or the output of a previous procedure within an extended processing chain."@en .

sosa:implementedBy  rdf:type   owl:ObjectProperty;
        rdfs:isDefinedBy       sosa-common:;
        rdfs:label             "implemented by"@en;
        schema:domainIncludes  sosa:Procedure;
        schema:rangeIncludes   sosa:Sampler , sosa:Sensor , sosa:System , sosa:Actuator;
        owl:inverseOf          sosa:implements;
        skos:definition        "\n  relation from a Procedure to a System that is capable of executing it\n  "@en;
        skos:example           "For example, the relationship between a scientific measuring Procedure and a sensor that senses via that Procedure."@en .

sosa:usedForExecution
        rdf:type               owl:ObjectProperty;
        rdfs:isDefinedBy       sosa-common:;
        rdfs:label             "used for execution"@en;
        schema:domainIncludes  sosa:Procedure;
        schema:rangeIncludes   sosa:Sampling , sosa:Observation , sosa:Execution , sosa:Actuation;
        owl:inverseOf          sosa:usedProcedure;
        skos:definition        "\n  relation from a Procedure to an Execution or ExecutionCollection made using it\n  "@en .

sosa:Procedure  rdf:type  owl:Class;
        rdfs:isDefinedBy  sosa-common:;
        rdfs:label        "Procedure"@en;
        rdfs:subClassOf   prov:Plan;
        rdfs:subClassOf   [ rdf:type           owl:Restriction;
                            owl:allValuesFrom  sosa:Property;
                            owl:onProperty     sosa:forProperty
                          ];
        rdfs:subClassOf   [ rdf:type           owl:Restriction;
                            owl:allValuesFrom  sosa:System;
                            owl:onProperty     sosa:implementedBy
                          ];
        skos:definition   "\n  workflow, protocol, plan, algorithm, or computational method specifying how to make an Execution\n\n  A Procedure is re-usable, and might be applied in many Actuations, Observations, or Samplings.\n  It explains the steps to be carried out to arrive at reproducible results.\n  "@en;
        skos:example      "The measured wind speed differs depending on the height of the sensor above the surface, e.g., due to friction. Consequently, procedures for measuring wind speed define a standard height for anemometers above ground, typically 10m for meteorological measures and 2m in Agrometeorology. This definition of height, sensor placement, and so forth are defined by the Procedure."@en;
        skos:scopeNote    "\n  Procedure generalizes the ActuationProcedure, ObservationProcedure, and SamplingProcedure classes. \n  It is included in the ontology to support the definition of a common pattern for executions and their properties. \n  "@en .

sosa:forProperty  rdf:type     owl:ObjectProperty;
        rdfs:isDefinedBy       sosa-common:;
        rdfs:label             "for property"@en;
        schema:domainIncludes  sosa:Sensor , sosa:System , sosa:Procedure , sosa:Actuator;
        schema:rangeIncludes   sosa:Property;
        owl:inverseOf          sosa:propertyFor;
        skos:definition        "\n  relation from some Procedure or System to a Property it acts on or observes\n  "@en;
        skos:example           "For example, from a Sensor to the properties it can observe; from an Actuator to the properties it can act on; from a SystemCapability to the Property the capability is described for."@en .

sosa:propertyFor  rdf:type     owl:ObjectProperty;
        rdfs:isDefinedBy       sosa-common:;
        rdfs:label             "property for"@en;
        schema:domainIncludes  sosa:Property;
        schema:rangeIncludes   sosa:Sensor , sosa:System , sosa:Procedure , sosa:Actuator;
        owl:inverseOf          sosa:forProperty;
        skos:definition        "\n  relation from a Property to some Procedure or System that acts on it or observes it\n  "@en;
        skos:example           "For example, from a Sensor to the properties it can observe; from an Actuator to the properties it can act on; from a SystemCapability to the Property the capability is described for."@en .

sosa:hasProcedure  rdf:type    owl:ObjectProperty;
        rdfs:isDefinedBy       sosa-common:;
        rdfs:label             "has procedure"@en;
        rdfs:subPropertyOf     sosa:propertyFor;
        schema:domainIncludes  sosa:Property;
        schema:rangeIncludes   sosa:Procedure;
        owl:inverseOf          sosa:isProcedureFor;
        owl:inverseOf          [ rdfs:subPropertyOf
                          sosa:forProperty ];
        skos:definition        "\n  relation from a Property to a Procedure that can observe or act on it\n  "@en .

sosa:isPropertyOf  rdf:type    owl:ObjectProperty;
        rdfs:isDefinedBy       sosa-common:;
        rdfs:label             "is property of"@en;
        schema:domainIncludes  sosa:Property;
        schema:rangeIncludes   sosa:FeatureOfInterest;
        owl:inverseOf          sosa:hasProperty;
        skos:definition        "\n  relation from a Property to a FeatureOfInterest that it is a quality of\n  "@en .

sosa:Property  rdf:type   owl:Class;
        rdfs:isDefinedBy  sosa-common:;
        rdfs:label        "Property"@en;
        rdfs:subClassOf   prov:Entity;
        rdfs:subClassOf   [ rdf:type           owl:Restriction;
                            owl:allValuesFrom  sosa:Stimulus;
                            owl:onProperty     [ owl:inverseOf  sosa:isProxyFor ]
                          ];
        rdfs:subClassOf   [ rdf:type           owl:Restriction;
                            owl:allValuesFrom  [ owl:unionOf  ( sosa:Observation sosa:ObservationCollection )
                                               ];
                            owl:onProperty     sosa:wasObservedBy
                          ];
        rdfs:subClassOf   [ rdf:type           owl:Restriction;
                            owl:allValuesFrom  sosa:Sensor;
                            owl:onProperty     sosa:isObservedBy
                          ];
        rdfs:subClassOf   [ rdf:type           owl:Restriction;
                            owl:allValuesFrom  sosa:Procedure;
                            owl:onProperty     sosa:hasProcedure
                          ];
        rdfs:subClassOf   [ rdf:type           owl:Restriction;
                            owl:allValuesFrom  sosa:FeatureOfInterest;
                            owl:onProperty     sosa:isPropertyOf
                          ];
        rdfs:subClassOf   [ rdf:type           owl:Restriction;
                            owl:allValuesFrom  [ owl:unionOf  ( sosa:Actuation sosa:ActuationCollection )
                                               ];
                            owl:onProperty     sosa:wasActedOnBy
                          ];
        rdfs:subClassOf   [ rdf:type           owl:Restriction;
                            owl:allValuesFrom  sosa:Actuator;
                            owl:onProperty     sosa:isActedOnBy
                          ];
        skos:definition   "\n  identifiable quality of features of interest that can be observed or acted upon\n\n  A property can apply to different features of interest.\n\n  "@en;
        skos:example      "Cars (a feature type) all have a characteristic colour, where 'colour' is a property."@en;
        skos:note         "Concepts from existing code lists, vocabularies, and taxonomies, may be used as instances of Property"@en .

sosa:isUltimateFeatureOfInterestOf
        rdf:type               owl:ObjectProperty;
        rdfs:isDefinedBy       sosa-common:;
        rdfs:label             "is ultimate feature of interest of"@en;
        schema:domainIncludes  sosa:FeatureOfInterest;
        schema:rangeIncludes   sosa:SamplingCollection , sosa:Sampling , sosa:ObservationCollection , sosa:Observation , sosa:ExecutionCollection , sosa:Execution , sosa:Deployment , sosa:ActuationCollection , sosa:Actuation;
        owl:inverseOf          sosa:hasUltimateFeatureOfInterest;
        skos:definition        "\n  relation from an ultimate FeatureOfInterest to an Execution, Execution Collection, or Deployment, for which it is the ultimate subject\n  "@en .

sosa:isFeatureOfInterestOf
        rdf:type               owl:ObjectProperty;
        rdfs:isDefinedBy       sosa-common:;
        rdfs:label             "is feature of interest of"@en;
        schema:domainIncludes  sosa:FeatureOfInterest;
        schema:rangeIncludes   sosa:SamplingCollection , sosa:Sampling , sosa:ObservationCollection , sosa:Observation , sosa:ExecutionCollection , sosa:Execution , sosa:Deployment , sosa:ActuationCollection , sosa:Actuation;
        owl:inverseOf          sosa:hasFeatureOfInterest;
        skos:definition        "\n  relation from a FeatureOfInterest to an Execution, Execution Collection, or Deployment, operating on it\n\n  i.e., to an Observation about it, to an Actuation acting on it, to an act of Sampling that sampled it,\n  or to a Deployment for which it is the subject.\n"@en .

sosa:hasProperty  rdf:type     owl:ObjectProperty;
        rdfs:isDefinedBy       sosa-common:;
        rdfs:label             "has property"@en;
        schema:domainIncludes  sosa:FeatureOfInterest;
        schema:rangeIncludes   sosa:Property;
        owl:inverseOf          sosa:isPropertyOf;
        skos:definition        "\n  relation from an entity to a Property of that entity\n  "@en .

sosa:FeatureOfInterest
        rdf:type          owl:Class;
        rdfs:isDefinedBy  sosa-common:;
        rdfs:label        "Feature Of Interest"@en;
        rdfs:subClassOf   prov:Entity;
        rdfs:subClassOf   [ rdf:type           owl:Restriction;
                            owl:allValuesFrom  sosa:Sample;
                            owl:onProperty     sosa:hasSample
                          ];
        rdfs:subClassOf   [ rdf:type           owl:Restriction;
                            owl:allValuesFrom  sosa:Property;
                            owl:onProperty     sosa:hasProperty
                          ];
        rdfs:subClassOf   [ rdf:type            owl:Restriction;
                            owl:onProperty      sosa:isFeatureOfInterestOf;
                            owl:someValuesFrom  [ rdf:type     owl:Class;
                                                  owl:unionOf  ( sosa:Deployment sosa:Execution sosa:ExecutionCollection )
                                                ]
                          ];
        skos:definition   "\n  entity that is the target of an Execution or Deployment\n\n  i.e., whose property is being estimated by an Observation, \n  or whose property is being manipulated by an Actuator, \n  or which is being sampled or transformed in an act of Sampling, \n  or which is the target of Executions planned as part of a Deployment.\n  "@en;
        skos:example      "When measuring the height of a tree, the height is the observed Property, 20m may be the Result of the Observation, and the tree is the FeatureOfInterest. A window is a FeatureOfInterest for an automatic window control Actuation."@en .

sosa:isMemberOf  rdf:type      owl:ObjectProperty;
        rdfs:isDefinedBy       sosa-common:;
        rdfs:label             "is member of collection";
        schema:domainIncludes  sosa:SamplingCollection , sosa:Sampling , sosa:SampleCollection , sosa:Sample , sosa:ActuationCollection , sosa:Actuation , sosa:Execution , sosa:ExecutionCollection , sosa:Observation , sosa:ObservationCollection;
        schema:rangeIncludes   sosa:SamplingCollection , sosa:SampleCollection , sosa:ActuationCollection , sosa:ExecutionCollection , sosa:ObservationCollection;
        owl:inverseOf          sosa:hasMember;
        skos:definition        "\n  link from an Execution or Sample or Collection of these, to a collection that it is part of\n  ";
        skos:editorialNote     "Note that there is a single `member` property. OWL or SHACL constraints may limit the range depending on the context of different collection types";
        skos:scopeNote         "rules for the consistency of values of properties of collections and properties of their members are given for each collection type" .

sosa:hasMember  rdf:type       owl:ObjectProperty;
        rdfs:isDefinedBy       sosa-common:;
        rdfs:label             "has member of collection";
        schema:domainIncludes  sosa:SamplingCollection , sosa:SampleCollection , sosa:ActuationCollection , sosa:ExecutionCollection , sosa:ObservationCollection;
        schema:rangeIncludes   sosa:SamplingCollection , sosa:Sampling , sosa:SampleCollection , sosa:Sample , sosa:Actuation , sosa:ActuationCollection , sosa:Execution , sosa:ExecutionCollection , sosa:Observation , sosa:ObservationCollection;
        owl:inverseOf          sosa:isMemberOf;
        skos:definition        "\n  link from a Collection to an Execution or Sample or Collection of these that is part of it\n  ";
        skos:editorialNote     "Note that there is a single `member` property. OWL or SHACL constraints may limit the range depending on the context of different collection types";
        skos:scopeNote         "rules for the consistency of values of properties of collections and properties of their members are given for each collection type" .

sosa:wasActedOnBy  rdf:type    owl:ObjectProperty;
        rdfs:isDefinedBy       sosa-act:;
        rdfs:label             "was acted on by"@en;
        schema:domainIncludes  sosa:Property;
        schema:rangeIncludes   sosa:ActuationCollection , sosa:Actuation;
        owl:inverseOf          sosa:actsOnProperty;
        skos:definition        "\n  relation from a Property to an Actuation that changed its state\n  "@en;
        skos:example           "In the activity (Actuation) of automatically closing a window if the temperature in a room drops below 20 degrees Celsius, the property upon which the Actuator acts is the state of the window as it changes from being open to being closed. "@en .

sosa:madeByActuator  rdf:type  owl:ObjectProperty;
        rdfs:isDefinedBy       sosa-act:;
        rdfs:label             "made by actuator"@en;
        rdfs:subPropertyOf     sosa:madeBySystem;
        schema:domainIncludes  sosa:ActuationCollection , sosa:Actuation;
        schema:rangeIncludes   sosa:Actuator;
        owl:inverseOf          sosa:madeActuation;
        skos:definition        "\n  relation from an Actuation or ActuationCollection to the Actuator that made it\n  "@en .

sosa:madeActuation  rdf:type   owl:ObjectProperty;
        rdfs:isDefinedBy       sosa-act:;
        rdfs:label             "made actuation"@en;
        rdfs:subPropertyOf     sosa:madeExecution;
        schema:domainIncludes  sosa:Actuator;
        schema:rangeIncludes   sosa:ActuationCollection , sosa:Actuation;
        owl:inverseOf          sosa:madeByActuator;
        skos:definition        "\n  relation from an Actuator to an Actuation or ActuationCollection it has made\n  "@en .

sosa:isActedOnBy  rdf:type     owl:ObjectProperty;
        rdfs:isDefinedBy       sosa-act:;
        rdfs:label             "is acted on by"@en;
        schema:domainIncludes  sosa:Property;
        schema:rangeIncludes   sosa:Actuator;
        owl:inverseOf          sosa:actsOn;
        skos:definition        "\n  relation from a Property to an Actuator that may change its state\n  "@en;
        skos:example           "In the activity (Actuation) of automatically closing a window if the temperature in a room drops below 20 degrees Celsius, the property upon which the Actuator acts is the state of the window as it changes from being open to being closed. "@en .

sosa:actsOnProperty  rdf:type  owl:ObjectProperty;
        rdfs:isDefinedBy       sosa-act:;
        rdfs:label             "acts on property"@en;
        schema:domainIncludes  sosa:ActuationCollection , sosa:Actuation;
        schema:rangeIncludes   sosa:Property;
        owl:inverseOf          sosa:wasActedOnBy;
        skos:definition        "\n  relation from an Actuation to the Property it acted upon\n  "@en;
        skos:example           "In the activity (Actuation) of automatically closing a window if the temperature in a room drops below 20 degrees Celsius, the property upon which the Actuator acts is the state of the window as it changes from being open to being closed. "@en .

sosa:actsOn  rdf:type          owl:ObjectProperty;
        rdfs:isDefinedBy       sosa-act:;
        rdfs:label             "acts on"@en;
        rdfs:subPropertyOf     sosa:forProperty;
        schema:domainIncludes  sosa:Actuator;
        schema:rangeIncludes   sosa:Property;
        owl:inverseOf          sosa:isActedOnBy;
        skos:definition        "\n  relation from an Actuator to a Property whose state may be changed by using it\n  "@en;
        skos:example           "In the activity (Actuation) of automatically closing a window if the temperature in a room drops below 20 degrees Celsius, the property upon which the Actuator acts is the state of the window as it changes from being open to being closed. "@en .

sosa:Actuator  rdf:type   owl:Class;
        rdfs:isDefinedBy  sosa-act:;
        rdfs:label        "Actuator"@en;
        rdfs:subClassOf   sosa:System;
        rdfs:subClassOf   [ rdf:type           owl:Restriction;
                            owl:allValuesFrom  [ rdf:type     owl:Class;
                                                 owl:unionOf  ( sosa:Actuation sosa:ActuationCollection )
                                               ];
                            owl:onProperty     sosa:madeActuation
                          ];
        rdfs:subClassOf   [ rdf:type           owl:Restriction;
                            owl:allValuesFrom  sosa:ActuatingProcedure;
                            owl:onProperty     sosa:implements
                          ];
        rdfs:subClassOf   [ rdf:type           owl:Restriction;
                            owl:allValuesFrom  sosa:Property;
                            owl:onProperty     sosa:actsOn
                          ];
        skos:definition   "\n  System that implements an ActuatingProcedure to change the value of an actuatable Property\n\n  This may be a device, a piece of infrastructure, an agent (including humans), or software (simulation)."@en;
        skos:example      "A window actuator for automatic window control, i.e., opening or closing the window."@en .

sosa:ActuationCollection
        rdf:type          owl:Class;
        rdfs:isDefinedBy  sosa-act:;
        rdfs:label        "Actuation Collection"@en;
        rdfs:subClassOf   sosa:ExecutionCollection;
        rdfs:subClassOf   [ rdf:type           owl:Restriction;
                            owl:allValuesFrom  [ owl:unionOf  ( sosa:Actuation sosa:ActuationCollection )
                                               ];
                            owl:onProperty     sosa:hasMember
                          ];
        rdfs:subClassOf   [ rdf:type           owl:Restriction;
                            owl:allValuesFrom  sosa:FeatureOfInterest;
                            owl:onProperty     sosa:hasFeatureOfInterest
                          ];
        rdfs:subClassOf   [ rdf:type           owl:Restriction;
                            owl:allValuesFrom  sosa:ActuatingProcedure;
                            owl:onProperty     sosa:usedProcedure
                          ];
        rdfs:subClassOf   [ rdf:type           owl:Restriction;
                            owl:allValuesFrom  sosa:Property;
                            owl:onProperty     sosa:actsOnProperty
                          ];
        rdfs:subClassOf   [ rdf:type           owl:Restriction;
                            owl:allValuesFrom  sosa:Actuator;
                            owl:onProperty     sosa:madeByActuator
                          ];
        owl:disjointWith  sosa:SamplingCollection , sosa:SampleCollection , sosa:ObservationCollection;
        skos:definition   "\n  set of one or more Actuations or ActuationCollections; collections may be nested\n\n  All Actuation properties may appear in an Actuation Collection, including:\n  hasFeatureOfInterest , usedProcedure , madeByActuator , actsOnProperty , endTime ,  hasResult , hasSimpleResult . \n  If they are present, the value of these properties summarize the values of the matching properties of the member actuations, where membership is either direct or transitive through one or more member actuation collections. \n  The following consistency rules apply with respect to the Actuation properties: \n  \n  1. Where an individual Actuation Collection omits a property, a member Actuation (direct or transitive) MAY have any value for that property.\n\n  2. Where an individual Actuation Collection has a single value for a property, each member Actuation (direct or transitive) MUST have that same value for the property - i.e., the collection is homogeneous in that property.  That property MAY then be omitted in any member Actuation or Actuation Collection.\n\n  3. Where an individual Actuation Collection has more than one value for a property, each member Actuation (direct or transitive) MUST have a value for that property that matches one of the values for the property in the collection. \n  \n  4. Where an individual Actuation Collection has a value for a property that is a range or interval, each member Actuation (direct or transitive) MUST have a value for that property that matches or falls within that range or interval.\n\n  5. Where an individual Actuation Collection has more than one value for a property that is a range or interval, each member Actuation (direct or transitive) MUST have a value for that property that either matches or falls within one of those ranges or intervals.\n  "@en;
        skos:note         "The members of a collection do not necessarily share a common value for any property. "@en .

sosa:Actuation  rdf:type  owl:Class;
        rdfs:isDefinedBy  sosa-act:;
        rdfs:label        "Actuation"@en;
        rdfs:subClassOf   sosa:Execution;
        rdfs:subClassOf   [ rdf:type           owl:Restriction;
                            owl:allValuesFrom  sosa:FeatureOfInterest;
                            owl:onProperty     sosa:hasFeatureOfInterest
                          ];
        rdfs:subClassOf   [ rdf:type           owl:Restriction;
                            owl:allValuesFrom  sosa:ActuatingProcedure;
                            owl:onProperty     sosa:usedProcedure
                          ];
        rdfs:subClassOf   [ rdf:type           owl:Restriction;
                            owl:allValuesFrom  sosa:Property;
                            owl:onProperty     sosa:actsOnProperty
                          ];
        rdfs:subClassOf   [ rdf:type           owl:Restriction;
                            owl:allValuesFrom  sosa:Actuator;
                            owl:onProperty     sosa:madeByActuator
                          ];
        skos:definition   "\n  act of carrying out an ActuatingProcedure using an Actuator to change the value of an actuatable Property of a FeatureOfInterest\n  \n  In this context hasResult may indicate the value of the Property at the completion of the Actuation\n  "@en;
        skos:example      "The activity of automatically closing a window if the temperature in a room drops below 20 degree Celsius. The activity is the Actuation and the device that closes the window is the Actuator. The Procedure is the rule, plan, or specification that defines the conditions that triggers the Actuation, here a drop in temperature. "@en;
        skos:note         "relatedObservation SHOULD be used to link to an associated Observation or ObservationCollection that monitors the actuated property to verify that the result value has been obtained. "@en;
        skos:scopeNote    "\n  An Actuation primarily concerns a single Property of a single FeatureOfInterest. \n  Changes to multiple properties, or other combinations of Actuations, may be described in an ActuationCollection.\n    \n  Alternatively, applications may choose to encapsulate complexity by defining a complex property with multiple individual components, and a corresponding complex result (e.g., a vector). \n  This approach is not prohibited by the SSN Ontology, but the details are beyond the scope of SSN.\n  "@en .

sosa:ActuatingProcedure
        rdf:type          owl:Class;
        rdfs:isDefinedBy  sosa-act:;
        rdfs:label        "Actuating Procedure"@en;
        rdfs:subClassOf   sosa:Procedure;
        rdfs:subClassOf   [ rdf:type           owl:Restriction;
                            owl:allValuesFrom  sosa:Actuator;
                            owl:onProperty     sosa:implementedBy
                          ];
        skos:definition   "\n  workflow, protocol, plan, algorithm, or computational method specifying how to make an Actuation\n  \n  An Actuating Procedure is re-usable, and might be applied in many Actuations.\n  It explains the steps to be carried out to arrive at reproducible results.\n  "@en .

sosa-act:  rdf:type          owl:Ontology;
        dcterms:created      "2024-02-02"^^xsd:date;
        dcterms:creator      [ rdf:type   foaf:Agent;
                               foaf:name  "W3C/OGC Spatial Data on the Web Working Group"@en
                             ];
        dcterms:description  "Actuation classes and properties for the SSN Ontology."@en;
        dcterms:license      <http://www.opengeospatial.org/ogc/Software> , <http://www.w3.org/Consortium/Legal/2015/copyright-software-and-document>;
        dcterms:rights       "Copyright 2025 W3C/OGC.";
        dcterms:title        "Sensor, Observation, Sample, and Actuator (SOSA) Ontology - actuation module"@en;
        owl:imports          sosa-common: .

prov:mentionOf  rdf:type    owl:ObjectProperty;
        rdfs:comment        "prov:mentionOf is used to specialize an entity as described in another bundle. It is to be used in conjuction with prov:asInBundle.\n\nprov:asInBundle is used to cite the Bundle in which the generalization was mentioned."@en;
        rdfs:domain         prov:Entity;
        rdfs:isDefinedBy    <http://www.w3.org/ns/prov-links#>;
        rdfs:label          "mentionOf";
        rdfs:range          prov:Entity;
        rdfs:subPropertyOf  prov:specializationOf;
        prov:inverse        "hadMention" .

prov:asInBundle  rdf:type          owl:ObjectProperty;
        rdfs:comment               "prov:asInBundle is used to specify which bundle the general entity of a prov:mentionOf property is described.\n\nWhen :x prov:mentionOf :y and :y is described in Bundle :b, the triple :x prov:asInBundle :b is also asserted to cite the Bundle in which :y was described."@en;
        rdfs:domain                prov:Entity;
        rdfs:isDefinedBy           <http://www.w3.org/ns/prov-links#>;
        rdfs:label                 "asInBundle";
        rdfs:range                 prov:Bundle;
        prov:inverse               "contextOf";
        prov:sharesDefinitionWith  prov:mentionOf .

<http://www.w3.org/ns/prov-links#>
        rdf:type               owl:Ontology;
        rdfs:comment           "This document is published by the Provenance Working Group (http://www.w3.org/2011/prov/wiki/Main_Page). If you wish to make comments regarding this document, please send them to public-prov-comments@w3.org (subscribe public-prov-comments-request@w3.org, archives http://lists.w3.org/Archives/Public/public-prov-comments/\n). All feedback is welcome."@en;
        rdfs:label             "W3C PROV Linking Across Provenance Bundles Ontology (PROV-LINKS)"@en;
        rdfs:seeAlso           <http://www.w3.org/ns/prov> , <http://www.w3.org/TR/prov-links/>;
        owl:imports            <http://www.w3.org/ns/prov-o#>;
        owl:versionIRI         <http://www.w3.org/ns/prov-links-20130430>;
        owl:versionInfo        "Working Group Note version 2013-04-30"@en;
        prov:specializationOf  <http://www.w3.org/ns/prov-links> .

prov:removedKey  rdf:type  owl:DatatypeProperty;
        rdfs:domain       prov:Removal;
        rdfs:isDefinedBy  prov:;
        rdfs:label        "removedKey";
        rdfs:range        rdfs:Literal;
        prov:category     "collections";
        prov:component    "collections";
        prov:constraints  "http://www.w3.org/TR/2013/NOTE-prov-dictionary-20130430/#dictionary-constraints"^^xsd:anyURI;
        prov:definition   "The key removed in a Removal.";
        prov:dm           "http://www.w3.org/TR/2013/NOTE-prov-dictionary-20130430/#term-dictionary-removal"^^xsd:anyURI;
        prov:n            "http://www.w3.org/TR/2013/NOTE-prov-dictionary-20130430/#expression-dictionary-removal"^^xsd:anyURI .

prov:qualifiedRemoval
        rdf:type            owl:ObjectProperty;
        rdfs:domain         prov:Dictionary;
        rdfs:isDefinedBy    prov:;
        rdfs:label          "qualifiedRemoval";
        rdfs:range          prov:Removal;
        rdfs:subPropertyOf  prov:qualifiedDerivation;
        prov:category       "collections";
        prov:component      "collections";
        prov:constraints    "http://www.w3.org/TR/2013/NOTE-prov-dictionary-20130430/#dictionary-constraints"^^xsd:anyURI;
        prov:definition     "The dictionary was derived from the other by removal. prov:qualifiedRemoval shows details of the removal, in particular the removed keys.";
        prov:dm             "http://www.w3.org/TR/2013/NOTE-prov-dictionary-20130430/#term-dictionary-removal"^^xsd:anyURI;
        prov:n              "http://www.w3.org/TR/2013/NOTE-prov-dictionary-20130430/#expression-dictionary-removal"^^xsd:anyURI .

prov:qualifiedInsertion
        rdf:type            owl:ObjectProperty;
        rdfs:domain         prov:Dictionary;
        rdfs:isDefinedBy    prov:;
        rdfs:label          "qualifiedInsertion";
        rdfs:range          prov:Insertion;
        rdfs:subPropertyOf  prov:qualifiedDerivation;
        prov:category       "collections";
        prov:component      "collections";
        prov:constraints    "http://www.w3.org/TR/2013/NOTE-prov-dictionary-20130430/#dictionary-constraints"^^xsd:anyURI;
        prov:definition     "The dictionary was derived from the other by insertion. prov:qualifiedInsertion shows details of the insertion, in particular the inserted key-entity pairs.";
        prov:dm             "http://www.w3.org/TR/2013/NOTE-prov-dictionary-20130430/#term-dictionary-insertion"^^xsd:anyURI;
        prov:n              "http://www.w3.org/TR/2013/NOTE-prov-dictionary-20130430/#expression-dictionary-insertion"^^xsd:anyURI .

prov:pairEntity  rdf:type  owl:FunctionalProperty , owl:ObjectProperty;
        rdfs:domain       prov:KeyEntityPair;
        rdfs:isDefinedBy  prov:;
        rdfs:label        "pairKey";
        rdfs:range        prov:Entity;
        prov:category     "collections";
        prov:component    "collections";
        prov:constraints  "http://www.w3.org/TR/2013/NOTE-prov-dictionary-20130430/#dictionary-constraints"^^xsd:anyURI;
        prov:definition   "The value of a KeyEntityPair.";
        prov:dm           "http://www.w3.org/TR/2013/NOTE-prov-dictionary-20130430/#term-dictionary-membership"^^xsd:anyURI;
        prov:n            "http://www.w3.org/TR/2013/NOTE-prov-dictionary-20130430/#expression-dictionary-membership"^^xsd:anyURI .

prov:pairKey  rdf:type    owl:FunctionalProperty , owl:DatatypeProperty;
        rdfs:domain       prov:KeyEntityPair;
        rdfs:isDefinedBy  prov:;
        rdfs:label        "pairKey";
        rdfs:range        rdfs:Literal;
        prov:category     "collections";
        prov:component    "collections";
        prov:constraints  "http://www.w3.org/TR/2013/NOTE-prov-dictionary-20130430/#dictionary-constraints"^^xsd:anyURI;
        prov:definition   "The key of a KeyEntityPair, which is an element of a prov:Dictionary.";
        prov:dm           "http://www.w3.org/TR/2013/NOTE-prov-dictionary-20130430/#term-dictionary-membership"^^xsd:anyURI;
        prov:n            "http://www.w3.org/TR/2013/NOTE-prov-dictionary-20130430/#expression-dictionary-membership"^^xsd:anyURI .

prov:hadDictionaryMember
        rdf:type          owl:ObjectProperty;
        rdfs:domain       prov:Dictionary;
        rdfs:isDefinedBy  prov:;
        rdfs:label        "hadDictionaryMember";
        rdfs:range        prov:KeyEntityPair;
        prov:category     "collections";
        prov:component    "collections";
        prov:constraints  "http://www.w3.org/TR/2013/NOTE-prov-dictionary-20130430/#dictionary-constraints"^^xsd:anyURI;
        prov:definition   "Describes the key-entity pair that was member of a prov:Dictionary. A dictionary can have multiple members.";
        prov:dm           "http://www.w3.org/TR/2013/NOTE-prov-dictionary-20130430/#term-dictionary-membership"^^xsd:anyURI;
        prov:n            "http://www.w3.org/TR/2013/NOTE-prov-dictionary-20130430/#expression-dictionary-membership"^^xsd:anyURI .

prov:insertedKeyEntityPair
        rdf:type          owl:ObjectProperty;
        rdfs:domain       prov:Insertion;
        rdfs:isDefinedBy  prov:;
        rdfs:label        "insertedKeyEntityPair";
        rdfs:range        prov:KeyEntityPair;
        prov:category     "collections";
        prov:component    "collections";
        prov:constraints  "http://www.w3.org/TR/2013/NOTE-prov-dictionary-20130430/#dictionary-constraints"^^xsd:anyURI;
        prov:definition   "An object property to refer to the prov:KeyEntityPair inserted into a prov:Dictionary.";
        prov:dm           "http://www.w3.org/TR/2013/NOTE-prov-dictionary-20130430/#term-dictionary-insertion"^^xsd:anyURI;
        prov:n            "http://www.w3.org/TR/2013/NOTE-prov-dictionary-20130430/#expression-dictionary-insertion"^^xsd:anyURI .

prov:derivedByRemovalFrom
        rdf:type            owl:ObjectProperty;
        rdfs:domain         prov:Dictionary;
        rdfs:isDefinedBy    prov:;
        rdfs:label          "derivedByRemovalFrom";
        rdfs:range          prov:Dictionary;
        rdfs:subPropertyOf  prov:wasDerivedFrom;
        prov:category       "collections";
        prov:component      "collections";
        prov:constraints    "http://www.w3.org/TR/2013/NOTE-prov-dictionary-20130430/#dictionary-constraints"^^xsd:anyURI;
        prov:definition     "The dictionary was derived from the other by removal. prov:qualifiedRemoval shows details of the removal, in particular the removed key-entity pairs.";
        prov:dm             "http://www.w3.org/TR/2013/NOTE-prov-dictionary-20130430/#term-dictionary-removal"^^xsd:anyURI;
        prov:n              "http://www.w3.org/TR/2013/NOTE-prov-dictionary-20130430/#expression-dictionary-removal"^^xsd:anyURI .

prov:derivedByInsertionFrom
        rdf:type            owl:ObjectProperty;
        rdfs:domain         prov:Dictionary;
        rdfs:isDefinedBy    prov:;
        rdfs:label          "derivedByInsertionFrom";
        rdfs:range          prov:Dictionary;
        rdfs:subPropertyOf  prov:wasDerivedFrom;
        prov:category       "collections";
        prov:component      "collections";
        prov:constraints    "http://www.w3.org/TR/2013/NOTE-prov-dictionary-20130430/#dictionary-constraints"^^xsd:anyURI;
        prov:definition     "The dictionary was derived from the other by insertion. prov:qualifiedInsertion shows details of the insertion, in particular the inserted key-entity pairs.";
        prov:dm             "http://www.w3.org/TR/2013/NOTE-prov-dictionary-20130430/#term-dictionary-insertion"^^xsd:anyURI;
        prov:n              "http://www.w3.org/TR/2013/NOTE-prov-dictionary-20130430/#expression-dictionary-insertion"^^xsd:anyURI .

prov:dictionary  rdf:type   owl:ObjectProperty;
        rdfs:domain         prov:Removal , prov:Insertion;
        rdfs:isDefinedBy    prov:;
        rdfs:label          "dictionary";
        rdfs:range          prov:Dictionary;
        rdfs:subPropertyOf  prov:entity;
        prov:category       "collections";
        prov:component      "collections";
        prov:constraints    "http://www.w3.org/TR/2013/NOTE-prov-dictionary-20130430/#dictionary-constraints"^^xsd:anyURI;
        prov:definition     "The property used by a prov:Insertion and prov:Removal to cite the prov:Dictionary that was prov:derivedByInsertionFrom or prov:derivedByRemovalFrom another dictionary.";
        prov:dm             "http://www.w3.org/TR/2013/NOTE-prov-dictionary-20130430/#term-dictionary-removal"^^xsd:anyURI , "http://www.w3.org/TR/2013/NOTE-prov-dictionary-20130430/#term-dictionary-insertion"^^xsd:anyURI;
        prov:n              "http://www.w3.org/TR/2013/NOTE-prov-dictionary-20130430/#expression-dictionary-removal"^^xsd:anyURI , "http://www.w3.org/TR/2013/NOTE-prov-dictionary-20130430/#expression-dictionary-insertion"^^xsd:anyURI .

prov:Removal  rdf:type        owl:Class;
        rdfs:isDefinedBy      prov:;
        rdfs:label            "Removal";
        rdfs:subClassOf       prov:Derivation;
        rdfs:subClassOf       [ rdf:type            owl:Restriction;
                                owl:minCardinality  "1"^^xsd:int;
                                owl:onProperty      prov:removedKey
                              ];
        rdfs:subClassOf       [ rdf:type         owl:Restriction;
                                owl:cardinality  "1"^^xsd:int;
                                owl:onProperty   prov:dictionary
                              ];
        prov:category         "collections";
        prov:component        "collections";
        prov:constraints      "http://www.w3.org/TR/2013/NOTE-prov-dictionary-20130430/#dictionary-constraints"^^xsd:anyURI;
        prov:definition       "Removal is a derivation that transforms a dictionary into another, by removing one or more key-entity pairs.";
        prov:dm               "http://www.w3.org/TR/2013/NOTE-prov-dictionary-20130430/#term-dictionary-removal"^^xsd:anyURI;
        prov:n                "http://www.w3.org/TR/2013/NOTE-prov-dictionary-20130430/#expression-dictionary-removal"^^xsd:anyURI;
        prov:unqualifiedForm  prov:derivedByRemovalFrom .

prov:Insertion  rdf:type      owl:Class;
        rdfs:isDefinedBy      prov:;
        rdfs:label            "Insertion";
        rdfs:subClassOf       prov:Derivation;
        rdfs:subClassOf       [ rdf:type            owl:Restriction;
                                owl:minCardinality  "1"^^xsd:int;
                                owl:onProperty      prov:insertedKeyEntityPair
                              ];
        rdfs:subClassOf       [ rdf:type         owl:Restriction;
                                owl:cardinality  "1"^^xsd:int;
                                owl:onProperty   prov:dictionary
                              ];
        prov:category         "collections";
        prov:component        "collections";
        prov:constraints      "http://www.w3.org/TR/2013/NOTE-prov-dictionary-20130430/#dictionary-constraints"^^xsd:anyURI;
        prov:definition       "Insertion is a derivation that transforms a dictionary into another, by insertion of one or more key-entity pairs.";
        prov:dm               "http://www.w3.org/TR/2013/NOTE-prov-dictionary-20130430/#term-dictionary-insertion"^^xsd:anyURI;
        prov:n                "http://www.w3.org/TR/2013/NOTE-prov-dictionary-20130430/#expression-dictionary-insertion"^^xsd:anyURI;
        prov:unqualifiedForm  prov:derivedByInsertionFrom .

prov:KeyEntityPair  rdf:type  owl:Class;
        rdfs:isDefinedBy  prov:;
        rdfs:label        "Key-Entity Pair";
        rdfs:subClassOf   [ rdf:type         owl:Restriction;
                            owl:cardinality  "1"^^xsd:int;
                            owl:onProperty   prov:pairEntity
                          ];
        rdfs:subClassOf   [ rdf:type         owl:Restriction;
                            owl:cardinality  "1"^^xsd:int;
                            owl:onProperty   prov:pairKey
                          ];
        prov:category     "collections";
        prov:component    "collections";
        prov:constraints  "http://www.w3.org/TR/2013/NOTE-prov-dictionary-20130430/#dictionary-constraints"^^xsd:anyURI;
        prov:definition   "A key-entity pair. Part of a prov:Dictionary through prov:hadDictionaryMember. The key is any RDF Literal, the value is a prov:Entity.";
        prov:dm           "http://www.w3.org/TR/2013/NOTE-prov-dictionary-20130430/#term-dictionary-membership"^^xsd:anyURI;
        prov:n            "http://www.w3.org/TR/2013/NOTE-prov-dictionary-20130430/#expression-dictionary-membership"^^xsd:anyURI .

prov:EmptyDictionary  rdf:type  owl:Class;
        rdfs:isDefinedBy  prov:;
        rdfs:label        "Empty Dictionary";
        rdfs:subClassOf   prov:Dictionary , prov:EmptyCollection;
        prov:category     "collections";
        prov:component    "collections";
        prov:constraints  "http://www.w3.org/TR/2013/NOTE-prov-dictionary-20130430/#dictionary-constraints"^^xsd:anyURI;
        prov:definition   "An empty dictionary (i.e. has no members).";
        prov:dm           "http://www.w3.org/TR/2013/NOTE-prov-dictionary-20130430/#dictionary-conceptual-definition"^^xsd:anyURI;
        prov:n            "http://www.w3.org/TR/2013/NOTE-prov-dictionary-20130430/#expression-dictionary"^^xsd:anyURI .

prov:Dictionary  rdf:type  owl:Class;
        rdfs:comment      "A given dictionary forms a given structure for its members. A different structure (obtained either by insertion or removal of members) constitutes a different dictionary." , "This concept allows for the provenance of the dictionary, but also of its constituents to be expressed. Such a notion of dictionary corresponds to a wide variety of concrete data structures, such as a maps or associative arrays.";
        rdfs:isDefinedBy  prov:;
        rdfs:label        "Dictionary";
        prov:category     "collections";
        prov:component    "collections";
        prov:constraints  "http://www.w3.org/TR/2013/NOTE-prov-dictionary-20130430/#dictionary-constraints"^^xsd:anyURI;
        prov:definition   "A dictionary is an entity that provides a structure to some constituents, which are themselves entities. These constituents are said to be member of the dictionary.";
        prov:dm           "http://www.w3.org/TR/2013/NOTE-prov-dictionary-20130430/#dictionary-conceptual-definition"^^xsd:anyURI;
        prov:n            "http://www.w3.org/TR/2013/NOTE-prov-dictionary-20130430/#expression-dictionary"^^xsd:anyURI .

<http://www.w3.org/ns/prov-dictionary#>
        rdf:type      owl:Ontology;
        rdfs:comment  "This document is published by the Provenance Working Group (http://www.w3.org/2011/prov/wiki/Main_Page). \r\n\r\nIf you wish to make comments regarding this document, please send them to public-prov-comments@w3.org (subscribe public-prov-comments-request@w3.org, archives http://lists.w3.org/Archives/Public/public-prov-comments/). All feedback is welcome."@en;
        rdfs:label    "W3C PROVenance Interchange Ontology (PROV-O) Dictionary Extension"@en;
        rdfs:seeAlso  <http://www.w3.org/ns/prov> , <http://www.w3.org/TR/prov-dictionary/> .

prov:Submit  rdf:type    owl:Class;
        rdfs:label       "Submit"@en;
        rdfs:subClassOf  prov:Activity;
        prov:definition  "Activity that identifies the issuance (e.g., publication) of a resource. "@en .

prov:RightsHolder  rdf:type  owl:Class;
        rdfs:label       "RightsHolder"@en;
        rdfs:subClassOf  prov:Role;
        prov:definition  "Role with the function of owning or managing rights over a resource. The Agent assigned to this role is associated with a RightsAssignment Activity"@en .

prov:RightsAssignment
        rdf:type         owl:Class;
        rdfs:label       "RightsAssignment"@en;
        rdfs:subClassOf  prov:Activity;
        prov:definition  "Activity that identifies the rights assignment of a resource."@en .

prov:Replace  rdf:type   owl:Class;
        rdfs:label       "Replace"@en;
        rdfs:subClassOf  prov:Activity;
        prov:definition  "Activity that identifies the replacement of a resource."@en .

prov:Publisher  rdf:type  owl:Class;
        rdfs:label       "Publisher"@en;
        rdfs:subClassOf  prov:Role;
        prov:definition  "Role with the function of publishing a resource. The Agent assigned to this role is associated with a Publish Activity"@en .

prov:Publish  rdf:type   owl:Class;
        rdfs:label       "Publish"@en;
        rdfs:subClassOf  prov:Activity;
        prov:definition  "Activity that identifies the publication of a resource"@en .

prov:Modify  rdf:type    owl:Class;
        rdfs:label       "Modify"@en;
        rdfs:subClassOf  prov:Activity;
        prov:definition  "Activity that identifies the modification of a resource. "@en .

prov:Creator  rdf:type   owl:Class;
        rdfs:label       "Creator"@en;
        rdfs:subClassOf  prov:Contributor;
        prov:definition  "Role with the function of creating a resource. The Agent assigned to this role is associated with a Create Activity"@en .

prov:Create  rdf:type    owl:Class;
        rdfs:label       "Create"@en;
        rdfs:subClassOf  prov:Contribute;
        prov:definition  "Activity that identifies the creation of a resource"@en .

prov:Copyright  rdf:type  owl:Class;
        rdfs:label       "Copyright"@en;
        rdfs:subClassOf  prov:Activity;
        prov:definition  "Activity that identifies the Copyrighting activity associated to a resource."@en .

prov:Contributor  rdf:type  owl:Class;
        rdfs:label       "Contributor"@en;
        rdfs:subClassOf  prov:Role;
        prov:definition  "Role with the function of having responsibility for making contributions to a resource. The Agent assigned to this role is associated with a Modify or Create Activities"@en .

prov:Contribute  rdf:type  owl:Class;
        rdfs:label       "Contribute\n"@en;
        rdfs:subClassOf  prov:Activity;
        prov:definition  "Activity that identifies any contribution of an agent to a resource. "@en .

prov:Accept  rdf:type    owl:Class;
        rdfs:label       "Accept"@en;
        rdfs:subClassOf  prov:Activity;
        prov:definition  "Activity that identifies the acceptance of a resource (e.g., an article in a conference)"@en .

<http://www.w3.org/ns/prov-dc#>
        rdf:type      owl:Ontology;
        rdfs:comment  "This document is published by the Provenance Working Group (http://www.w3.org/2011/prov/wiki/Main_Page). \n\nIf you wish to make comments regarding this document, please send them to public-prov-comments@w3.org (subscribe public-prov-comments-request@w3.org, archives http://lists.w3.org/Archives/Public/public-prov-comments/). All feedback is welcome."@en;
        rdfs:label    "Dublin Core extensions of the W3C PROVenance Interchange Ontology (PROV-O) "@en;
        owl:imports   <http://www.w3.org/ns/prov-o#> .

owl:topObjectProperty
        rdf:type  owl:ObjectProperty .

prov:pingback  rdf:type   owl:ObjectProperty;
        rdfs:comment      "Relates a resource to a provenance pingback service that may receive additional provenance links about the resource."@en;
        rdfs:isDefinedBy  prov:;
        rdfs:label        "provenance pingback";
        prov:aq           "http://www.w3.org/TR/2013/NOTE-prov-aq-20130430/#provenance-pingback"^^xsd:anyURI;
        prov:category     "access-and-query" .

prov:provenanceUriTemplate
        rdf:type          owl:DatatypeProperty;
        rdfs:comment      "Relates a provenance service to a URI template string for constructing provenance-URIs."@en;
        rdfs:isDefinedBy  prov:;
        rdfs:label        "provenanceUriTemplate";
        prov:aq           "http://www.w3.org/TR/2013/NOTE-prov-aq-20130430/"^^xsd:anyURI;
        prov:category     "access-and-query" .

prov:describesService
        rdf:type          owl:ObjectProperty;
        rdfs:comment      "relates a generic provenance query service resource (type prov:ServiceDescription) to a specific query service description (e.g. a prov:DirectQueryService or a sd:Service)."@en;
        rdfs:isDefinedBy  prov:;
        rdfs:label        "describesService";
        prov:aq           "http://www.w3.org/TR/2013/NOTE-prov-aq-20130430/rovenance-query-service-description"^^xsd:anyURI;
        prov:category     "access-and-query";
        prov:inverse      "serviceDescribedBy" .

prov:has_query_service
        rdf:type          owl:ObjectProperty;
        rdfs:comment      "Indicates a provenance query service that can access provenance related to its subject or anchor resource."@en;
        rdfs:isDefinedBy  prov:;
        rdfs:label        "hasProvenanceService";
        prov:aq           "http://www.w3.org/TR/2013/NOTE-prov-aq-20130430/"^^xsd:anyURI;
        prov:category     "access-and-query";
        prov:inverse      "provenanceQueryServiceOf" .

prov:has_provenance  rdf:type  owl:ObjectProperty;
        rdfs:comment      "Indicates a provenance-URI for a resource; the resource identified by this property presents a provenance record about its subject or anchor resource."@en;
        rdfs:isDefinedBy  prov:;
        rdfs:label        "has_provenance";
        prov:aq           "http://www.w3.org/TR/2013/NOTE-prov-aq-20130430/#resource-represented-as-html"^^xsd:anyURI;
        prov:category     "access-and-query";
        prov:inverse      "provenanceOf" .

prov:has_anchor  rdf:type  owl:ObjectProperty;
        rdfs:comment      "Indicates anchor URI for a potentially dynamic resource instance."@en;
        rdfs:isDefinedBy  prov:;
        rdfs:label        "has_anchor";
        prov:aq           "http://www.w3.org/TR/2013/NOTE-prov-aq-20130430/#resource-represented-as-html"^^xsd:anyURI;
        prov:category     "access-and-query";
        prov:inverse      "anchorOf" .

prov:DirectQueryService
        rdf:type          owl:Class;
        rdfs:comment      "Type for a generic provenance query service. Mainly for use in RDF provenance query service descriptions, to facilitate discovery in linked data environments.";
        rdfs:isDefinedBy  prov:;
        rdfs:label        "ProvenanceService";
        rdfs:subClassOf   prov:SoftwareAgent;
        prov:aq           "http://www.w3.org/TR/2013/NOTE-prov-aq-20130430/#provenance-query-service-discovery"^^xsd:anyURI;
        prov:category     "access-and-query" .

prov:ServiceDescription
        rdf:type          owl:Class;
        rdfs:comment      "Type for a generic provenance query service. Mainly for use in RDF provenance query service descriptions, to facilitate discovery in linked data environments.";
        rdfs:isDefinedBy  prov:;
        rdfs:label        "ServiceDescription";
        rdfs:subClassOf   prov:SoftwareAgent;
        prov:aq           "http://www.w3.org/TR/2013/NOTE-prov-aq-20130430/#provenance-query-service-discovery"^^xsd:anyURI;
        prov:category     "access-and-query" .

<http://www.w3.org/ns/prov-aq#>
        rdf:type        owl:Ontology;
        rdfs:comment    "This document is published by the Provenance Working Group (http://www.w3.org/2011/prov/wiki/Main_Page). \n\nIf you wish to make comments regarding this document, please send them to public-prov-comments@w3.org (subscribe public-prov-comments-request@w3.org, archives http://lists.w3.org/Archives/Public/public-prov-comments/). All feedback is welcome."@en , "0.2";
        rdfs:label      "PROV Access and Query Ontology"@en;
        rdfs:seeAlso    <http://www.w3.org/TR/prov-aq/> , prov:;
        owl:versionIRI  <http://www.w3.org/TR/2013/NOTE-prov-aq-20130430/> .

prov:started  rdfs:isDefinedBy  <http://www.w3.org/ns/prov-o-inverses#>;
        rdfs:label        "started";
        owl:inverseOf     prov:wasStartedBy .

prov:hadRevision  rdfs:isDefinedBy  <http://www.w3.org/ns/prov-o-inverses#>;
        rdfs:label        "hadRevision";
        owl:inverseOf     prov:wasRevisionOf .

prov:quotedAs  rdfs:isDefinedBy  <http://www.w3.org/ns/prov-o-inverses#>;
        rdfs:label        "quotedAs";
        owl:inverseOf     prov:wasQuotedFrom .

prov:informed  rdfs:isDefinedBy  <http://www.w3.org/ns/prov-o-inverses#>;
        rdfs:label        "informed";
        owl:inverseOf     prov:wasInformedBy .

prov:ended  rdfs:isDefinedBy  <http://www.w3.org/ns/prov-o-inverses#>;
        rdfs:label        "ended";
        owl:inverseOf     prov:wasEndedBy .

prov:hadDerivation  rdfs:isDefinedBy  <http://www.w3.org/ns/prov-o-inverses#>;
        rdfs:label        "hadDerivation";
        owl:inverseOf     prov:wasDerivedFrom .

prov:contributed  rdfs:isDefinedBy  <http://www.w3.org/ns/prov-o-inverses#>;
        rdfs:label        "contributed";
        owl:inverseOf     prov:wasAttributedTo .

prov:wasAssociateFor  rdfs:isDefinedBy  <http://www.w3.org/ns/prov-o-inverses#>;
        rdfs:label        "wasAssociateFor";
        owl:inverseOf     prov:wasAssociatedWith .

prov:wasUsedBy  rdfs:isDefinedBy  <http://www.w3.org/ns/prov-o-inverses#>;
        rdfs:label        "wasUsedBy";
        owl:inverseOf     prov:used .

prov:generalizationOf
        rdfs:isDefinedBy  <http://www.w3.org/ns/prov-o-inverses#>;
        rdfs:label        "generalizationOf";
        owl:inverseOf     prov:specializationOf .

prov:qualifiedUsingActivity
        rdfs:isDefinedBy  <http://www.w3.org/ns/prov-o-inverses#>;
        rdfs:label        "qualifiedUsingActivity";
        owl:inverseOf     prov:qualifiedUsage .

prov:qualifiedStartOf
        rdfs:isDefinedBy  <http://www.w3.org/ns/prov-o-inverses#>;
        rdfs:label        "qualifiedStartOf";
        owl:inverseOf     prov:qualifiedStart .

prov:revisedEntity  rdfs:isDefinedBy  <http://www.w3.org/ns/prov-o-inverses#>;
        rdfs:label        "revisedEntity";
        owl:inverseOf     prov:qualifiedRevision .

prov:qualifiedQuotationOf
        rdfs:isDefinedBy  <http://www.w3.org/ns/prov-o-inverses#>;
        rdfs:label        "qualifiedQuotationOf";
        owl:inverseOf     prov:qualifiedQuotation .

prov:qualifiedSourceOf
        rdfs:isDefinedBy  <http://www.w3.org/ns/prov-o-inverses#>;
        rdfs:label        "qualifiedSourceOf";
        owl:inverseOf     prov:qualifiedPrimarySource .

prov:qualifiedInvalidationOf
        rdfs:isDefinedBy  <http://www.w3.org/ns/prov-o-inverses#>;
        rdfs:label        "qualifiedInvalidationOf";
        owl:inverseOf     prov:qualifiedInvalidation .

prov:qualifiedInfluenceOf
        rdfs:isDefinedBy  <http://www.w3.org/ns/prov-o-inverses#>;
        rdfs:label        "qualifiedInfluenceOf";
        owl:inverseOf     prov:qualifiedInfluence .

prov:qualifiedGenerationOf
        rdfs:isDefinedBy  <http://www.w3.org/ns/prov-o-inverses#>;
        rdfs:label        "qualifiedGenerationOf";
        owl:inverseOf     prov:qualifiedGeneration .

prov:qualifiedEndOf  rdfs:isDefinedBy  <http://www.w3.org/ns/prov-o-inverses#>;
        rdfs:label        "qualifiedEndOf";
        owl:inverseOf     prov:qualifiedEnd .

prov:qualifiedDerivationOf
        rdfs:isDefinedBy  <http://www.w3.org/ns/prov-o-inverses#>;
        rdfs:label        "qualifiedDerivationOf";
        owl:inverseOf     prov:qualifiedDerivation .

prov:qualifiedDelegationOf
        rdfs:isDefinedBy  <http://www.w3.org/ns/prov-o-inverses#>;
        rdfs:label        "qualifiedDelegationOf";
        owl:inverseOf     prov:qualifiedDelegation .

prov:qualifiedCommunicationOf
        rdfs:isDefinedBy  <http://www.w3.org/ns/prov-o-inverses#>;
        rdfs:label        "qualifiedCommunicationOf";
        owl:inverseOf     prov:qualifiedCommunication .

prov:qualifiedAttributionOf
        rdfs:isDefinedBy  <http://www.w3.org/ns/prov-o-inverses#>;
        rdfs:label        "qualifiedAttributionOf";
        owl:inverseOf     prov:qualifiedAttribution .

prov:qualifiedAssociationOf
        rdfs:isDefinedBy  <http://www.w3.org/ns/prov-o-inverses#>;
        rdfs:label        "qualifiedAssociationOf";
        owl:inverseOf     prov:qualifiedAssociation .

prov:hadInfluence  rdfs:isDefinedBy  <http://www.w3.org/ns/prov-o-inverses#>;
        rdfs:label        "hadInfluence";
        owl:inverseOf     prov:influencer .

prov:wasUsedInDerivation
        rdfs:isDefinedBy  <http://www.w3.org/ns/prov-o-inverses#>;
        rdfs:label        "wasUsedInDerivation";
        owl:inverseOf     prov:hadUsage .

prov:wasRoleIn  rdfs:isDefinedBy  <http://www.w3.org/ns/prov-o-inverses#>;
        rdfs:label        "wasRoleIn";
        owl:inverseOf     prov:hadRole .

prov:wasPrimarySourceOf
        rdfs:isDefinedBy  <http://www.w3.org/ns/prov-o-inverses#>;
        rdfs:label        "wasPrimarySourceOf";
        owl:inverseOf     prov:hadPrimarySource .

prov:wasPlanOf  rdfs:isDefinedBy  <http://www.w3.org/ns/prov-o-inverses#>;
        rdfs:label        "wasPlanOf";
        owl:inverseOf     prov:hadPlan .

prov:wasMemberOf  rdfs:isDefinedBy  <http://www.w3.org/ns/prov-o-inverses#>;
        rdfs:label        "wasMemberOf";
        owl:inverseOf     prov:hadMember .

prov:generatedAsDerivation
        rdfs:isDefinedBy  <http://www.w3.org/ns/prov-o-inverses#>;
        rdfs:label        "generatedAsDerivation";
        owl:inverseOf     prov:hadGeneration .

prov:wasActivityOfInfluence
        rdfs:isDefinedBy  <http://www.w3.org/ns/prov-o-inverses#>;
        rdfs:label        "wasActivityOfInfluence";
        owl:inverseOf     prov:hadActivity .

prov:entityOfInfluence
        rdfs:isDefinedBy  <http://www.w3.org/ns/prov-o-inverses#>;
        rdfs:label        "entityOfInfluence";
        owl:inverseOf     prov:entity .

prov:locationOf  rdfs:isDefinedBy  <http://www.w3.org/ns/prov-o-inverses#>;
        rdfs:label        "locationOf";
        owl:inverseOf     prov:atLocation .

prov:agentOfInfluence
        rdfs:isDefinedBy  <http://www.w3.org/ns/prov-o-inverses#>;
        rdfs:label        "agentOfInfluence";
        owl:inverseOf     prov:agent .

prov:activityOfInfluence
        rdfs:isDefinedBy  <http://www.w3.org/ns/prov-o-inverses#>;
        rdfs:label        "activityOfInfluence";
        owl:inverseOf     prov:activity .

prov:hadDelegate  rdfs:isDefinedBy  <http://www.w3.org/ns/prov-o-inverses#>;
        rdfs:label        "hadDelegate";
        owl:inverseOf     prov:actedOnBehalfOf .

<file:///tmp/sosa/prov.ttl#>
        rdf:type               owl:Ontology;
        rdfs:seeAlso           <http://www.w3.org/TR/prov-o/#names-of-inverse-properties>;
        owl:imports            <http://www.w3.org/ns/prov-o#>;
        owl:versionIRI         <http://www.w3.org/ns/prov-o-inverses-20130430>;
        prov:specializationOf  <http://www.w3.org/ns/prov-o-inverses>;
        prov:wasDerivedFrom    <http://www.w3.org/ns/prov-o-20130430>;
        prov:wasRevisionOf     <http://www.w3.org/ns/prov-o-inverses-20120312> .

[ rdf:type               owl:Axiom;
  rdfs:comment           "Revision is a derivation (see http://www.w3.org/TR/prov-dm/#term-Revision). Moreover, according to \nhttp://www.w3.org/TR/2013/REC-prov-constraints-20130430/#term-Revision 23 April 2012 'wasRevisionOf is a strict sub-relation of wasDerivedFrom since two entities e2 and e1 may satisfy wasDerivedFrom(e2,e1) without being a variant of each other.'";
  owl:annotatedProperty  rdfs:subPropertyOf;
  owl:annotatedSource    prov:wasRevisionOf;
  owl:annotatedTarget    prov:wasDerivedFrom
] .

[ rdf:type               owl:Axiom;
  rdfs:comment           "Quotation is a particular case of derivation (see http://www.w3.org/TR/prov-dm/#term-quotation) in which an entity is derived from an original entity by copying, or \"quoting\", some or all of it. ";
  owl:annotatedProperty  rdfs:subPropertyOf;
  owl:annotatedSource    prov:wasQuotedFrom;
  owl:annotatedTarget    prov:wasDerivedFrom
] .

[ rdf:type               owl:Axiom;
  owl:annotatedProperty  rdfs:domain;
  owl:annotatedSource    prov:wasInfluencedBy;
  owl:annotatedTarget    [ rdf:type     owl:Class;
                           owl:unionOf  ( prov:Activity prov:Agent prov:Entity )
                         ];
  prov:definition        "influencee: an identifier (o2) for an entity, activity, or agent; ";
  prov:dm                "http://www.w3.org/TR/2013/REC-prov-dm-20130430/#term-influence"
] .

[ rdf:type               owl:Axiom;
  owl:annotatedProperty  rdfs:range;
  owl:annotatedSource    prov:wasInfluencedBy;
  owl:annotatedTarget    [ rdf:type     owl:Class;
                           owl:unionOf  ( prov:Activity prov:Agent prov:Entity )
                         ];
  prov:definition        "influencer: an identifier (o1) for an ancestor entity, activity, or agent that the former depends on;";
  prov:dm                "http://www.w3.org/TR/2013/REC-prov-dm-20130430/#term-influence"
] .

[ rdf:type               owl:Axiom;
  rdfs:comment           "Derivation is a particular case of trace (see http://www.w3.org/TR/prov-dm/#term-trace), since it links an entity to another entity that contributed to its existence.";
  owl:annotatedProperty  rdfs:subPropertyOf;
  owl:annotatedSource    prov:wasDerivedFrom;
  owl:annotatedTarget    prov:wasInfluencedBy
] .

[ rdf:type               owl:Axiom;
  rdfs:comment           "Attribution is a particular case of trace (see http://www.w3.org/TR/prov-dm/#concept-trace), in the sense that it links an entity to the agent that ascribed it.";
  owl:annotatedProperty  rdfs:subPropertyOf;
  owl:annotatedSource    prov:wasAttributedTo;
  owl:annotatedTarget    prov:wasInfluencedBy;
  prov:definition        "IF wasAttributedTo(e2,ag1,aAttr) holds, THEN wasInfluencedBy(e2,ag1) also holds. "
] .

[ rdf:type               owl:Axiom;
  rdfs:comment           "hadPrimarySource property is a particular case of wasDerivedFrom (see http://www.w3.org/TR/prov-dm/#term-original-source) that aims to give credit to the source that originated some information.";
  owl:annotatedProperty  rdfs:subPropertyOf;
  owl:annotatedSource    prov:hadPrimarySource;
  owl:annotatedTarget    prov:wasDerivedFrom
] .

[ rdf:type               owl:Axiom;
  rdfs:comment           "A collection is an entity that provides a structure to some constituents, which are themselves entities. These constituents are said to be member of the collections."@en;
  owl:annotatedProperty  rdfs:range;
  owl:annotatedSource    prov:hadMember;
  owl:annotatedTarget    prov:Entity;
  prov:dm                "http://www.w3.org/TR/2013/REC-prov-dm-20130430/#term-collection"
] .

<http://www.w3.org/ns/prov-o#>
        rdf:type               owl:Ontology;
        rdfs:comment           "This document is published by the Provenance Working Group (http://www.w3.org/2011/prov/wiki/Main_Page). \n\nIf you wish to make comments regarding this document, please send them to public-prov-comments@w3.org (subscribe public-prov-comments-request@w3.org, archives http://lists.w3.org/Archives/Public/public-prov-comments/). All feedback is welcome."@en;
        rdfs:label             "W3C PROVenance Interchange Ontology (PROV-O)"@en;
        rdfs:seeAlso           <http://www.w3.org/ns/prov> , <http://www.w3.org/TR/prov-o/>;
        owl:versionIRI         <http://www.w3.org/ns/prov-o-20130430>;
        owl:versionInfo        "Recommendation version 2013-04-30"@en;
        prov:specializationOf  <http://www.w3.org/ns/prov-o>;
        prov:wasRevisionOf     <http://www.w3.org/ns/prov-o-20120312> .

prov:wasStartedBy  rdf:type     owl:ObjectProperty;
        rdfs:comment            "Start is when an activity is deemed to have started. A start may refer to an entity, known as trigger, that initiated the activity."@en;
        rdfs:domain             prov:Activity;
        rdfs:isDefinedBy        <http://www.w3.org/ns/prov-o#>;
        rdfs:label              "wasStartedBy";
        rdfs:range              prov:Entity;
        rdfs:subPropertyOf      prov:wasInfluencedBy;
        owl:propertyChainAxiom  ( prov:qualifiedStart prov:entity );
        prov:category           "expanded";
        prov:component          "entities-activities";
        prov:inverse            "started";
        prov:qualifiedForm      prov:qualifiedStart , prov:Start .

prov:wasRevisionOf  rdf:type    owl:ObjectProperty , owl:AnnotationProperty;
        rdfs:comment            "A revision is a derivation that revises an entity into a revised version."@en;
        rdfs:domain             prov:Entity;
        rdfs:isDefinedBy        <http://www.w3.org/ns/prov-o#>;
        rdfs:label              "wasRevisionOf";
        rdfs:range              prov:Entity;
        rdfs:subPropertyOf      prov:wasDerivedFrom;
        owl:propertyChainAxiom  ( prov:qualifiedRevision prov:entity );
        prov:category           "expanded";
        prov:component          "derivations";
        prov:inverse            "hadRevision";
        prov:qualifiedForm      prov:qualifiedRevision , prov:Revision .

prov:wasQuotedFrom  rdf:type    owl:ObjectProperty;
        rdfs:comment            "An entity is derived from an original entity by copying, or 'quoting', some or all of it."@en;
        rdfs:domain             prov:Entity;
        rdfs:isDefinedBy        <http://www.w3.org/ns/prov-o#>;
        rdfs:label              "wasQuotedFrom";
        rdfs:range              prov:Entity;
        rdfs:subPropertyOf      prov:wasDerivedFrom;
        owl:propertyChainAxiom  ( prov:qualifiedQuotation prov:entity );
        prov:category           "expanded";
        prov:component          "derivations";
        prov:inverse            "quotedAs";
        prov:qualifiedForm      prov:qualifiedQuotation , prov:Quotation .

prov:wasInvalidatedBy
        rdf:type                owl:ObjectProperty;
        rdfs:domain             prov:Entity;
        rdfs:isDefinedBy        <http://www.w3.org/ns/prov-o-inverses#> , <http://www.w3.org/ns/prov-o#>;
        rdfs:label              "wasInvalidatedBy";
        rdfs:range              prov:Activity;
        rdfs:subPropertyOf      prov:wasInfluencedBy;
        owl:inverseOf           prov:invalidated;
        owl:propertyChainAxiom  ( prov:qualifiedInvalidation prov:activity );
        prov:category           "expanded";
        prov:component          "entities-activities";
        prov:inverse            "invalidated";
        prov:qualifiedForm      prov:qualifiedInvalidation , prov:Invalidation .

prov:wasInformedBy  rdf:type    owl:ObjectProperty;
        rdfs:comment            "An activity a2 is dependent on or informed by another activity a1, by way of some unspecified entity that is generated by a1 and used by a2."@en;
        rdfs:domain             prov:Activity;
        rdfs:isDefinedBy        <http://www.w3.org/ns/prov-o#>;
        rdfs:label              "wasInformedBy";
        rdfs:range              prov:Activity;
        rdfs:subPropertyOf      prov:wasInfluencedBy;
        owl:propertyChainAxiom  ( prov:qualifiedCommunication prov:activity );
        prov:category           "starting-point";
        prov:component          "entities-activities";
        prov:inverse            "informed";
        prov:qualifiedForm      prov:qualifiedCommunication , prov:Communication .

prov:wasInfluencedBy  rdf:type     owl:ObjectProperty;
        rdfs:comment               "Because prov:wasInfluencedBy is a broad relation, its more specific subproperties (e.g. prov:wasInformedBy, prov:actedOnBehalfOf, prov:wasEndedBy, etc.) should be used when applicable."@en , "This property has multiple RDFS domains to suit multiple OWL Profiles. See <a href=\"#owl-profile\">PROV-O OWL Profile</a>.";
        rdfs:domain                [ rdf:type     owl:Class;
                                     owl:unionOf  ( prov:Activity prov:Agent prov:Entity )
                                   ];
        rdfs:isDefinedBy           <http://www.w3.org/ns/prov-o#> , <http://www.w3.org/ns/prov-o-inverses#>;
        rdfs:label                 "wasInfluencedBy";
        rdfs:range                 [ rdf:type     owl:Class;
                                     owl:unionOf  ( prov:Activity prov:Agent prov:Entity )
                                   ];
        owl:inverseOf              prov:influenced;
        prov:category              "qualified";
        prov:component             "agents-responsibility";
        prov:editorialNote         "The sub-properties of prov:wasInfluencedBy can be elaborated in more detail using the Qualification Pattern. For example, the binary relation :baking prov:used :spoon can be qualified by asserting :baking prov:qualifiedUsage [ a prov:Usage; prov:entity :spoon; prov:atLocation :kitchen ] .\n\nSubproperties of prov:wasInfluencedBy may also be asserted directly without being qualified.\n\nprov:wasInfluencedBy should not be used without also using one of its subproperties. \n"@en;
        prov:inverse               "influenced";
        prov:qualifiedForm         prov:Influence , prov:qualifiedInfluence;
        prov:sharesDefinitionWith  prov:Influence .

prov:wasGeneratedBy  rdf:type   owl:ObjectProperty;
        rdfs:domain             prov:Entity;
        rdfs:isDefinedBy        <http://www.w3.org/ns/prov-o-inverses#> , <http://www.w3.org/ns/prov-o#>;
        rdfs:label              "wasGeneratedBy";
        rdfs:range              prov:Activity;
        rdfs:subPropertyOf      prov:wasInfluencedBy;
        owl:inverseOf           prov:generated;
        owl:propertyChainAxiom  ( prov:qualifiedGeneration prov:activity );
        prov:category           "starting-point";
        prov:component          "entities-activities";
        prov:inverse            "generated";
        prov:qualifiedForm      prov:qualifiedGeneration , prov:Generation .

prov:wasEndedBy  rdf:type       owl:ObjectProperty;
        rdfs:comment            "End is when an activity is deemed to have ended. An end may refer to an entity, known as trigger, that terminated the activity."@en;
        rdfs:domain             prov:Activity;
        rdfs:isDefinedBy        <http://www.w3.org/ns/prov-o#>;
        rdfs:label              "wasEndedBy";
        rdfs:range              prov:Entity;
        rdfs:subPropertyOf      prov:wasInfluencedBy;
        owl:propertyChainAxiom  ( prov:qualifiedEnd prov:entity );
        prov:category           "expanded";
        prov:component          "entities-activities";
        prov:inverse            "ended";
        prov:qualifiedForm      prov:qualifiedEnd , prov:End .

prov:wasDerivedFrom  rdf:type   owl:ObjectProperty;
        rdfs:comment            "The more specific subproperties of prov:wasDerivedFrom (i.e., prov:wasQuotedFrom, prov:wasRevisionOf, prov:hadPrimarySource) should be used when applicable."@en;
        rdfs:domain             prov:Entity;
        rdfs:isDefinedBy        <http://www.w3.org/ns/prov-o#>;
        rdfs:label              "wasDerivedFrom";
        rdfs:range              prov:Entity;
        rdfs:subPropertyOf      prov:wasInfluencedBy;
        owl:propertyChainAxiom  ( prov:qualifiedDerivation prov:entity );
        prov:category           "starting-point";
        prov:component          "derivations";
        prov:definition         "A derivation is a transformation of an entity into another, an update of an entity resulting in a new one, or the construction of a new entity based on a pre-existing entity."@en;
        prov:inverse            "hadDerivation";
        prov:qualifiedForm      prov:qualifiedDerivation , prov:Derivation .

prov:wasAttributedTo  rdf:type  owl:ObjectProperty;
        rdfs:comment            "Attribution is the ascribing of an entity to an agent."@en;
        rdfs:domain             prov:Entity;
        rdfs:isDefinedBy        <http://www.w3.org/ns/prov-o#>;
        rdfs:label              "wasAttributedTo";
        rdfs:range              prov:Agent;
        rdfs:subPropertyOf      prov:wasInfluencedBy;
        owl:propertyChainAxiom  ( prov:qualifiedAttribution prov:agent );
        prov:category           "starting-point";
        prov:component          "agents-responsibility";
        prov:definition         "Attribution is the ascribing of an entity to an agent."@en;
        prov:inverse            "contributed";
        prov:qualifiedForm      prov:qualifiedAttribution , prov:Attribution .

prov:wasAssociatedWith
        rdf:type                owl:ObjectProperty;
        rdfs:comment            "An prov:Agent that had some (unspecified) responsibility for the occurrence of this prov:Activity."@en;
        rdfs:domain             prov:Activity;
        rdfs:isDefinedBy        <http://www.w3.org/ns/prov-o#>;
        rdfs:label              "wasAssociatedWith";
        rdfs:range              prov:Agent;
        rdfs:subPropertyOf      prov:wasInfluencedBy;
        owl:propertyChainAxiom  ( prov:qualifiedAssociation prov:agent );
        prov:category           "starting-point";
        prov:component          "agents-responsibility";
        prov:inverse            "wasAssociateFor";
        prov:qualifiedForm      prov:qualifiedAssociation , prov:Association .

prov:value  rdf:type        owl:DatatypeProperty;
        rdfs:domain         prov:Entity;
        rdfs:isDefinedBy    <http://www.w3.org/ns/prov-o#>;
        rdfs:label          "value";
        prov:category       "expanded";
        prov:component      "entities-activities";
        prov:definition     "Provides a value that is a direct representation of an entity."@en;
        prov:dm             "http://www.w3.org/TR/2013/REC-prov-dm-20130430/#term-attribute-value"^^xsd:anyURI;
        prov:editorialNote  "This property serves the same purpose as rdf:value, but has been reintroduced to avoid some of the definitional ambiguity in the RDF specification (specifically, 'may be used in describing structured values')."@en , "The editor's definition comes from http://www.w3.org/TR/rdf-primer/#rdfvalue" .

prov:used  rdf:type             owl:ObjectProperty;
        rdfs:comment            "A prov:Entity that was used by this prov:Activity. For example, :baking prov:used :spoon, :egg, :oven ."@en;
        rdfs:domain             prov:Activity;
        rdfs:isDefinedBy        <http://www.w3.org/ns/prov-o#>;
        rdfs:label              "used";
        rdfs:range              prov:Entity;
        rdfs:subPropertyOf      prov:wasInfluencedBy;
        owl:propertyChainAxiom  ( prov:qualifiedUsage prov:entity );
        prov:category           "starting-point";
        prov:component          "entities-activities";
        prov:inverse            "wasUsedBy";
        prov:qualifiedForm      prov:qualifiedUsage , prov:Usage .

prov:unqualifiedForm  rdf:type  owl:AnnotationProperty;
        rdfs:comment        "Classes and properties used to qualify relationships are annotated with prov:unqualifiedForm to indicate the property used to assert an unqualified provenance relation."@en;
        rdfs:isDefinedBy    prov: , <http://www.w3.org/ns/prov-o#>;
        rdfs:subPropertyOf  rdfs:seeAlso .

prov:todo  rdf:type  owl:AnnotationProperty .

prov:startedAtTime  rdf:type  owl:DatatypeProperty;
        rdfs:comment        "The time at which an activity started. See also prov:endedAtTime."@en;
        rdfs:domain         prov:Activity;
        rdfs:isDefinedBy    <http://www.w3.org/ns/prov-o#>;
        rdfs:label          "startedAtTime";
        rdfs:range          xsd:dateTime;
        prov:category       "starting-point";
        prov:component      "entities-activities";
        prov:editorialNote  "It is the intent that the property chain holds: (prov:qualifiedStart o prov:atTime) rdfs:subPropertyOf prov:startedAtTime."@en;
        prov:qualifiedForm  prov:atTime , prov:Start .

prov:specializationOf
        rdf:type            owl:AnnotationProperty , owl:ObjectProperty;
        rdfs:domain         prov:Entity;
        rdfs:isDefinedBy    <http://www.w3.org/ns/prov-o#> , prov:;
        rdfs:label          "specializationOf";
        rdfs:range          prov:Entity;
        rdfs:seeAlso        prov:alternateOf;
        rdfs:subPropertyOf  owl:topObjectProperty , prov:alternateOf;
        prov:category       "expanded";
        prov:component      "alternate";
        prov:constraints    "http://www.w3.org/TR/2012/WD-prov-dm-20120703/prov-constraints.html#prov-dm-constraints-fig"^^xsd:anyURI , "http://www.w3.org/TR/2013/REC-prov-constraints-20130430/#prov-dm-constraints-fig"^^xsd:anyURI;
        prov:definition     "An entity that is a specialization of another shares all aspects of the latter, and additionally presents more specific aspects of the same thing as the latter. In particular, the lifetime of the entity being specialized contains that of any specialization. Examples of aspects include a time period, an abstraction, and a context associated with the entity."@en;
        prov:dm             "http://www.w3.org/TR/2012/WD-prov-dm-20120703/prov-dm.html#term-specialization"^^xsd:anyURI , "http://www.w3.org/TR/2013/REC-prov-dm-20130430/#term-specialization"^^xsd:anyURI;
        prov:inverse        "generalizationOf";
        prov:n              "http://www.w3.org/TR/2012/WD-prov-dm-20120703/prov-n.html#expression-specialization"^^xsd:anyURI , "http://www.w3.org/TR/2013/REC-prov-n-20130430/#expression-specialization"^^xsd:anyURI .

prov:sharesDefinitionWith
        rdf:type            owl:AnnotationProperty;
        rdfs:isDefinedBy    prov: , <http://www.w3.org/ns/prov-o#>;
        rdfs:subPropertyOf  rdfs:seeAlso .

prov:qualifiedUsage  rdf:type      owl:ObjectProperty;
        rdfs:comment               "If this Activity prov:used Entity :e, then it can qualify how it used it using prov:qualifiedUsage [ a prov:Usage; prov:entity :e; :foo :bar ]."@en;
        rdfs:domain                prov:Activity;
        rdfs:isDefinedBy           <http://www.w3.org/ns/prov-o#>;
        rdfs:label                 "qualifiedUsage";
        rdfs:range                 prov:Usage;
        rdfs:subPropertyOf         prov:qualifiedInfluence;
        prov:category              "qualified";
        prov:component             "entities-activities";
        prov:inverse               "qualifiedUsingActivity";
        prov:sharesDefinitionWith  prov:Usage;
        prov:unqualifiedForm       prov:used .

prov:qualifiedStart  rdf:type      owl:ObjectProperty;
        rdfs:comment               "If this Activity prov:wasStartedBy Entity :e1, then it can qualify how it was started using prov:qualifiedStart [ a prov:Start;  prov:entity :e1; :foo :bar ]."@en;
        rdfs:domain                prov:Activity;
        rdfs:isDefinedBy           <http://www.w3.org/ns/prov-o#>;
        rdfs:label                 "qualifiedStart";
        rdfs:range                 prov:Start;
        rdfs:subPropertyOf         prov:qualifiedInfluence;
        prov:category              "qualified";
        prov:component             "entities-activities";
        prov:inverse               "qualifiedStartOf";
        prov:sharesDefinitionWith  prov:Start;
        prov:unqualifiedForm       prov:wasStartedBy .

prov:qualifiedRevision
        rdf:type                   owl:ObjectProperty;
        rdfs:comment               "If this Entity prov:wasRevisionOf Entity :e, then it can qualify how it was revised using prov:qualifiedRevision [ a prov:Revision;  prov:entity :e; :foo :bar ]."@en;
        rdfs:domain                prov:Entity;
        rdfs:isDefinedBy           <http://www.w3.org/ns/prov-o#>;
        rdfs:label                 "qualifiedRevision";
        rdfs:range                 prov:Revision;
        rdfs:subPropertyOf         prov:qualifiedInfluence;
        prov:category              "qualified";
        prov:component             "derivations";
        prov:inverse               "revisedEntity";
        prov:sharesDefinitionWith  prov:Revision;
        prov:unqualifiedForm       prov:wasRevisionOf .

prov:qualifiedQuotation
        rdf:type                   owl:ObjectProperty;
        rdfs:comment               "If this Entity prov:wasQuotedFrom Entity :e, then it can qualify how using prov:qualifiedQuotation [ a prov:Quotation;  prov:entity :e; :foo :bar ]."@en;
        rdfs:domain                prov:Entity;
        rdfs:isDefinedBy           <http://www.w3.org/ns/prov-o#>;
        rdfs:label                 "qualifiedQuotation";
        rdfs:range                 prov:Quotation;
        rdfs:subPropertyOf         prov:qualifiedInfluence;
        prov:category              "qualified";
        prov:component             "derivations";
        prov:inverse               "qualifiedQuotationOf";
        prov:sharesDefinitionWith  prov:Quotation;
        prov:unqualifiedForm       prov:wasQuotedFrom .

prov:qualifiedPrimarySource
        rdf:type                   owl:ObjectProperty;
        rdfs:comment               "If this Entity prov:hadPrimarySource Entity :e, then it can qualify how using prov:qualifiedPrimarySource [ a prov:PrimarySource; prov:entity :e; :foo :bar ]."@en;
        rdfs:domain                prov:Entity;
        rdfs:isDefinedBy           <http://www.w3.org/ns/prov-o#>;
        rdfs:label                 "qualifiedPrimarySource";
        rdfs:range                 prov:PrimarySource;
        rdfs:subPropertyOf         prov:qualifiedInfluence;
        prov:category              "qualified";
        prov:component             "derivations";
        prov:inverse               "qualifiedSourceOf";
        prov:sharesDefinitionWith  prov:PrimarySource;
        prov:unqualifiedForm       prov:hadPrimarySource .

prov:qualifiedInvalidation
        rdf:type                   owl:ObjectProperty;
        rdfs:comment               "If this Entity prov:wasInvalidatedBy Activity :a, then it can qualify how it was invalidated using prov:qualifiedInvalidation [ a prov:Invalidation;  prov:activity :a; :foo :bar ]."@en;
        rdfs:domain                prov:Entity;
        rdfs:isDefinedBy           <http://www.w3.org/ns/prov-o#>;
        rdfs:label                 "qualifiedInvalidation";
        rdfs:range                 prov:Invalidation;
        rdfs:subPropertyOf         prov:qualifiedInfluence;
        prov:category              "qualified";
        prov:component             "entities-activities";
        prov:inverse               "qualifiedInvalidationOf";
        prov:sharesDefinitionWith  prov:Invalidation;
        prov:unqualifiedForm       prov:wasInvalidatedBy .

prov:qualifiedInfluence
        rdf:type                   owl:ObjectProperty;
        rdfs:comment               "Because prov:qualifiedInfluence is a broad relation, the more specific relations (qualifiedCommunication, qualifiedDelegation, qualifiedEnd, etc.) should be used when applicable."@en;
        rdfs:domain                [ rdf:type     owl:Class;
                                     owl:unionOf  ( prov:Activity prov:Agent prov:Entity )
                                   ];
        rdfs:isDefinedBy           <http://www.w3.org/ns/prov-o#>;
        rdfs:label                 "qualifiedInfluence";
        rdfs:range                 prov:Influence;
        prov:category              "qualified";
        prov:component             "derivations";
        prov:inverse               "qualifiedInfluenceOf";
        prov:sharesDefinitionWith  prov:Influence;
        prov:unqualifiedForm       prov:wasInfluencedBy .

prov:qualifiedGeneration
        rdf:type                   owl:ObjectProperty;
        rdfs:comment               "If this Activity prov:generated Entity :e, then it can qualify how it performed the Generation using prov:qualifiedGeneration [ a prov:Generation;  prov:entity :e; :foo :bar ]."@en;
        rdfs:domain                prov:Entity;
        rdfs:isDefinedBy           <http://www.w3.org/ns/prov-o#>;
        rdfs:label                 "qualifiedGeneration";
        rdfs:range                 prov:Generation;
        rdfs:subPropertyOf         prov:qualifiedInfluence;
        prov:category              "qualified";
        prov:component             "entities-activities";
        prov:inverse               "qualifiedGenerationOf";
        prov:sharesDefinitionWith  prov:Generation;
        prov:unqualifiedForm       prov:wasGeneratedBy .

prov:qualifiedForm  rdf:type  owl:AnnotationProperty;
        rdfs:comment        "This annotation property links a subproperty of prov:wasInfluencedBy with the subclass of prov:Influence and the qualifying property that are used to qualify it. \n\nExample annotation:\n\n    prov:wasGeneratedBy prov:qualifiedForm prov:qualifiedGeneration, prov:Generation .\n\nThen this unqualified assertion:\n\n    :entity1 prov:wasGeneratedBy :activity1 .\n\ncan be qualified by adding:\n\n   :entity1 prov:qualifiedGeneration :entity1Gen .\n   :entity1Gen \n       a prov:Generation, prov:Influence;\n       prov:activity :activity1;\n       :customValue 1337 .\n\nNote how the value of the unqualified influence (prov:wasGeneratedBy :activity1) is mirrored as the value of the prov:activity (or prov:entity, or prov:agent) property on the influence class."@en;
        rdfs:isDefinedBy    prov: , <http://www.w3.org/ns/prov-o#>;
        rdfs:subPropertyOf  rdfs:seeAlso .

prov:qualifiedEnd  rdf:type        owl:ObjectProperty;
        rdfs:comment               "If this Activity prov:wasEndedBy Entity :e1, then it can qualify how it was ended using prov:qualifiedEnd [ a prov:End;  prov:entity :e1; :foo :bar ]."@en;
        rdfs:domain                prov:Activity;
        rdfs:isDefinedBy           <http://www.w3.org/ns/prov-o#>;
        rdfs:label                 "qualifiedEnd";
        rdfs:range                 prov:End;
        rdfs:subPropertyOf         prov:qualifiedInfluence;
        prov:category              "qualified";
        prov:component             "entities-activities";
        prov:inverse               "qualifiedEndOf";
        prov:sharesDefinitionWith  prov:End;
        prov:unqualifiedForm       prov:wasEndedBy .

prov:qualifiedDerivation
        rdf:type                   owl:ObjectProperty;
        rdfs:comment               "If this Entity prov:wasDerivedFrom Entity :e, then it can qualify how it was derived using prov:qualifiedDerivation [ a prov:Derivation;  prov:entity :e; :foo :bar ]."@en;
        rdfs:domain                prov:Entity;
        rdfs:isDefinedBy           <http://www.w3.org/ns/prov-o#>;
        rdfs:label                 "qualifiedDerivation";
        rdfs:range                 prov:Derivation;
        rdfs:subPropertyOf         prov:qualifiedInfluence;
        prov:category              "qualified";
        prov:component             "derivations";
        prov:inverse               "qualifiedDerivationOf";
        prov:sharesDefinitionWith  prov:Derivation;
        prov:unqualifiedForm       prov:wasDerivedFrom .

prov:qualifiedDelegation
        rdf:type                   owl:ObjectProperty;
        rdfs:comment               "If this Agent prov:actedOnBehalfOf Agent :ag, then it can qualify how with prov:qualifiedResponsibility [ a prov:Responsibility;  prov:agent :ag; :foo :bar ]."@en;
        rdfs:domain                prov:Agent;
        rdfs:isDefinedBy           <http://www.w3.org/ns/prov-o#>;
        rdfs:label                 "qualifiedDelegation";
        rdfs:range                 prov:Delegation;
        rdfs:subPropertyOf         prov:qualifiedInfluence;
        prov:category              "qualified";
        prov:component             "agents-responsibility";
        prov:inverse               "qualifiedDelegationOf";
        prov:sharesDefinitionWith  prov:Delegation;
        prov:unqualifiedForm       prov:actedOnBehalfOf .

prov:qualifiedCommunication
        rdf:type                   owl:ObjectProperty;
        rdfs:comment               "If this Activity prov:wasInformedBy Activity :a, then it can qualify how it was influenced using prov:qualifiedCommunication [ a prov:Communication;  prov:activity :a; :foo :bar ]."@en;
        rdfs:domain                prov:Activity;
        rdfs:isDefinedBy           <http://www.w3.org/ns/prov-o#>;
        rdfs:label                 "qualifiedCommunication";
        rdfs:range                 prov:Communication;
        rdfs:subPropertyOf         prov:qualifiedInfluence;
        prov:category              "qualified";
        prov:component             "entities-activities";
        prov:inverse               "qualifiedCommunicationOf";
        prov:qualifiedForm         prov:Communication;
        prov:sharesDefinitionWith  prov:Communication .

prov:qualifiedAttribution
        rdf:type                   owl:ObjectProperty;
        rdfs:comment               "If this Entity prov:wasAttributedTo Agent :ag, then it can qualify how it was influenced using prov:qualifiedAttribution [ a prov:Attribution;  prov:agent :ag; :foo :bar ]."@en;
        rdfs:domain                prov:Entity;
        rdfs:isDefinedBy           <http://www.w3.org/ns/prov-o#>;
        rdfs:label                 "qualifiedAttribution";
        rdfs:range                 prov:Attribution;
        rdfs:subPropertyOf         prov:qualifiedInfluence;
        prov:category              "qualified";
        prov:component             "agents-responsibility";
        prov:inverse               "qualifiedAttributionOf";
        prov:sharesDefinitionWith  prov:Attribution;
        prov:unqualifiedForm       prov:wasAttributedTo .

prov:qualifiedAssociation
        rdf:type                   owl:ObjectProperty;
        rdfs:comment               "If this Activity prov:wasAssociatedWith Agent :ag, then it can qualify the Association using prov:qualifiedAssociation [ a prov:Association;  prov:agent :ag; :foo :bar ]."@en;
        rdfs:domain                prov:Activity;
        rdfs:isDefinedBy           <http://www.w3.org/ns/prov-o#>;
        rdfs:label                 "qualifiedAssociation";
        rdfs:range                 prov:Association;
        rdfs:subPropertyOf         prov:qualifiedInfluence;
        prov:category              "qualified";
        prov:component             "agents-responsibility";
        prov:inverse               "qualifiedAssociationOf";
        prov:sharesDefinitionWith  prov:Association;
        prov:unqualifiedForm       prov:wasAssociatedWith .

prov:order  rdf:type      owl:AnnotationProperty;
        rdfs:comment      "The position that this OWL term should be listed within documentation. The scope of the documentation (e.g., among all terms, among terms within a prov:category, among properties applying to a particular class, etc.) is unspecified."@en;
        rdfs:isDefinedBy  <http://www.w3.org/ns/prov-o#> .

prov:n  rdf:type            owl:AnnotationProperty;
        rdfs:comment        "A reference to the principal section of the PROV-M document that describes this concept."@en , "A reference to the principal section of the PROV-DM document that describes this concept."@en;
        rdfs:isDefinedBy    prov: , <http://www.w3.org/ns/prov-o#>;
        rdfs:subPropertyOf  rdfs:seeAlso .

prov:inverse  rdf:type    owl:AnnotationProperty;
        rdfs:comment      "PROV-O does not define all property inverses. The directionalities defined in PROV-O should be given preference over those not defined. However, if users wish to name the inverse of a PROV-O property, the local name given by prov:inverse should be used."@en;
        rdfs:isDefinedBy  prov: , <http://www.w3.org/ns/prov-o#>;
        rdfs:seeAlso      <http://www.w3.org/TR/prov-o/#names-of-inverse-properties> .

prov:invalidatedAtTime
        rdf:type            owl:DatatypeProperty;
        rdfs:comment        "The time at which an entity was invalidated (i.e., no longer usable)."@en;
        rdfs:domain         prov:Entity;
        rdfs:isDefinedBy    <http://www.w3.org/ns/prov-o#>;
        rdfs:label          "invalidatedAtTime";
        rdfs:range          xsd:dateTime;
        prov:category       "expanded";
        prov:component      "entities-activities";
        prov:editorialNote  "It is the intent that the property chain holds: (prov:qualifiedInvalidation o prov:atTime) rdfs:subPropertyOf prov:invalidatedAtTime."@en;
        prov:qualifiedForm  prov:atTime , prov:Invalidation .

prov:invalidated  rdf:type         owl:ObjectProperty;
        rdfs:domain                prov:Activity;
        rdfs:isDefinedBy           <http://www.w3.org/ns/prov-o-inverses#> , <http://www.w3.org/ns/prov-o#>;
        rdfs:label                 "invalidated";
        rdfs:range                 prov:Entity;
        rdfs:subPropertyOf         prov:influenced;
        owl:inverseOf              prov:wasInvalidatedBy;
        prov:category              "expanded";
        prov:component             "entities-activities";
        prov:editorialNote         "prov:invalidated is one of few inverse property defined, to allow Activity-oriented assertions in addition to Entity-oriented assertions."@en;
        prov:inverse               "wasInvalidatedBy";
        prov:sharesDefinitionWith  prov:Invalidation .

prov:influencer  rdf:type       owl:ObjectProperty;
        rdfs:comment            "Subproperties of prov:influencer are used to cite the object of an unqualified PROV-O triple whose predicate is a subproperty of prov:wasInfluencedBy (e.g. prov:used, prov:wasGeneratedBy). prov:influencer is used much like rdf:object is used."@en;
        rdfs:domain             prov:Influence;
        rdfs:isDefinedBy        <http://www.w3.org/ns/prov-o#>;
        rdfs:label              "influencer";
        rdfs:range              owl:Thing;
        prov:category           "qualified";
        prov:dm                 "http://www.w3.org/TR/2013/REC-prov-dm-20130430/#term-influence"^^xsd:anyURI;
        prov:editorialNote      "This property and its subproperties are used in the same way as the rdf:object property, i.e. to reference the object of an unqualified prov:wasInfluencedBy or prov:influenced triple."@en;
        prov:editorsDefinition  "This property is used as part of the qualified influence pattern. Subclasses of prov:Influence use these subproperties to reference the resource (Entity, Agent, or Activity) whose influence is being qualified."@en;
        prov:inverse            "hadInfluence" .

prov:influenced  rdf:type          owl:ObjectProperty;
        rdfs:isDefinedBy           <http://www.w3.org/ns/prov-o-inverses#> , <http://www.w3.org/ns/prov-o#>;
        rdfs:label                 "influenced";
        owl:inverseOf              prov:wasInfluencedBy;
        prov:category              "expanded";
        prov:component             "agents-responsibility";
        prov:inverse               "wasInfluencedBy";
        prov:sharesDefinitionWith  prov:Influence .

prov:hadUsage  rdf:type            owl:ObjectProperty;
        rdfs:comment               "The _optional_ Usage involved in an Entity's Derivation."@en;
        rdfs:domain                prov:Derivation;
        rdfs:isDefinedBy           prov: , <http://www.w3.org/ns/prov-o#>;
        rdfs:label                 "hadUsage";
        rdfs:range                 prov:Usage;
        prov:category              "qualified";
        prov:component             "derivations";
        prov:inverse               "wasUsedInDerivation";
        prov:sharesDefinitionWith  prov:Usage .

prov:hadRole  rdf:type             owl:ObjectProperty;
        rdfs:comment               "This property has multiple RDFS domains to suit multiple OWL Profiles. See <a href=\"#owl-profile\">PROV-O OWL Profile</a>." , "The _optional_ Role that an Entity assumed in the context of an Activity. For example, :baking prov:used :spoon; prov:qualified [ a prov:Usage; prov:entity :spoon; prov:hadRole roles:mixing_implement ]."@en;
        rdfs:domain                prov:Influence;
        rdfs:domain                [ rdf:type     owl:Class;
                                     owl:unionOf  ( prov:Association prov:InstantaneousEvent )
                                   ];
        rdfs:isDefinedBy           <http://www.w3.org/ns/prov-o#>;
        rdfs:label                 "hadRole";
        rdfs:range                 prov:Role;
        prov:category              "qualified";
        prov:component             "agents-responsibility";
        prov:editorsDefinition     "prov:hadRole references the Role (i.e. the function of an entity with respect to an activity), in the context of an instantaneous usage, generation, association, start, and end."@en;
        prov:inverse               "wasRoleIn";
        prov:sharesDefinitionWith  prov:Role .

prov:hadPrimarySource
        rdf:type                owl:ObjectProperty;
        rdfs:domain             prov:Entity;
        rdfs:isDefinedBy        <http://www.w3.org/ns/prov-o#>;
        rdfs:label              "hadPrimarySource";
        rdfs:range              prov:Entity;
        rdfs:subPropertyOf      prov:wasDerivedFrom;
        owl:propertyChainAxiom  ( prov:qualifiedPrimarySource prov:entity );
        prov:category           "expanded";
        prov:component          "derivations";
        prov:inverse            "wasPrimarySourceOf";
        prov:qualifiedForm      prov:qualifiedPrimarySource , prov:PrimarySource .

prov:hadPlan  rdf:type             owl:ObjectProperty;
        rdfs:comment               "The _optional_ Plan adopted by an Agent in Association with some Activity. Plan specifications are out of the scope of this specification."@en;
        rdfs:domain                prov:Association;
        rdfs:isDefinedBy           <http://www.w3.org/ns/prov-o#>;
        rdfs:label                 "hadPlan";
        rdfs:range                 prov:Plan;
        prov:category              "qualified";
        prov:component             "agents-responsibility";
        prov:inverse               "wasPlanOf";
        prov:sharesDefinitionWith  prov:Plan .

prov:hadMember  rdf:type           owl:ObjectProperty;
        rdfs:domain                prov:Collection;
        rdfs:isDefinedBy           <http://www.w3.org/ns/prov-o#>;
        rdfs:label                 "hadMember";
        rdfs:range                 prov:Entity;
        rdfs:subPropertyOf         prov:wasInfluencedBy;
        prov:category              "expanded";
        prov:component             "expanded";
        prov:inverse               "wasMemberOf";
        prov:sharesDefinitionWith  prov:Collection .

prov:hadGeneration  rdf:type       owl:ObjectProperty;
        rdfs:comment               "The _optional_ Generation involved in an Entity's Derivation."@en;
        rdfs:domain                prov:Derivation;
        rdfs:isDefinedBy           <http://www.w3.org/ns/prov-o#>;
        rdfs:label                 "hadGeneration";
        rdfs:range                 prov:Generation;
        prov:category              "qualified";
        prov:component             "derivations";
        prov:inverse               "generatedAsDerivation";
        prov:sharesDefinitionWith  prov:Generation .

prov:hadActivity  rdf:type         owl:ObjectProperty;
        rdfs:comment               "This property has multiple RDFS domains to suit multiple OWL Profiles. See <a href=\"#owl-profile\">PROV-O OWL Profile</a>." , "The _optional_ Activity of an Influence, which used, generated, invalidated, or was the responsibility of some Entity. This property is _not_ used by ActivityInfluence (use prov:activity instead)."@en;
        rdfs:domain                prov:Influence;
        rdfs:domain                [ rdf:type     owl:Class;
                                     owl:unionOf  ( prov:Delegation prov:Derivation prov:End prov:Start )
                                   ];
        rdfs:isDefinedBy           <http://www.w3.org/ns/prov-o#>;
        rdfs:label                 "hadActivity";
        rdfs:range                 prov:Activity;
        prov:category              "qualified";
        prov:component             "derivations";
        prov:editorialNote         "The multiple rdfs:domain assertions are intended. One is simpler and works for OWL-RL, the union is more specific but is not recognized by OWL-RL."@en;
        prov:inverse               "wasActivityOfInfluence";
        prov:sharesDefinitionWith  prov:Activity .

prov:generatedAtTime  rdf:type  owl:DatatypeProperty;
        rdfs:comment        "The time at which an entity was completely created and is available for use."@en;
        rdfs:domain         prov:Entity;
        rdfs:isDefinedBy    <http://www.w3.org/ns/prov-o#>;
        rdfs:label          "generatedAtTime";
        rdfs:range          xsd:dateTime;
        prov:category       "expanded";
        prov:component      "entities-activities";
        prov:editorialNote  "It is the intent that the property chain holds: (prov:qualifiedGeneration o prov:atTime) rdfs:subPropertyOf prov:generatedAtTime."@en;
        prov:qualifiedForm  prov:atTime , prov:Generation .

prov:generated  rdf:type           owl:ObjectProperty;
        rdfs:domain                prov:Activity;
        rdfs:isDefinedBy           <http://www.w3.org/ns/prov-o-inverses#> , <http://www.w3.org/ns/prov-o#>;
        rdfs:label                 "generated";
        rdfs:range                 prov:Entity;
        rdfs:subPropertyOf         prov:influenced;
        owl:inverseOf              prov:wasGeneratedBy;
        prov:category              "expanded";
        prov:component             "entities-activities";
        prov:editorialNote         "prov:generated is one of few inverse property defined, to allow Activity-oriented assertions in addition to Entity-oriented assertions."@en;
        prov:inverse               "wasGeneratedBy";
        prov:sharesDefinitionWith  prov:Generation .

prov:entity  rdf:type           owl:ObjectProperty;
        rdfs:domain             prov:EntityInfluence;
        rdfs:isDefinedBy        <http://www.w3.org/ns/prov-o#>;
        rdfs:label              "entity";
        rdfs:range              prov:Entity;
        rdfs:subPropertyOf      prov:influencer;
        prov:category           "qualified";
        prov:editorialNote      "This property behaves in spirit like rdf:object; it references the object of a prov:wasInfluencedBy triple."@en;
        prov:editorsDefinition  "The prov:entity property references an prov:Entity which influenced a resource. This property applies to an prov:EntityInfluence, which is given by a subproperty of prov:qualifiedInfluence from the influenced prov:Entity, prov:Activity or prov:Agent.";
        prov:inverse            "entityOfInfluence" .

prov:endedAtTime  rdf:type  owl:DatatypeProperty;
        rdfs:comment        "The time at which an activity ended. See also prov:startedAtTime."@en;
        rdfs:domain         prov:Activity;
        rdfs:isDefinedBy    <http://www.w3.org/ns/prov-o#>;
        rdfs:label          "endedAtTime";
        rdfs:range          xsd:dateTime;
        prov:category       "starting-point";
        prov:component      "entities-activities";
        prov:editorialNote  "It is the intent that the property chain holds: (prov:qualifiedEnd o prov:atTime) rdfs:subPropertyOf prov:endedAtTime."@en;
        prov:qualifiedForm  prov:atTime , prov:End .

prov:editorsDefinition
        rdf:type            owl:AnnotationProperty;
        rdfs:comment        "When the prov-o term does not have a definition drawn from prov-dm, and the prov-o editor provides one."@en;
        rdfs:isDefinedBy    prov: , <http://www.w3.org/ns/prov-o#>;
        rdfs:subPropertyOf  prov:definition .

prov:editorialNote  rdf:type  owl:AnnotationProperty;
        rdfs:comment      "A note by the OWL development team about how this term expresses the PROV-DM concept, or how it should be used in context of semantic web or linked data."@en;
        rdfs:isDefinedBy  prov: , <http://www.w3.org/ns/prov-o#> .

prov:dm  rdf:type           owl:AnnotationProperty;
        rdfs:comment        "A reference to the principal section of the PROV-DM document that describes this concept."@en;
        rdfs:isDefinedBy    prov: , <http://www.w3.org/ns/prov-o#>;
        rdfs:subPropertyOf  rdfs:seeAlso .

prov:definition  rdf:type  owl:AnnotationProperty;
        rdfs:comment      "A definition quoted from PROV-DM or PROV-CONSTRAINTS that describes the concept expressed with this OWL term."@en;
        rdfs:isDefinedBy  prov: , <http://www.w3.org/ns/prov-o#> .

prov:constraints  rdf:type  owl:AnnotationProperty;
        rdfs:comment        "A reference to the principal section of the PROV-CONSTRAINTS document that describes this concept."@en;
        rdfs:isDefinedBy    prov: , <http://www.w3.org/ns/prov-o#>;
        rdfs:subPropertyOf  rdfs:seeAlso .

prov:component  rdf:type  owl:AnnotationProperty;
        rdfs:comment      "Classify prov-o terms into six components according to prov-dm, including 'agents-responsibility', 'alternate', 'annotations', 'collections', 'derivations', and 'entities-activities'. This classification is used so that readers of prov-o specification can find its correspondence with the prov-dm specification."@en;
        rdfs:isDefinedBy  prov: , <http://www.w3.org/ns/prov-o#> .

prov:category  rdf:type   owl:AnnotationProperty;
        rdfs:comment      "Classify prov-o terms into three categories, including 'starting-point', 'qualifed', and 'extended'. This classification is used by the prov-o html document to gently introduce prov-o terms to its users. "@en;
        rdfs:isDefinedBy  prov: , <http://www.w3.org/ns/prov-o#> .

prov:atTime  rdf:type              owl:DatatypeProperty;
        rdfs:comment               "The time at which an InstantaneousEvent occurred, in the form of xsd:dateTime."@en;
        rdfs:domain                prov:InstantaneousEvent;
        rdfs:isDefinedBy           <http://www.w3.org/ns/prov-o#>;
        rdfs:label                 "atTime";
        rdfs:range                 xsd:dateTime;
        prov:category              "qualified";
        prov:component             "entities-activities";
        prov:sharesDefinitionWith  prov:InstantaneousEvent;
        prov:unqualifiedForm       prov:startedAtTime , prov:invalidatedAtTime , prov:generatedAtTime , prov:endedAtTime .

prov:atLocation  rdf:type          owl:ObjectProperty;
        rdfs:comment               "This property has multiple RDFS domains to suit multiple OWL Profiles. See <a href=\"#owl-profile\">PROV-O OWL Profile</a>." , "The Location of any resource."@en;
        rdfs:domain                [ rdf:type     owl:Class;
                                     owl:unionOf  ( prov:Activity prov:Agent prov:Entity prov:InstantaneousEvent )
                                   ];
        rdfs:isDefinedBy           <http://www.w3.org/ns/prov-o#>;
        rdfs:label                 "atLocation";
        rdfs:range                 prov:Location;
        prov:category              "expanded";
        prov:editorialNote         "This property is not functional because the many values could be at a variety of granularies (In this building, in this room, in that chair)."@en , "The naming of prov:atLocation parallels prov:atTime, and is not named prov:hadLocation to avoid conflicting with the convention that prov:had* properties are used on prov:Influence classes."@en;
        prov:inverse               "locationOf";
        prov:sharesDefinitionWith  prov:Location .

prov:aq  rdf:type           owl:AnnotationProperty;
        rdfs:isDefinedBy    prov: , <http://www.w3.org/ns/prov-o#>;
        rdfs:subPropertyOf  rdfs:seeAlso .

prov:alternateOf  rdf:type  owl:ObjectProperty;
        rdfs:domain       prov:Entity;
        rdfs:isDefinedBy  <http://www.w3.org/ns/prov-o-inverses#> , <http://www.w3.org/ns/prov-o#>;
        rdfs:label        "alternateOf";
        rdfs:range        prov:Entity;
        rdfs:seeAlso      prov:specializationOf;
        owl:inverseOf     prov:alternateOf;
        prov:category     "expanded";
        prov:component    "alternate";
        prov:constraints  "http://www.w3.org/TR/2013/REC-prov-constraints-20130430/#prov-dm-constraints-fig"^^xsd:anyURI;
        prov:definition   "Two alternate entities present aspects of the same thing. These aspects may be the same or different, and the alternate entities may or may not overlap in time."@en;
        prov:dm           "http://www.w3.org/TR/2013/REC-prov-dm-20130430/#term-alternate"^^xsd:anyURI;
        prov:inverse      "alternateOf";
        prov:n            "http://www.w3.org/TR/2013/REC-prov-n-20130430/#expression-alternate"^^xsd:anyURI .

prov:agent  rdf:type            owl:ObjectProperty;
        rdfs:domain             prov:AgentInfluence;
        rdfs:isDefinedBy        <http://www.w3.org/ns/prov-o#>;
        rdfs:label              "agent";
        rdfs:range              prov:Agent;
        rdfs:subPropertyOf      prov:influencer;
        prov:category           "qualified";
        prov:editorialNote      "This property behaves in spirit like rdf:object; it references the object of a prov:wasInfluencedBy triple."@en;
        prov:editorsDefinition  "The prov:agent property references an prov:Agent which influenced a resource. This property applies to an prov:AgentInfluence, which is given by a subproperty of prov:qualifiedInfluence from the influenced prov:Entity, prov:Activity or prov:Agent."@en;
        prov:inverse            "agentOfInfluence" .

prov:activity  rdf:type         owl:ObjectProperty;
        rdfs:domain             prov:ActivityInfluence;
        rdfs:isDefinedBy        <http://www.w3.org/ns/prov-o#>;
        rdfs:label              "activity";
        rdfs:range              prov:Activity;
        rdfs:subPropertyOf      prov:influencer;
        prov:category           "qualified";
        prov:editorialNote      "This property behaves in spirit like rdf:object; it references the object of a prov:wasInfluencedBy triple."@en;
        prov:editorsDefinition  "The prov:activity property references an prov:Activity which influenced a resource. This property applies to an prov:ActivityInfluence, which is given by a subproperty of prov:qualifiedInfluence from the influenced prov:Entity, prov:Activity or prov:Agent.";
        prov:inverse            "activityOfInfluence" .

prov:actedOnBehalfOf  rdf:type  owl:ObjectProperty;
        rdfs:comment            "An object property to express the accountability of an agent towards another agent. The subordinate agent acted on behalf of the responsible agent in an actual activity. "@en;
        rdfs:domain             prov:Agent;
        rdfs:isDefinedBy        <http://www.w3.org/ns/prov-o#>;
        rdfs:label              "actedOnBehalfOf";
        rdfs:range              prov:Agent;
        rdfs:subPropertyOf      prov:wasInfluencedBy;
        owl:propertyChainAxiom  ( prov:qualifiedDelegation prov:agent );
        prov:category           "starting-point";
        prov:component          "agents-responsibility";
        prov:inverse            "hadDelegate";
        prov:qualifiedForm      prov:qualifiedDelegation , prov:Delegation .

prov:Usage  rdf:type          owl:Class;
        rdfs:comment          "An instance of prov:Usage provides additional descriptions about the binary prov:used relation from some prov:Activity to an prov:Entity that it used. For example, :keynote prov:used :podium; prov:qualifiedUsage [ a prov:Usage; prov:entity :podium; :foo :bar ]."@en;
        rdfs:isDefinedBy      <http://www.w3.org/ns/prov-o#>;
        rdfs:label            "Usage";
        rdfs:subClassOf       prov:InstantaneousEvent , prov:EntityInfluence;
        prov:category         "qualified";
        prov:component        "entities-activities";
        prov:constraints      "http://www.w3.org/TR/2013/REC-prov-constraints-20130430/#prov-dm-constraints-fig"^^xsd:anyURI;
        prov:definition       "Usage is the beginning of utilizing an entity by an activity. Before usage, the activity had not begun to utilize this entity and could not have been affected by the entity."@en;
        prov:dm               "http://www.w3.org/TR/2013/REC-prov-dm-20130430/#term-Usage"^^xsd:anyURI;
        prov:n                "http://www.w3.org/TR/2013/REC-prov-n-20130430/#expression-Usage"^^xsd:anyURI;
        prov:unqualifiedForm  prov:used .

prov:Start  rdf:type          owl:Class;
        rdfs:comment          "An instance of prov:Start provides additional descriptions about the binary prov:wasStartedBy relation from some started prov:Activity to an prov:Entity that started it. For example, :foot_race prov:wasStartedBy :bang; prov:qualifiedStart [ a prov:Start; prov:entity :bang; :foo :bar; prov:atTime '2012-03-09T08:05:08-05:00'^^xsd:dateTime ] ."@en;
        rdfs:isDefinedBy      <http://www.w3.org/ns/prov-o#>;
        rdfs:label            "Start";
        rdfs:subClassOf       prov:InstantaneousEvent , prov:EntityInfluence;
        prov:category         "qualified";
        prov:component        "entities-activities";
        prov:constraints      "http://www.w3.org/TR/2013/REC-prov-constraints-20130430/#prov-dm-constraints-fig"^^xsd:anyURI;
        prov:definition       "Start is when an activity is deemed to have been started by an entity, known as trigger. The activity did not exist before its start. Any usage, generation, or invalidation involving an activity follows the activity's start. A start may refer to a trigger entity that set off the activity, or to an activity, known as starter, that generated the trigger."@en;
        prov:dm               "http://www.w3.org/TR/2013/REC-prov-dm-20130430/#term-Start"^^xsd:anyURI;
        prov:n                "http://www.w3.org/TR/2013/REC-prov-n-20130430/#expression-Start"^^xsd:anyURI;
        prov:unqualifiedForm  prov:wasStartedBy .

prov:SoftwareAgent  rdf:type  owl:Class;
        rdfs:isDefinedBy  prov: , <http://www.w3.org/ns/prov-o#>;
        rdfs:label        "SoftwareAgent";
        rdfs:subClassOf   owl:Thing , prov:Agent;
        prov:category     "expanded";
        prov:component    "agents-responsibility";
        prov:definition   "A software agent is running software."@en;
        prov:dm           "http://www.w3.org/TR/2012/WD-prov-dm-20120703/prov-dm.html#term-agent"^^xsd:anyURI , "http://www.w3.org/TR/2013/REC-prov-dm-20130430/#term-agent"^^xsd:anyURI;
        prov:n            "http://www.w3.org/TR/2012/WD-prov-dm-20120703/prov-n.html#expression-types"^^xsd:anyURI , "http://www.w3.org/TR/2013/REC-prov-n-20130430/#expression-types"^^xsd:anyURI .

prov:Role  rdf:type       owl:Class;
        rdfs:isDefinedBy  <http://www.w3.org/ns/prov-o#>;
        rdfs:label        "Role";
        rdfs:seeAlso      prov:hadRole;
        prov:category     "qualified";
        prov:component    "agents-responsibility";
        prov:definition   "A role is the function of an entity or agent with respect to an activity, in the context of a usage, generation, invalidation, association, start, and end."@en;
        prov:dm           "http://www.w3.org/TR/2013/REC-prov-dm-20130430/#term-attribute-role"^^xsd:anyURI;
        prov:n            "http://www.w3.org/TR/2013/REC-prov-n-20130430/#expression-attribute"^^xsd:anyURI .

prov:Revision  rdf:type       owl:Class;
        rdfs:comment          "An instance of prov:Revision provides additional descriptions about the binary prov:wasRevisionOf relation from some newer prov:Entity to an earlier prov:Entity. For example, :draft_2 prov:wasRevisionOf :draft_1; prov:qualifiedRevision [ a prov:Revision; prov:entity :draft_1; :foo :bar ]."@en;
        rdfs:isDefinedBy      <http://www.w3.org/ns/prov-o#>;
        rdfs:label            "Revision";
        rdfs:subClassOf       prov:Derivation;
        prov:category         "qualified";
        prov:component        "derivations";
        prov:definition       "A revision is a derivation for which the resulting entity is a revised version of some original. The implication here is that the resulting entity contains substantial content from the original. Revision is a particular case of derivation."@en;
        prov:dm               "http://www.w3.org/TR/2013/REC-prov-dm-20130430/#term-revision"^^xsd:anyURI;
        prov:n                "http://www.w3.org/TR/2013/REC-prov-n-20130430/#expression-Revision"^^xsd:anyURI;
        prov:unqualifiedForm  prov:wasRevisionOf .

prov:Quotation  rdf:type      owl:Class;
        rdfs:comment          "An instance of prov:Quotation provides additional descriptions about the binary prov:wasQuotedFrom relation from some taken prov:Entity from an earlier, larger prov:Entity. For example, :here_is_looking_at_you_kid prov:wasQuotedFrom :casablanca_script; prov:qualifiedQuotation [ a prov:Quotation; prov:entity :casablanca_script; :foo :bar ]."@en;
        rdfs:isDefinedBy      <http://www.w3.org/ns/prov-o#>;
        rdfs:label            "Quotation";
        rdfs:subClassOf       prov:Derivation;
        prov:category         "qualified";
        prov:component        "derivations";
        prov:definition       "A quotation is the repeat of (some or all of) an entity, such as text or image, by someone who may or may not be its original author. Quotation is a particular case of derivation."@en;
        prov:dm               "http://www.w3.org/TR/2013/REC-prov-dm-20130430/#term-quotation"^^xsd:anyURI;
        prov:n                "http://www.w3.org/TR/2013/REC-prov-n-20130430/#expression-quotation"^^xsd:anyURI;
        prov:unqualifiedForm  prov:wasQuotedFrom .

prov:PrimarySource  rdf:type  owl:Class;
        rdfs:comment          "An instance of prov:PrimarySource provides additional descriptions about the binary prov:hadPrimarySource relation from some secondary prov:Entity to an earlier, primary prov:Entity. For example, :blog prov:hadPrimarySource :newsArticle; prov:qualifiedPrimarySource [ a prov:PrimarySource; prov:entity :newsArticle; :foo :bar ] ."@en;
        rdfs:isDefinedBy      <http://www.w3.org/ns/prov-o#>;
        rdfs:label            "PrimarySource";
        rdfs:subClassOf       prov:Derivation;
        prov:category         "qualified";
        prov:component        "derivations";
        prov:definition       "A primary source for a topic refers to something produced by some agent with direct experience and knowledge about the topic, at the time of the topic's study, without benefit from hindsight.\n\nBecause of the directness of primary sources, they 'speak for themselves' in ways that cannot be captured through the filter of secondary sources. As such, it is important for secondary sources to reference those primary sources from which they were derived, so that their reliability can be investigated.\n\nA primary source relation is a particular case of derivation of secondary materials from their primary sources. It is recognized that the determination of primary sources can be up to interpretation, and should be done according to conventions accepted within the application's domain."@en;
        prov:dm               "http://www.w3.org/TR/2013/REC-prov-dm-20130430/#term-primary-source"^^xsd:anyURI;
        prov:n                "http://www.w3.org/TR/2013/REC-prov-n-20130430/#expression-original-source"^^xsd:anyURI;
        prov:unqualifiedForm  prov:hadPrimarySource .

prov:Plan  rdf:type       owl:Class;
        rdfs:comment      "There exist no prescriptive requirement on the nature of plans, their representation, the actions or steps they consist of, or their intended goals. Since plans may evolve over time, it may become necessary to track their provenance, so plans themselves are entities. Representing the plan explicitly in the provenance can be useful for various tasks: for example, to validate the execution as represented in the provenance record, to manage expectation failures, or to provide explanations."@en;
        rdfs:isDefinedBy  <http://www.w3.org/ns/prov-o#>;
        rdfs:label        "Plan";
        rdfs:subClassOf   prov:Entity;
        prov:category     "qualified" , "expanded";
        prov:component    "agents-responsibility";
        prov:definition   "A plan is an entity that represents a set of actions or steps intended by one or more agents to achieve some goals.";
        prov:dm           "http://www.w3.org/TR/2013/REC-prov-dm-20130430/#term-Association"^^xsd:anyURI;
        prov:n            "http://www.w3.org/TR/2013/REC-prov-n-20130430/#expression-Association"^^xsd:anyURI .

prov:Person  rdf:type     owl:Class;
        rdfs:isDefinedBy  <http://www.w3.org/ns/prov-o#>;
        rdfs:label        "Person";
        rdfs:subClassOf   prov:Agent;
        prov:category     "expanded";
        prov:component    "agents-responsibility";
        prov:definition   "Person agents are people."@en;
        prov:dm           "http://www.w3.org/TR/2013/REC-prov-dm-20130430/#term-agent"^^xsd:anyURI;
        prov:n            "http://www.w3.org/TR/2013/REC-prov-n-20130430/#expression-types"^^xsd:anyURI .

prov:Organization  rdf:type  owl:Class;
        rdfs:isDefinedBy  <http://www.w3.org/ns/prov-o#>;
        rdfs:label        "Organization";
        rdfs:subClassOf   prov:Agent;
        prov:category     "expanded";
        prov:component    "agents-responsibility";
        prov:definition   "An organization is a social or legal institution such as a company, society, etc.";
        prov:dm           "http://www.w3.org/TR/2013/REC-prov-dm-20130430/#term-agent"^^xsd:anyURI;
        prov:n            "http://www.w3.org/TR/2013/REC-prov-n-20130430/#expression-types"^^xsd:anyURI .

prov:Location  rdf:type   owl:Class;
        rdfs:isDefinedBy  <http://www.w3.org/ns/prov-o#>;
        rdfs:label        "Location";
        rdfs:seeAlso      prov:atLocation;
        prov:category     "expanded";
        prov:definition   "A location can be an identifiable geographic place (ISO 19112), but it can also be a non-geographic place such as a directory, row, or column. As such, there are numerous ways in which location can be expressed, such as by a coordinate, address, landmark, and so forth."@en;
        prov:dm           "http://www.w3.org/TR/2013/REC-prov-dm-20130430/#term-attribute-location"^^xsd:anyURI;
        prov:n            "http://www.w3.org/TR/2013/REC-prov-n-20130430/#expression-attribute"^^xsd:anyURI .

prov:Invalidation  rdf:type   owl:Class;
        rdfs:comment          "An instance of prov:Invalidation provides additional descriptions about the binary prov:wasInvalidatedBy relation from an invalidated prov:Entity to the prov:Activity that invalidated it. For example, :uncracked_egg prov:wasInvalidatedBy :baking; prov:qualifiedInvalidation [ a prov:Invalidation; prov:activity :baking; :foo :bar ]."@en;
        rdfs:isDefinedBy      <http://www.w3.org/ns/prov-o#>;
        rdfs:label            "Invalidation";
        rdfs:subClassOf       prov:InstantaneousEvent , prov:ActivityInfluence;
        prov:category         "qualified";
        prov:component        "entities-activities";
        prov:constraints      "http://www.w3.org/TR/2013/REC-prov-constraints-20130430/#prov-dm-constraints-fig"^^xsd:anyURI;
        prov:definition       "Invalidation is the start of the destruction, cessation, or expiry of an existing entity by an activity. The entity is no longer available for use (or further invalidation) after invalidation. Any generation or usage of an entity precedes its invalidation.";
        prov:dm               "http://www.w3.org/TR/2013/REC-prov-dm-20130430/#term-Invalidation"^^xsd:anyURI;
        prov:n                "http://www.w3.org/TR/2013/REC-prov-n-20130430/#expression-Invalidation"^^xsd:anyURI;
        prov:unqualifiedForm  prov:wasInvalidatedBy .

prov:InstantaneousEvent
        rdf:type          owl:Class;
        rdfs:comment      "An instantaneous event, or event for short, happens in the world and marks a change in the world, in its activities and in its entities. The term 'event' is commonly used in process algebra with a similar meaning. Events represent communications or interactions; they are assumed to be atomic and instantaneous."@en;
        rdfs:isDefinedBy  <http://www.w3.org/ns/prov-o#>;
        rdfs:label        "InstantaneousEvent";
        prov:category     "qualified";
        prov:component    "entities-activities";
        prov:constraints  "http://www.w3.org/TR/2013/REC-prov-constraints-20130430/#dfn-event"^^xsd:anyURI;
        prov:definition   "The PROV data model is implicitly based on a notion of instantaneous events (or just events), that mark transitions in the world. Events include generation, usage, or invalidation of entities, as well as starting or ending of activities. This notion of event is not first-class in the data model, but it is useful for explaining its other concepts and its semantics."@en .

prov:Influence  rdf:type      owl:Class;
        rdfs:comment          "Because prov:Influence is a broad relation, its most specific subclasses (e.g. prov:Communication, prov:Delegation, prov:End, prov:Revision, etc.) should be used when applicable."@en , "An instance of prov:Influence provides additional descriptions about the binary prov:wasInfluencedBy relation from some influenced Activity, Entity, or Agent to the influencing Activity, Entity, or Agent. For example, :stomach_ache prov:wasInfluencedBy :spoon; prov:qualifiedInfluence [ a prov:Influence; prov:entity :spoon; :foo :bar ] . Because prov:Influence is a broad relation, the more specific relations (Communication, Delegation, End, etc.) should be used when applicable."@en;
        rdfs:isDefinedBy      <http://www.w3.org/ns/prov-o#>;
        rdfs:label            "Influence";
        prov:category         "qualified";
        prov:component        "derivations";
        prov:definition       "Influence is the capacity of an entity, activity, or agent to have an effect on the character, development, or behavior of another by means of usage, start, end, generation, invalidation, communication, derivation, attribution, association, or delegation."@en;
        prov:dm               "http://www.w3.org/TR/2013/REC-prov-dm-20130430/#term-influence"^^xsd:anyURI;
        prov:n                "http://www.w3.org/TR/2013/REC-prov-n-20130430/#expression-influence"^^xsd:anyURI;
        prov:unqualifiedForm  prov:wasInfluencedBy .

prov:Generation  rdf:type     owl:Class;
        rdfs:comment          "An instance of prov:Generation provides additional descriptions about the binary prov:wasGeneratedBy relation from a generated prov:Entity to the prov:Activity that generated it. For example, :cake prov:wasGeneratedBy :baking; prov:qualifiedGeneration [ a prov:Generation; prov:activity :baking; :foo :bar ]."@en;
        rdfs:isDefinedBy      <http://www.w3.org/ns/prov-o#>;
        rdfs:label            "Generation";
        rdfs:subClassOf       prov:InstantaneousEvent , prov:ActivityInfluence;
        prov:category         "qualified";
        prov:component        "entities-activities";
        prov:constraints      "http://www.w3.org/TR/2013/REC-prov-constraints-20130430/#prov-dm-constraints-fig"^^xsd:anyURI;
        prov:definition       "Generation is the completion of production of a new entity by an activity. This entity did not exist before generation and becomes available for usage after this generation."@en;
        prov:dm               "http://www.w3.org/TR/2013/REC-prov-dm-20130430/#term-Generation"^^xsd:anyURI;
        prov:n                "http://www.w3.org/TR/2013/REC-prov-n-20130430/#expression-Generation"^^xsd:anyURI;
        prov:unqualifiedForm  prov:wasGeneratedBy .

prov:EntityInfluence  rdf:type  owl:Class;
        rdfs:comment            "It is not recommended that the type EntityInfluence be asserted without also asserting one of its more specific subclasses."@en , "EntityInfluence provides additional descriptions of an Entity's binary influence upon any other kind of resource. Instances of EntityInfluence use the prov:entity property to cite the influencing Entity."@en;
        rdfs:isDefinedBy        <http://www.w3.org/ns/prov-o#>;
        rdfs:label              "EntityInfluence";
        rdfs:seeAlso            prov:entity;
        rdfs:subClassOf         prov:Influence;
        prov:category           "qualified";
        prov:editorsDefinition  "EntityInfluence is the capacity of an entity to have an effect on the character, development, or behavior of another by means of usage, start, end, derivation, or other. "@en .

prov:Entity  rdf:type     owl:Class;
        rdfs:isDefinedBy  <http://www.w3.org/ns/prov-o#>;
        rdfs:label        "Entity";
        owl:disjointWith  prov:InstantaneousEvent;
        prov:category     "starting-point";
        prov:component    "entities-activities";
        prov:constraints  "http://www.w3.org/TR/2013/REC-prov-constraints-20130430/#prov-dm-constraints-fig"^^xsd:anyURI;
        prov:definition   "An entity is a physical, digital, conceptual, or other kind of thing with some fixed aspects; entities may be real or imaginary. "@en;
        prov:dm           "http://www.w3.org/TR/2013/REC-prov-dm-20130430/#term-entity"^^xsd:anyURI;
        prov:n            "http://www.w3.org/TR/2013/REC-prov-n-20130430/#expression-Entity"^^xsd:anyURI .

prov:End  rdf:type            owl:Class;
        rdfs:comment          "An instance of prov:End provides additional descriptions about the binary prov:wasEndedBy relation from some ended prov:Activity to an prov:Entity that ended it. For example, :ball_game prov:wasEndedBy :buzzer; prov:qualifiedEnd [ a prov:End; prov:entity :buzzer; :foo :bar; prov:atTime '2012-03-09T08:05:08-05:00'^^xsd:dateTime ]."@en;
        rdfs:isDefinedBy      <http://www.w3.org/ns/prov-o#>;
        rdfs:label            "End";
        rdfs:subClassOf       prov:InstantaneousEvent , prov:EntityInfluence;
        prov:category         "qualified";
        prov:component        "entities-activities";
        prov:constraints      "http://www.w3.org/TR/2013/REC-prov-constraints-20130430/#prov-dm-constraints-fig"^^xsd:anyURI;
        prov:definition       "End is when an activity is deemed to have been ended by an entity, known as trigger. The activity no longer exists after its end. Any usage, generation, or invalidation involving an activity precedes the activity's end. An end may refer to a trigger entity that terminated the activity, or to an activity, known as ender that generated the trigger."@en;
        prov:dm               "http://www.w3.org/TR/2013/REC-prov-dm-20130430/#term-End"^^xsd:anyURI;
        prov:n                "http://www.w3.org/TR/2013/REC-prov-n-20130430/#expression-End"^^xsd:anyURI;
        prov:unqualifiedForm  prov:wasEndedBy .

prov:EmptyCollection  rdf:type  owl:NamedIndividual , owl:Class;
        rdfs:isDefinedBy  <http://www.w3.org/ns/prov-o#>;
        rdfs:label        "EmptyCollection"@en;
        rdfs:subClassOf   prov:Collection;
        prov:category     "expanded";
        prov:component    "collections";
        prov:definition   "An empty collection is a collection without members."@en .

prov:Derivation  rdf:type     owl:Class;
        rdfs:comment          "The more specific forms of prov:Derivation (i.e., prov:Revision, prov:Quotation, prov:PrimarySource) should be asserted if they apply."@en , "An instance of prov:Derivation provides additional descriptions about the binary prov:wasDerivedFrom relation from some derived prov:Entity to another prov:Entity from which it was derived. For example, :chewed_bubble_gum prov:wasDerivedFrom :unwrapped_bubble_gum; prov:qualifiedDerivation [ a prov:Derivation; prov:entity :unwrapped_bubble_gum; :foo :bar ]."@en;
        rdfs:isDefinedBy      <http://www.w3.org/ns/prov-o#>;
        rdfs:label            "Derivation";
        rdfs:subClassOf       prov:EntityInfluence;
        prov:category         "qualified";
        prov:component        "derivations";
        prov:constraints      "http://www.w3.org/TR/2013/REC-prov-constraints-20130430/#prov-dm-constraints-fig"^^xsd:anyURI;
        prov:definition       "A derivation is a transformation of an entity into another, an update of an entity resulting in a new one, or the construction of a new entity based on a pre-existing entity."@en;
        prov:dm               "http://www.w3.org/TR/2013/REC-prov-dm-20130430/#term-Derivation"^^xsd:anyURI;
        prov:n                "http://www.w3.org/TR/2013/REC-prov-n-20130430/#Derivation-Relation"^^xsd:anyURI;
        prov:unqualifiedForm  prov:wasDerivedFrom .

prov:Delegation  rdf:type     owl:Class;
        rdfs:comment          "An instance of prov:Delegation provides additional descriptions about the binary prov:actedOnBehalfOf relation from a performing prov:Agent to some prov:Agent for whom it was performed. For example, :mixing prov:wasAssociatedWith :toddler . :toddler prov:actedOnBehalfOf :mother; prov:qualifiedDelegation [ a prov:Delegation; prov:entity :mother; :foo :bar ]."@en;
        rdfs:isDefinedBy      <http://www.w3.org/ns/prov-o#>;
        rdfs:label            "Delegation";
        rdfs:subClassOf       prov:AgentInfluence;
        prov:category         "qualified";
        prov:component        "agents-responsibility";
        prov:definition       "Delegation is the assignment of authority and responsibility to an agent (by itself or by another agent) to carry out a specific activity as a delegate or representative, while the agent it acts on behalf of retains some responsibility for the outcome of the delegated work.\n\nFor example, a student acted on behalf of his supervisor, who acted on behalf of the department chair, who acted on behalf of the university; all those agents are responsible in some way for the activity that took place but we do not say explicitly who bears responsibility and to what degree."@en;
        prov:dm               "http://www.w3.org/TR/2013/REC-prov-dm-20130430/#term-delegation"^^xsd:anyURI;
        prov:n                "http://www.w3.org/TR/2013/REC-prov-n-20130430/#expression-delegation"^^xsd:anyURI;
        prov:unqualifiedForm  prov:actedOnBehalfOf .

prov:Communication  rdf:type  owl:Class;
        rdfs:comment          "An instance of prov:Communication provides additional descriptions about the binary prov:wasInformedBy relation from an informed prov:Activity to the prov:Activity that informed it. For example, :you_jumping_off_bridge prov:wasInformedBy :everyone_else_jumping_off_bridge; prov:qualifiedCommunication [ a prov:Communication; prov:activity :everyone_else_jumping_off_bridge; :foo :bar ]."@en;
        rdfs:isDefinedBy      <http://www.w3.org/ns/prov-o#>;
        rdfs:label            "Communication";
        rdfs:subClassOf       prov:ActivityInfluence;
        prov:category         "qualified";
        prov:component        "entities-activities";
        prov:constraints      "http://www.w3.org/TR/2013/REC-prov-constraints-20130430/#prov-dm-constraints-fig"^^xsd:anyURI;
        prov:definition       "Communication is the exchange of an entity by two activities, one activity using the entity generated by the other.";
        prov:dm               "http://www.w3.org/TR/2013/REC-prov-dm-20130430/#term-Communication"^^xsd:anyURI;
        prov:n                "http://www.w3.org/TR/2013/REC-prov-n-20130430/#expression-wasInformedBy"^^xsd:anyURI;
        prov:unqualifiedForm  prov:wasInformedBy .

prov:Collection  rdf:type  owl:Class;
        rdfs:isDefinedBy  <http://www.w3.org/ns/prov-o#>;
        rdfs:label        "Collection";
        rdfs:subClassOf   prov:Entity;
        prov:category     "expanded";
        prov:component    "collections";
        prov:definition   "A collection is an entity that provides a structure to some constituents, which are themselves entities. These constituents are said to be member of the collections."@en;
        prov:dm           "http://www.w3.org/TR/2013/REC-prov-dm-20130430/#term-collection"^^xsd:anyURI .

prov:Bundle  rdf:type     owl:Class;
        rdfs:comment      "Note that there are kinds of bundles (e.g. handwritten letters, audio recordings, etc.) that are not expressed in PROV-O, but can be still be described by PROV-O."@en;
        rdfs:isDefinedBy  <http://www.w3.org/ns/prov-o#>;
        rdfs:label        "Bundle";
        rdfs:subClassOf   prov:Entity;
        prov:category     "expanded";
        prov:definition   "A bundle is a named set of provenance descriptions, and is itself an Entity, so allowing provenance of provenance to be expressed."@en;
        prov:dm           "http://www.w3.org/TR/2013/REC-prov-dm-20130430/#term-bundle-entity"^^xsd:anyURI;
        prov:n            "http://www.w3.org/TR/2013/REC-prov-n-20130430/#expression-bundle-declaration"^^xsd:anyURI .

prov:Attribution  rdf:type    owl:Class;
        rdfs:comment          "An instance of prov:Attribution provides additional descriptions about the binary prov:wasAttributedTo relation from an prov:Entity to some prov:Agent that had some responsible for it. For example, :cake prov:wasAttributedTo :baker; prov:qualifiedAttribution [ a prov:Attribution; prov:entity :baker; :foo :bar ]."@en;
        rdfs:isDefinedBy      <http://www.w3.org/ns/prov-o#>;
        rdfs:label            "Attribution";
        rdfs:subClassOf       prov:AgentInfluence;
        prov:category         "qualified";
        prov:component        "agents-responsibility";
        prov:constraints      "http://www.w3.org/TR/2013/REC-prov-constraints-20130430/#prov-dm-constraints-fig"^^xsd:anyURI;
        prov:definition       "Attribution is the ascribing of an entity to an agent.\n\nWhen an entity e is attributed to agent ag, entity e was generated by some unspecified activity that in turn was associated to agent ag. Thus, this relation is useful when the activity is not known, or irrelevant."@en;
        prov:dm               "http://www.w3.org/TR/2013/REC-prov-dm-20130430/#term-attribution"^^xsd:anyURI;
        prov:n                "http://www.w3.org/TR/2013/REC-prov-n-20130430/#expression-attribution"^^xsd:anyURI;
        prov:unqualifiedForm  prov:wasAttributedTo .

prov:Association  rdf:type    owl:Class;
        rdfs:comment          "An instance of prov:Association provides additional descriptions about the binary prov:wasAssociatedWith relation from an prov:Activity to some prov:Agent that had some responsiblity for it. For example, :baking prov:wasAssociatedWith :baker; prov:qualifiedAssociation [ a prov:Association; prov:agent :baker; :foo :bar ]."@en;
        rdfs:isDefinedBy      <http://www.w3.org/ns/prov-o#>;
        rdfs:label            "Association";
        rdfs:subClassOf       prov:AgentInfluence;
        prov:category         "qualified";
        prov:component        "agents-responsibility";
        prov:definition       "An activity association is an assignment of responsibility to an agent for an activity, indicating that the agent had a role in the activity. It further allows for a plan to be specified, which is the plan intended by the agent to achieve some goals in the context of this activity."@en;
        prov:dm               "http://www.w3.org/TR/2013/REC-prov-dm-20130430/#term-Association"^^xsd:anyURI;
        prov:n                "http://www.w3.org/TR/2013/REC-prov-n-20130430/#expression-Association"^^xsd:anyURI;
        prov:unqualifiedForm  prov:wasAssociatedWith .

prov:AgentInfluence  rdf:type   owl:Class;
        rdfs:comment            "It is not recommended that the type AgentInfluence be asserted without also asserting one of its more specific subclasses."@en , "AgentInfluence provides additional descriptions of an Agent's binary influence upon any other kind of resource. Instances of AgentInfluence use the prov:agent property to cite the influencing Agent."@en;
        rdfs:isDefinedBy        <http://www.w3.org/ns/prov-o#>;
        rdfs:label              "AgentInfluence";
        rdfs:seeAlso            prov:agent;
        rdfs:subClassOf         prov:Influence;
        prov:category           "qualified";
        prov:editorsDefinition  "AgentInfluence is the capacity of an agent to have an effect on the character, development, or behavior of another by means of attribution, association, delegation, or other."@en .

prov:Agent  rdf:type      owl:Class;
        rdfs:isDefinedBy  <http://www.w3.org/ns/prov-o#>;
        rdfs:label        "Agent";
        owl:disjointWith  prov:InstantaneousEvent;
        prov:category     "starting-point";
        prov:component    "agents-responsibility";
        prov:definition   "An agent is something that bears some form of responsibility for an activity taking place, for the existence of an entity, or for another agent's activity. "@en;
        prov:dm           "http://www.w3.org/TR/2013/REC-prov-dm-20130430/#term-agent"^^xsd:anyURI;
        prov:n            "http://www.w3.org/TR/2013/REC-prov-n-20130430/#expression-Agent"^^xsd:anyURI .

prov:ActivityInfluence
        rdf:type                owl:Class;
        rdfs:comment            "It is not recommended that the type ActivityInfluence be asserted without also asserting one of its more specific subclasses."@en , "ActivityInfluence provides additional descriptions of an Activity's binary influence upon any other kind of resource. Instances of ActivityInfluence use the prov:activity property to cite the influencing Activity."@en;
        rdfs:isDefinedBy        <http://www.w3.org/ns/prov-o#>;
        rdfs:label              "ActivityInfluence";
        rdfs:seeAlso            prov:activity;
        rdfs:subClassOf         prov:Influence;
        rdfs:subClassOf         [ rdf:type            owl:Restriction;
                                  owl:maxCardinality  "0"^^xsd:nonNegativeInteger;
                                  owl:onProperty      prov:hadActivity
                                ];
        owl:disjointWith        prov:EntityInfluence;
        prov:category           "qualified";
        prov:editorsDefinition  "ActivitiyInfluence is the capacity of an activity to have an effect on the character, development, or behavior of another by means of generation, invalidation, communication, or other."@en .

prov:Activity  rdf:type   owl:Class;
        rdfs:isDefinedBy  <http://www.w3.org/ns/prov-o#>;
        rdfs:label        "Activity";
        owl:disjointWith  prov:Entity;
        prov:category     "starting-point";
        prov:component    "entities-activities";
        prov:constraints  "http://www.w3.org/TR/2013/REC-prov-constraints-20130430/#prov-dm-constraints-fig"^^xsd:anyURI;
        prov:definition   "An activity is something that occurs over a period of time and acts upon or with entities; it may include consuming, processing, transforming, modifying, relocating, using, or generating entities.";
        prov:dm           "http://www.w3.org/TR/2013/REC-prov-dm-20130430/#term-Activity"^^xsd:anyURI;
        prov:n            "http://www.w3.org/TR/2013/REC-prov-n-20130430/#expression-Activity"^^xsd:anyURI .

owl:versionInfo  rdf:type  owl:AnnotationProperty .

owl:Thing  rdf:type  owl:Class .

rdfs:seeAlso  rdf:type  owl:AnnotationProperty;
        rdfs:comment  ""@en .

rdfs:label  rdf:type      owl:AnnotationProperty;
        rdfs:comment      ""@en;
        rdfs:isDefinedBy  prov: , <http://www.w3.org/ns/prov-o#> .

rdfs:isDefinedBy  rdf:type  owl:AnnotationProperty .

rdfs:comment  rdf:type    owl:AnnotationProperty;
        rdfs:comment      ""@en;
        rdfs:isDefinedBy  prov: , <http://www.w3.org/ns/prov-o#> .

prov:   rdf:type             owl:Ontology;
        rdfs:comment         "This document is published by the Provenance Working Group (http://www.w3.org/2011/prov/wiki/Main_Page).\n\nIf you wish to make comments regarding this document, please send them to public-prov-comments@w3.org (subscribe public-prov-comments-request@w3.org, archives http://lists.w3.org/\nArchives/Public/public-prov-comments/). All feedback is welcome."@en;
        rdfs:isDefinedBy     <http://www.w3.org/ns/prov>;
        rdfs:label           "W3C PROVenance Interchange"@en;
        rdfs:seeAlso         <http://www.w3.org/TR/prov-overview/>;
        owl:imports          <http://www.w3.org/ns/prov-aq#> , <http://www.w3.org/ns/prov-dc#> , <http://www.w3.org/ns/prov-dictionary#> , <http://www.w3.org/ns/prov-links#> , <http://www.w3.org/ns/prov-o#> , <http://www.w3.org/ns/prov-o-inverses#>;
        owl:versionIRI       <http://www.w3.org/ns/prov-20130430>;
        prov:wasDerivedFrom  <http://www.w3.org/ns/prov-o-inverses#> , <http://www.w3.org/ns/prov-o#> , <http://www.w3.org/ns/prov-aq#> , <http://www.w3.org/ns/prov-dc#> , <http://www.w3.org/ns/prov-dictionary#> , <http://www.w3.org/ns/prov-links#>;
        prov:wasRevisionOf   <http://www.w3.org/ns/prov-20130312> .
